<?xml version="1.0" encoding="utf-8"?>
<rdf:RDF
   xmlns:cco="https://www.commoncoreontologies.org/"
   xmlns:dcterms="http://purl.org/dc/terms/"
   xmlns:owl="http://www.w3.org/2002/07/owl#"
   xmlns:rdf="http://www.w3.org/1999/02/22-rdf-syntax-ns#"
   xmlns:rdfs="http://www.w3.org/2000/01/rdf-schema#"
   xmlns:skos="http://www.w3.org/2004/02/skos/core#"
>
  <rdf:Description rdf:about="https://www.commoncoreontologies.org/ont00001658">
    <rdf:type rdf:resource="http://www.w3.org/2002/07/owl#NamedIndividual"/>
    <rdf:type rdf:resource="https://www.commoncoreontologies.org/ont00001328"/>
    <rdfs:comment xml:lang="en">Teph (the 'eph' is written as subscript) is an ephemeris time argument developed and calculated at the Jet Propulsion Laboratory (JPL) and implemented in a series of numerically integrated Development Ephemerides (DE), including the currently used DE405. Teph is characterized as a relativistic coordinate time that is nearly equivalent to the IAU's definition of TCB, though Teph is not currently an IAU time standard. Teph is used by the JPL to generate the ephemerides it publishes to support spacecraft navigation and astronomy.</rdfs:comment>
    <rdfs:label xml:lang="en">Jet Propulsion Laboratory Ephemeris Time Argument</rdfs:label>
    <skos:altLabel xml:lang="en">JPL Ephemeris Time</skos:altLabel>
    <cco:ont00001753>Teph</cco:ont00001753>
    <cco:ont00001760 rdf:datatype="http://www.w3.org/2001/XMLSchema#anyURI">https://www.commoncoreontologies.org/InformationEntityOntology</cco:ont00001760>
  </rdf:Description>
  <rdf:Description rdf:about="https://www.commoncoreontologies.org/ont00001914">
    <rdf:type rdf:resource="http://www.w3.org/2002/07/owl#ObjectProperty"/>
    <rdfs:subPropertyOf rdf:resource="https://www.commoncoreontologies.org/ont00001904"/>
    <rdfs:domain rdf:resource="http://purl.obolibrary.org/obo/BFO_0000001"/>
    <rdfs:range rdf:resource="https://www.commoncoreontologies.org/ont00000293"/>
    <rdfs:label xml:lang="en">is measured by nominal</rdfs:label>
    <skos:definition xml:lang="en">x is_measured_by_nominal y iff y is an instance of Nominal Measurement Information Content Entity and x is an instance of Entity, such that y classifies x relative to some set of shared, possibly arbitrary, characteristics.</skos:definition>
    <cco:ont00001760 rdf:datatype="http://www.w3.org/2001/XMLSchema#anyURI">https://www.commoncoreontologies.org/InformationEntityOntology</cco:ont00001760>
  </rdf:Description>
  <rdf:Description rdf:about="https://www.commoncoreontologies.org/ont00001146">
    <rdf:type rdf:resource="http://www.w3.org/2002/07/owl#Class"/>
    <rdfs:subClassOf rdf:resource="https://www.commoncoreontologies.org/ont00001328"/>
    <rdfs:comment xml:lang="en">Sidereal Time is the angle measured from an observer's meridian along the celestial equator to the Great Circle that passes through the March equinox and both poles. This angle is usually expressed in Hours, Minutes, and Seconds.</rdfs:comment>
    <rdfs:label xml:lang="en">Sidereal Time Reference System</rdfs:label>
    <skos:definition xml:lang="en">A Temporal Reference System that is based on Earth's rate of rotation measured relative to one or more fixed Stars (rather than the Sun).</skos:definition>
    <cco:ont00001760 rdf:datatype="http://www.w3.org/2001/XMLSchema#anyURI">https://www.commoncoreontologies.org/InformationEntityOntology</cco:ont00001760>
  </rdf:Description>
  <rdf:Description rdf:about="https://www.commoncoreontologies.org/ont00001446">
    <rdf:type rdf:resource="http://www.w3.org/2002/07/owl#NamedIndividual"/>
    <rdf:type rdf:resource="https://www.commoncoreontologies.org/ont00001235"/>
    <rdfs:comment xml:lang="en">Mike Time Zone is the same local time as Yankee Time Zone, but is 1 Day (i.e. 24 Hours) ahead of Yankee Time Zone as they are on opposite sides of the International Date Line.</rdfs:comment>
    <rdfs:comment xml:lang="en">Offset from Universal Coordinated Time = UTC+12</rdfs:comment>
    <rdfs:label xml:lang="en">Mike Time Zone</rdfs:label>
    <cco:ont00001753>M</cco:ont00001753>
    <cco:ont00001760 rdf:datatype="http://www.w3.org/2001/XMLSchema#anyURI">https://www.commoncoreontologies.org/InformationEntityOntology</cco:ont00001760>
  </rdf:Description>
  <rdf:Description rdf:about="https://www.commoncoreontologies.org/ont00001488">
    <rdf:type rdf:resource="http://www.w3.org/2002/07/owl#NamedIndividual"/>
    <rdf:type rdf:resource="https://www.commoncoreontologies.org/ont00001235"/>
    <rdfs:comment xml:lang="en">Offset from Universal Coordinated Time = UTC-7</rdfs:comment>
    <rdfs:label xml:lang="en">Tango Time Zone</rdfs:label>
    <cco:ont00001753>T</cco:ont00001753>
    <cco:ont00001760 rdf:datatype="http://www.w3.org/2001/XMLSchema#anyURI">https://www.commoncoreontologies.org/InformationEntityOntology</cco:ont00001760>
  </rdf:Description>
  <rdf:Description rdf:about="https://www.commoncoreontologies.org/ont00000990">
    <rdf:type rdf:resource="http://www.w3.org/2002/07/owl#Class"/>
    <rdfs:subClassOf rdf:resource="https://www.commoncoreontologies.org/ont00000003"/>
    <rdfs:label xml:lang="en">Nickname</rdfs:label>
    <skos:definition xml:lang="en">A Designative Name that is a familiar or humorous substitute for an entity's Proper Name.</skos:definition>
    <skos:example>Ike, Chief, P-Fox</skos:example>
    <cco:ont00001760 rdf:datatype="http://www.w3.org/2001/XMLSchema#anyURI">https://www.commoncoreontologies.org/InformationEntityOntology</cco:ont00001760>
  </rdf:Description>
  <rdf:Description rdf:about="https://www.commoncoreontologies.org/ont00001364">
    <rdf:type rdf:resource="http://www.w3.org/2002/07/owl#Class"/>
    <owl:equivalentClass rdf:nodeID="na8580e9876f64da8bd2fccebf064ee6cb75"/>
    <rdfs:subClassOf rdf:resource="https://www.commoncoreontologies.org/ont00001163"/>
    <rdfs:comment xml:lang="en">Four of the subtypes of measurements used here (Interval, Nominal, Ordinal, and Ratio) were originally defined by S.S. Stevens in the article "On the Theory of Scales of Measurement" in Science, Vol. 103 No. 2684 on June 7, 1946. For an introductory article with links to additional content including criticisms and alternate classifications of measurements see https://en.wikipedia.org/wiki/Level_of_measurement</rdfs:comment>
    <rdfs:label xml:lang="en">Interval Measurement Information Content Entity</rdfs:label>
    <skos:definition xml:lang="en">A Measurement Information Content Entity that places a Quality of an Entity onto some interval scale having no true zero value.</skos:definition>
    <skos:example xml:lang="en">The sentence "The temperature reached -27 degrees Fahrenheit on January 20, 1985 in Chicago, IL." is the carrier of an interval measurement as 0 degrees on the Fahrenheit scale does not describe absolute zero.</skos:example>
    <cco:ont00001760 rdf:datatype="http://www.w3.org/2001/XMLSchema#anyURI">https://www.commoncoreontologies.org/InformationEntityOntology</cco:ont00001760>
  </rdf:Description>
  <rdf:Description rdf:about="https://www.commoncoreontologies.org/ont00000314">
    <rdf:type rdf:resource="http://www.w3.org/2002/07/owl#Class"/>
    <rdfs:subClassOf rdf:resource="http://purl.obolibrary.org/obo/BFO_0000019"/>
    <rdfs:subClassOf rdf:nodeID="na8580e9876f64da8bd2fccebf064ee6cb18"/>
    <rdfs:comment xml:lang="en">Typically, an IQE will be a complex pattern made up of multiple qualities joined together spatially.</rdfs:comment>
    <rdfs:label xml:lang="en">Information Quality Entity</rdfs:label>
    <skos:altLabel xml:lang="en">IQE</skos:altLabel>
    <skos:definition xml:lang="en">A Quality that concretizes some Information Content Entity.</skos:definition>
    <cco:ont00001760 rdf:datatype="http://www.w3.org/2001/XMLSchema#anyURI">https://www.commoncoreontologies.org/InformationEntityOntology</cco:ont00001760>
  </rdf:Description>
  <rdf:Description rdf:nodeID="na8580e9876f64da8bd2fccebf064ee6cb40">
    <owl:intersectionOf rdf:nodeID="na8580e9876f64da8bd2fccebf064ee6cb42"/>
    <rdf:type rdf:resource="http://www.w3.org/2002/07/owl#Class"/>
  </rdf:Description>
  <rdf:Description rdf:about="https://www.commoncoreontologies.org/ont00000833">
    <rdf:type rdf:resource="http://www.w3.org/2002/07/owl#Class"/>
    <rdfs:subClassOf rdf:resource="https://www.commoncoreontologies.org/ont00000973"/>
    <rdfs:subClassOf rdf:nodeID="na8580e9876f64da8bd2fccebf064ee6cb44"/>
    <rdfs:subClassOf rdf:nodeID="na8580e9876f64da8bd2fccebf064ee6cb45"/>
    <rdfs:subClassOf rdf:nodeID="na8580e9876f64da8bd2fccebf064ee6cb46"/>
    <rdfs:label xml:lang="en">Julian Date Identifier</rdfs:label>
    <skos:definition xml:lang="en">A Decimal Time of Day Identifier that designates a Julian Date and is composed of both a Julian Day Number and a Julian Date Fraction.</skos:definition>
    <cco:ont00001760 rdf:datatype="http://www.w3.org/2001/XMLSchema#anyURI">https://www.commoncoreontologies.org/InformationEntityOntology</cco:ont00001760>
  </rdf:Description>
  <rdf:Description rdf:nodeID="na8580e9876f64da8bd2fccebf064ee6cb69">
    <rdf:first rdf:resource="https://www.commoncoreontologies.org/ont00000958"/>
    <rdf:rest rdf:nodeID="na8580e9876f64da8bd2fccebf064ee6cb70"/>
  </rdf:Description>
  <rdf:Description rdf:about="https://www.commoncoreontologies.org/ont00002008">
    <rdf:type rdf:resource="http://www.w3.org/2002/07/owl#Class"/>
    <rdfs:subClassOf rdf:resource="https://www.commoncoreontologies.org/ont00002007"/>
    <rdfs:label xml:lang="en">Code List</rdfs:label>
    <skos:definition xml:lang="en">A List whose parts are Code Identifiers.</skos:definition>
    <cco:ont00001760 rdf:datatype="http://www.w3.org/2001/XMLSchema#anyURI">https://www.commoncoreontologies.org/InformationEntityOntology</cco:ont00001760>
  </rdf:Description>
  <rdf:Description rdf:about="https://www.commoncoreontologies.org/ont00002007">
    <rdf:type rdf:resource="http://www.w3.org/2002/07/owl#Class"/>
    <rdfs:subClassOf rdf:resource="https://www.commoncoreontologies.org/ont00002001"/>
    <rdfs:label xml:lang="en">List</rdfs:label>
    <skos:definition xml:lang="en">A Media Content Entity whose parts are the subject of some Sequence Position Ordinality.</skos:definition>
    <cco:ont00001754 rdf:datatype="http://www.w3.org/2001/XMLSchema#anyURI">https://en.wikipedia.org/w/index.php?title=List_(abstract_data_type)&amp;oldid=1041588680</cco:ont00001754>
    <cco:ont00001760 rdf:datatype="http://www.w3.org/2001/XMLSchema#anyURI">https://www.commoncoreontologies.org/InformationEntityOntology</cco:ont00001760>
  </rdf:Description>
  <rdf:Description rdf:about="https://www.commoncoreontologies.org/ont00001674">
    <rdf:type rdf:resource="http://www.w3.org/2002/07/owl#NamedIndividual"/>
    <rdf:type rdf:resource="https://www.commoncoreontologies.org/ont00000276"/>
    <rdfs:comment xml:lang="en">The Gregorian Calendar was instituted by Pope Gregory XIII via papal bull on 24 February 1582 as a reform of the Julian Calendar to stop the drift of the calendar with respect to the equinoxes and solstices. The Gregorian Calendar is currently the most widely used civil Calendar System in the world and is 13 days ahead of the Julian Calendar Date.</rdfs:comment>
    <rdfs:label xml:lang="en">Gregorian Calendar</rdfs:label>
    <skos:definition xml:lang="en">A Solar Calendar System that has a regular Year of 365 24-Hour Days divided into 12 Months with a leap day added at the end of February every 4 Years except Years that are evenly divisible by 100 but not 400 such that there are 97 leap Years every 400 Years and the average length of a Gregorian Year is 365.2425 Days (365 Days 5 Hours 49 Minutes 12 Seconds).</skos:definition>
    <cco:ont00001754 rdf:datatype="http://www.w3.org/2001/XMLSchema#anyURI">https://en.wikipedia.org/w/index.php?title=Gregorian_calendar&amp;oldid=1062360692</cco:ont00001754>
    <cco:ont00001760 rdf:datatype="http://www.w3.org/2001/XMLSchema#anyURI">https://www.commoncoreontologies.org/InformationEntityOntology</cco:ont00001760>
  </rdf:Description>
  <rdf:Description rdf:about="https://www.commoncoreontologies.org/ont00000845">
    <rdf:type rdf:resource="http://www.w3.org/2002/07/owl#Class"/>
    <rdfs:subClassOf rdf:resource="https://www.commoncoreontologies.org/ont00001022"/>
    <rdfs:comment xml:lang="en">A percentage is one way to express a proportional measure where the decimal expression of the proportion is multiplied by 100, thus giving the proportional value with respect to a whole of 100. E.g., the ratio of pigs to cows on a farm is 44 to 79 (44:79 or 44/79). The proportion of pigs to total animals is 44 to 123 or 44/123. The percentage of pigs is the decimal equivalent of the proportion (0.36) multiplied by a 100 (36%). The percentage can be expressed as a proportion where the numerator value is transformed for a denominator of 100, i.e., 36 of a 100 animals are pigs (36/100).</rdfs:comment>
    <rdfs:comment xml:lang="en">We may want to add either a subclass for Percentage or a data property (has percentage value) that links the percentage expression for a proportion to the relevant IBE.</rdfs:comment>
    <rdfs:label xml:lang="en">Proportional Ratio Measurement Information Content Entity</rdfs:label>
    <skos:definition xml:lang="en">A Ratio Measurement Information Content Entity that is a measurement of a portion of a whole (described by the numerator) compared against that whole (described by the denominator) where the whole is a nominally described set of like entities.</skos:definition>
    <cco:ont00001760 rdf:datatype="http://www.w3.org/2001/XMLSchema#anyURI">https://www.commoncoreontologies.org/InformationEntityOntology</cco:ont00001760>
  </rdf:Description>
  <rdf:Description rdf:about="https://www.commoncoreontologies.org/ont00001916">
    <rdf:type rdf:resource="http://www.w3.org/2002/07/owl#ObjectProperty"/>
    <rdfs:subPropertyOf rdf:resource="https://www.commoncoreontologies.org/ont00001808"/>
    <rdfs:domain rdf:resource="https://www.commoncoreontologies.org/ont00000686"/>
    <rdfs:range rdf:resource="http://purl.obolibrary.org/obo/BFO_0000001"/>
    <rdfs:label xml:lang="en">designates</rdfs:label>
    <skos:definition xml:lang="en">x designates y iff x is an instance of a Designative Information Content Entity, and y is an instance of an Entity, such that given some context, x uniquely distinguishes y from other entities.</skos:definition>
    <skos:example>a URL designates the location of a Web Page on the internet</skos:example>
    <skos:example>a person's name designates that person</skos:example>
    <skos:example>a vehicle identification number designates some vehicle</skos:example>
    <skos:scopeNote xml:lang="en">Given a stronger temporal interpretation, this property may be functional. For more info please refer to https://github.com/BFO-ontology/BFO-2020/tree/master/src/owl/temporal%20extensions.</skos:scopeNote>
    <cco:ont00001760 rdf:datatype="http://www.w3.org/2001/XMLSchema#anyURI">https://www.commoncoreontologies.org/InformationEntityOntology</cco:ont00001760>
  </rdf:Description>
  <rdf:Description rdf:about="https://www.commoncoreontologies.org/ont00001352">
    <rdf:type rdf:resource="http://www.w3.org/2002/07/owl#Class"/>
    <rdfs:subClassOf rdf:resource="https://www.commoncoreontologies.org/ont00000829"/>
    <rdfs:comment xml:lang="en">Greenwich Mean Time (GMT) is the mean solar time at the Royal Observatory in Greenwich, London and has been superseded by Coordinated Universal Time (UTC).</rdfs:comment>
    <rdfs:label xml:lang="en">Greenwich Mean Time Zone Identifier</rdfs:label>
    <skos:definition xml:lang="en">A Time Zone Identifier that designates a spatial region where the local time is calculated according to the specified offset from Greenwich Mean Time.</skos:definition>
    <cco:ont00001760 rdf:datatype="http://www.w3.org/2001/XMLSchema#anyURI">https://www.commoncoreontologies.org/InformationEntityOntology</cco:ont00001760>
  </rdf:Description>
  <rdf:Description rdf:about="https://www.commoncoreontologies.org/ont00000683">
    <rdf:type rdf:resource="http://www.w3.org/2002/07/owl#Class"/>
    <rdfs:subClassOf rdf:resource="https://www.commoncoreontologies.org/ont00000605"/>
    <rdfs:label xml:lang="en">Diminutive Name</rdfs:label>
    <skos:definition xml:lang="en">An Abbreviated Name that is a familiar form of a Proper Name.</skos:definition>
    <skos:example>Alex, Bob, Cathy</skos:example>
    <skos:scopeNote xml:lang="en">"Familiar form of a Proper Name" means: that the name is (originally) a short, affectionate version of the fuller name, used (originally) by family or friends.</skos:scopeNote>
    <cco:ont00001760 rdf:datatype="http://www.w3.org/2001/XMLSchema#anyURI">https://www.commoncoreontologies.org/InformationEntityOntology</cco:ont00001760>
  </rdf:Description>
  <rdf:Description rdf:about="https://www.commoncoreontologies.org/ont00002041">
    <rdf:type rdf:resource="http://www.w3.org/2002/07/owl#Class"/>
    <rdfs:subClassOf rdf:resource="https://www.commoncoreontologies.org/ont00002039"/>
    <rdfs:label xml:lang="en">Transcript</rdfs:label>
    <skos:definition xml:lang="en">A Document Content Entity that was originally recorded in a different medium.</skos:definition>
    <cco:ont00001754 rdf:datatype="http://www.w3.org/2001/XMLSchema#anyURI">https://en.wikipedia.org/w/index.php?title=Transcript&amp;oldid=1038510063</cco:ont00001754>
    <cco:ont00001760 rdf:datatype="http://www.w3.org/2001/XMLSchema#anyURI">https://www.commoncoreontologies.org/InformationEntityOntology</cco:ont00001760>
  </rdf:Description>
  <rdf:Description rdf:about="https://www.commoncoreontologies.org/ont00001603">
    <rdf:type rdf:resource="http://www.w3.org/2002/07/owl#NamedIndividual"/>
    <rdf:type rdf:resource="https://www.commoncoreontologies.org/ont00001235"/>
    <rdfs:comment xml:lang="en">Offset from Universal Coordinated Time = UTC-1</rdfs:comment>
    <rdfs:label xml:lang="en">November Time Zone</rdfs:label>
    <cco:ont00001753>N</cco:ont00001753>
    <cco:ont00001760 rdf:datatype="http://www.w3.org/2001/XMLSchema#anyURI">https://www.commoncoreontologies.org/InformationEntityOntology</cco:ont00001760>
  </rdf:Description>
  <rdf:Description rdf:about="https://www.commoncoreontologies.org/ont00000592">
    <rdf:type rdf:resource="http://www.w3.org/2002/07/owl#Class"/>
    <rdfs:subClassOf rdf:resource="https://www.commoncoreontologies.org/ont00001163"/>
    <rdfs:comment xml:lang="en">'Deviation Measurement Information Content Entity' and 'Veracity Measurement Information Content Entity' are complementary notions. Deviation is a measure of whether reality conforms to an ICE (e.g., a plan or prediction), whereas Veracity is a measure of whether a Descriptive ICE conforms to reality.</rdfs:comment>
    <rdfs:comment xml:lang="en">Note, the term 'accuracy' is avoided due to its ambiguity between: correctness-of-performance (see: 'Reliability Measurement Information Content Entity'), correctness-of-information ('Veracity Measurement Information Content Entity'), and adherance-to-expectations (see: 'Deviation Measurement Information Content Entity').</rdfs:comment>
    <rdfs:label xml:lang="en">Veracity Measurement Information Content Entity</rdfs:label>
    <skos:altLabel xml:lang="en">Accuracy of Information</skos:altLabel>
    <skos:altLabel xml:lang="en">Trueness Measurement</skos:altLabel>
    <skos:altLabel xml:lang="en">Veracity Measurement</skos:altLabel>
    <skos:definition xml:lang="en">A Measurement Information Content Entity that is a measurement of the extent to which a description conforms to the reality it describes.</skos:definition>
    <cco:ont00001760 rdf:datatype="http://www.w3.org/2001/XMLSchema#anyURI">https://www.commoncoreontologies.org/InformationEntityOntology</cco:ont00001760>
  </rdf:Description>
  <rdf:Description rdf:about="https://www.commoncoreontologies.org/ont00001398">
    <rdf:type rdf:resource="http://www.w3.org/2002/07/owl#NamedIndividual"/>
    <rdf:type rdf:resource="https://www.commoncoreontologies.org/ont00000469"/>
    <rdfs:label xml:lang="en">Global Area Reference System</rdfs:label>
    <cco:ont00001753>GARS</cco:ont00001753>
    <cco:ont00001760 rdf:datatype="http://www.w3.org/2001/XMLSchema#anyURI">https://www.commoncoreontologies.org/InformationEntityOntology</cco:ont00001760>
  </rdf:Description>
  <rdf:Description rdf:nodeID="na8580e9876f64da8bd2fccebf064ee6cb43">
    <rdf:first rdf:nodeID="na8580e9876f64da8bd2fccebf064ee6cb41"/>
    <rdf:rest rdf:resource="http://www.w3.org/1999/02/22-rdf-syntax-ns#nil"/>
  </rdf:Description>
  <rdf:Description rdf:about="https://www.commoncoreontologies.org/ont00002037">
    <rdf:type rdf:resource="http://www.w3.org/2002/07/owl#Class"/>
    <rdfs:subClassOf rdf:resource="https://www.commoncoreontologies.org/ont00002001"/>
    <rdfs:label xml:lang="en">Information Line</rdfs:label>
    <skos:definition xml:lang="en">A Media Content entity consisting of a single line or row in some Document Content entity of which it is a part.</skos:definition>
    <skos:example>a line in a computer file that bears a portion of code for some computer program</skos:example>
    <skos:example>a line of data in a database</skos:example>
    <skos:example>a line of text in a book</skos:example>
    <cco:ont00001760 rdf:datatype="http://www.w3.org/2001/XMLSchema#anyURI">https://www.commoncoreontologies.org/InformationEntityOntology</cco:ont00001760>
  </rdf:Description>
  <rdf:Description rdf:about="https://www.commoncoreontologies.org/ont00001461">
    <rdf:type rdf:resource="http://www.w3.org/2002/07/owl#NamedIndividual"/>
    <rdf:type rdf:resource="https://www.commoncoreontologies.org/ont00001328"/>
    <rdfs:comment xml:lang="en">TDB is a linear scaling of Barycentric Coordinate Time (TCB) and is a relativistic coordinate time scale used in astronomy as a time standard that accounts for time dilation when calculating Orbits and Ephemerides of Astronomical Bodies and interplanetary Spacecraft in the Solar System. TDB is a successor of Ephemeris Time (ET) and is nearly equivalent to the time scale Teph used for DE405 planetary and lunar ephemerides generated by the Jet Propulsion Laboratory.</rdfs:comment>
    <rdfs:label xml:lang="en">Barycentric Dynamical Time</rdfs:label>
    <cco:ont00001753>TDB</cco:ont00001753>
    <cco:ont00001760 rdf:datatype="http://www.w3.org/2001/XMLSchema#anyURI">https://www.commoncoreontologies.org/InformationEntityOntology</cco:ont00001760>
  </rdf:Description>
  <rdf:Description rdf:about="https://www.commoncoreontologies.org/ont00001811">
    <rdf:type rdf:resource="http://www.w3.org/2002/07/owl#ObjectProperty"/>
    <rdfs:subPropertyOf rdf:resource="https://www.commoncoreontologies.org/ont00001966"/>
    <owl:inverseOf rdf:resource="https://www.commoncoreontologies.org/ont00001963"/>
    <rdfs:domain rdf:resource="https://www.commoncoreontologies.org/ont00001010"/>
    <rdfs:range rdf:resource="http://purl.obolibrary.org/obo/BFO_0000001"/>
    <rdfs:label xml:lang="en">is an ordinal measurement of</rdfs:label>
    <skos:definition xml:lang="en">x is_an_ordinal_measurement_of y iff x is an instance of Information Content Entity and y is an instance of Entity and y is_measured_by_ordinal x.</skos:definition>
    <cco:ont00001760 rdf:datatype="http://www.w3.org/2001/XMLSchema#anyURI">https://www.commoncoreontologies.org/InformationEntityOntology</cco:ont00001760>
  </rdf:Description>
  <rdf:Description rdf:about="https://www.commoncoreontologies.org/ont00000731">
    <rdf:type rdf:resource="http://www.w3.org/2002/07/owl#Class"/>
    <rdfs:subClassOf rdf:resource="https://www.commoncoreontologies.org/ont00001163"/>
    <rdfs:comment xml:lang="en">'Deviation Measurement Information Content Entity' and 'Veracity Measurement Information Content Entity' are complementary notions. Deviation is a measure of whether reality conforms to an ICE (e.g., a plan or prediction), whereas Veracity is a measure of whether a Descriptive ICE conforms to reality.</rdfs:comment>
    <rdfs:comment xml:lang="en">Note, the term 'accuracy' is avoided due to its ambiguity between: correctness-of-performance (see: 'Reliability Measurement Information Content Entity'), correctness-of-information (see: 'Veracity Measurement Information Content Entity'), and adherance-to-expectations ('Deviation Measurement Information Content Entity').</rdfs:comment>
    <rdfs:label xml:lang="en">Deviation Measurement Information Content Entity</rdfs:label>
    <skos:altLabel xml:lang="en">Conformance Measurement</skos:altLabel>
    <skos:altLabel xml:lang="en">Degree of Conformance</skos:altLabel>
    <skos:altLabel xml:lang="en">Degree of Deviation</skos:altLabel>
    <skos:altLabel xml:lang="en">Deviation Measurement</skos:altLabel>
    <skos:definition xml:lang="en">A Measurement Information Content Entity that is a measurement of the extent to which an entity conforms to how it is expected or supposed to be.</skos:definition>
    <skos:example>a missile impact deviates from its target location by 100 feet</skos:example>
    <skos:example>a satellite deviaties from its predicted orbital path by 5 kilometers</skos:example>
    <skos:example>an overweight piece of luggage deviates from an airline's maximum allowed weight by +10 pounds</skos:example>
    <skos:scopeNote xml:lang="en">In order for a Deviation to exist, an entity must first be expected, represented, prescribed, or predicted as being a certain way. Then, at a future time, this value can be compared to its actual, reported, or measured value to determine the Deviation between these values.</skos:scopeNote>
    <cco:ont00001760 rdf:datatype="http://www.w3.org/2001/XMLSchema#anyURI">https://www.commoncoreontologies.org/InformationEntityOntology</cco:ont00001760>
  </rdf:Description>
  <rdf:Description rdf:about="https://www.commoncoreontologies.org/ont00000669">
    <rdf:type rdf:resource="http://www.w3.org/2002/07/owl#Class"/>
    <rdfs:subClassOf rdf:resource="https://www.commoncoreontologies.org/ont00001022"/>
    <rdfs:label xml:lang="en">Distance Measurement Information Content Entity</rdfs:label>
    <skos:definition xml:lang="en">A Ratio Measurement Information Content Entity that is a measurement of a One-Dimensional Extent inhering in some Site that is externally connected to two Independent Continuants.</skos:definition>
    <skos:scopeNote xml:lang="en">Displacement (vector) is the shortest possible distance (scalar) between two points. Further thought is needed to adequately handle measurements of distance traveled along a path, e.g., a circuitous path or an arc (such as the surface of a planet), versus the simple case of a direct, straight line between two points.</skos:scopeNote>
    <skos:scopeNote xml:lang="en">Distance is a measure between two reference points, which are located on or in, or in some manner part of, the two obejcts for which the length of the extent between is sought. For exmple, the center point of the indentation of a ball in the sand and the edge of the foul line, the forwardmost point on a car's bumper and the closest point on the 2-dimensional plane that serves as the fiat boundary of a crosswalk, the center of an antenna array and closest point on ground.</skos:scopeNote>
    <cco:ont00001760 rdf:datatype="http://www.w3.org/2001/XMLSchema#anyURI">https://www.commoncoreontologies.org/InformationEntityOntology</cco:ont00001760>
  </rdf:Description>
  <rdf:Description rdf:about="https://www.commoncoreontologies.org/ont00001436">
    <rdf:type rdf:resource="http://www.w3.org/2002/07/owl#NamedIndividual"/>
    <rdf:type rdf:resource="https://www.commoncoreontologies.org/ont00000630"/>
    <rdfs:label xml:lang="en">Universal Time 1 D</rdfs:label>
    <cco:ont00001753>UT1D</cco:ont00001753>
    <cco:ont00001760 rdf:datatype="http://www.w3.org/2001/XMLSchema#anyURI">https://www.commoncoreontologies.org/InformationEntityOntology</cco:ont00001760>
  </rdf:Description>
  <rdf:Description rdf:about="https://www.commoncoreontologies.org/ont00001966">
    <rdf:type rdf:resource="http://www.w3.org/2002/07/owl#ObjectProperty"/>
    <rdfs:subPropertyOf rdf:resource="https://www.commoncoreontologies.org/ont00001982"/>
    <rdfs:domain rdf:resource="https://www.commoncoreontologies.org/ont00001163"/>
    <rdfs:range rdf:resource="http://purl.obolibrary.org/obo/BFO_0000001"/>
    <rdfs:comment xml:lang="en">This object property, as well as all of its children are typified as functional properties. This means that for instances x, y, and z if x is a measurement of y and x is a measurement of z, then y = z.</rdfs:comment>
    <rdfs:label xml:lang="en">is a measurement of</rdfs:label>
    <skos:definition xml:lang="en">x is_a_measurement_of y iff x is an instance of Information Content Entity and y is an instance of Entity, such that x describes some attribute of y relative to some scale or classification scheme.</skos:definition>
    <skos:scopeNote xml:lang="en">Given a stronger temporal interpretation, this property may be functional. For more info please refer to https://github.com/BFO-ontology/BFO-2020/tree/master/src/owl/temporal%20extensions.</skos:scopeNote>
    <cco:ont00001760 rdf:datatype="http://www.w3.org/2001/XMLSchema#anyURI">https://www.commoncoreontologies.org/InformationEntityOntology</cco:ont00001760>
  </rdf:Description>
  <rdf:Description rdf:about="https://www.commoncoreontologies.org/ont00001235">
    <rdf:type rdf:resource="http://www.w3.org/2002/07/owl#Class"/>
    <rdfs:subClassOf rdf:resource="https://www.commoncoreontologies.org/ont00000829"/>
    <rdfs:label xml:lang="en">Military Time Zone Identifier</rdfs:label>
    <skos:definition xml:lang="en">A Time Zone Identifier that designates a spatial region where the local time is calculated according to the specified offset from Zulu time, which has no offset from Coordinated Universal Time.</skos:definition>
    <cco:ont00001760 rdf:datatype="http://www.w3.org/2001/XMLSchema#anyURI">https://www.commoncoreontologies.org/InformationEntityOntology</cco:ont00001760>
  </rdf:Description>
  <rdf:Description rdf:about="https://www.commoncoreontologies.org/ont00000469">
    <rdf:type rdf:resource="http://www.w3.org/2002/07/owl#Class"/>
    <rdfs:subClassOf rdf:resource="https://www.commoncoreontologies.org/ont00000275"/>
    <rdfs:label xml:lang="en">Geospatial Coordinate Reference System</rdfs:label>
    <skos:altLabel xml:lang="en">Geographic Coordinate System</skos:altLabel>
    <skos:definition xml:lang="en">A Spatial Reference System that is used to determine and identify the location of a point or object at or near the surface of the Earth.</skos:definition>
    <cco:ont00001760 rdf:datatype="http://www.w3.org/2001/XMLSchema#anyURI">https://www.commoncoreontologies.org/InformationEntityOntology</cco:ont00001760>
  </rdf:Description>
  <rdf:Description rdf:about="https://www.commoncoreontologies.org/ont00001702">
    <rdf:type rdf:resource="http://www.w3.org/2002/07/owl#NamedIndividual"/>
    <rdf:type rdf:resource="https://www.commoncoreontologies.org/ont00001352"/>
    <rdfs:label xml:lang="en">GMT+5:30</rdfs:label>
    <skos:altLabel xml:lang="en">Indian Standard Time</skos:altLabel>
    <skos:altLabel xml:lang="en">Sri Lanka Standard Time</skos:altLabel>
    <cco:ont00001753>IST</cco:ont00001753>
    <cco:ont00001753>SLST</cco:ont00001753>
    <cco:ont00001760 rdf:datatype="http://www.w3.org/2001/XMLSchema#anyURI">https://www.commoncoreontologies.org/InformationEntityOntology</cco:ont00001760>
  </rdf:Description>
  <rdf:Description rdf:about="https://www.commoncoreontologies.org/ont00002033">
    <rdf:type rdf:resource="http://www.w3.org/2002/07/owl#Class"/>
    <rdfs:subClassOf rdf:resource="https://www.commoncoreontologies.org/ont00002020"/>
    <rdfs:label xml:lang="en">Code 128 Barcode</rdfs:label>
    <skos:definition xml:lang="en">A One-Dimensional Barcode that represents to 128 ASCII characters and is used primarily in supply chains.</skos:definition>
    <cco:ont00001760 rdf:datatype="http://www.w3.org/2001/XMLSchema#anyURI">https://www.commoncoreontologies.org/InformationEntityOntology</cco:ont00001760>
  </rdf:Description>
  <rdf:Description rdf:about="https://www.commoncoreontologies.org/ont00001467">
    <rdf:type rdf:resource="http://www.w3.org/2002/07/owl#NamedIndividual"/>
    <rdf:type rdf:resource="https://www.commoncoreontologies.org/ont00001352"/>
    <rdfs:label xml:lang="en">GMT-4</rdfs:label>
    <skos:altLabel xml:lang="en">PRT</skos:altLabel>
    <skos:altLabel xml:lang="en">Puerto Rico and US Virgin Islands Time</skos:altLabel>
    <cco:ont00001760 rdf:datatype="http://www.w3.org/2001/XMLSchema#anyURI">https://www.commoncoreontologies.org/InformationEntityOntology</cco:ont00001760>
  </rdf:Description>
  <rdf:Description rdf:about="https://www.commoncoreontologies.org/ont00001648">
    <rdf:type rdf:resource="http://www.w3.org/2002/07/owl#NamedIndividual"/>
    <rdf:type rdf:resource="https://www.commoncoreontologies.org/ont00000469"/>
    <rdf:type rdf:resource="https://www.commoncoreontologies.org/ont00001351"/>
    <rdfs:label xml:lang="en">Earth-Centered Earth-Fixed Coordinate System</rdfs:label>
    <skos:altLabel xml:lang="en">Conventional Terrestrial Coordinate System</skos:altLabel>
    <skos:altLabel xml:lang="en">ECEF</skos:altLabel>
    <skos:altLabel xml:lang="en">ECR</skos:altLabel>
    <skos:altLabel xml:lang="en">Earth Centered Earth Fixed</skos:altLabel>
    <skos:altLabel xml:lang="en">Earth Centered Rotational Coordinate System</skos:altLabel>
    <skos:altLabel xml:lang="en">Earth-Centered Earth-Fixed</skos:altLabel>
    <skos:altLabel xml:lang="en">Earth-Centered, Earth-Fixed</skos:altLabel>
    <skos:definition xml:lang="en">A Geospatial and Cartesian Coordinate System that identifies positions using an x-axis, y-axis, and z-axis coordinate where the zero point is the center of the Earth, the z-Axis extends toward the North Pole but does not always coincide exactly with the Earth's Axis of Rotation, the x-Axis extends through the intersection of the Prime Meridian and the Equator, the y-Axis completes the right-handed system, and all three axes are fixed to the Earth such that they rotate along with the Earth.</skos:definition>
    <cco:ont00001754 rdf:datatype="http://www.w3.org/2001/XMLSchema#anyURI">https://en.wikipedia.org/w/index.php?title=Earth-centered,_Earth-fixed_coordinate_system&amp;oldid=1062678600</cco:ont00001754>
    <cco:ont00001760 rdf:datatype="http://www.w3.org/2001/XMLSchema#anyURI">https://www.commoncoreontologies.org/InformationEntityOntology</cco:ont00001760>
  </rdf:Description>
  <rdf:Description rdf:about="https://www.commoncoreontologies.org/ont00002032">
    <rdf:type rdf:resource="http://www.w3.org/2002/07/owl#Class"/>
    <rdfs:subClassOf rdf:resource="https://www.commoncoreontologies.org/ont00002020"/>
    <rdfs:label xml:lang="en">Code 39 Barcode</rdfs:label>
    <skos:definition xml:lang="en">A One-Dimensional Barcode that represents 39 characters that are numbers 0-9, capital letters A-Z, or the symbols -.$/+% and space and is used primarily in automotive and defense industries.</skos:definition>
    <cco:ont00001760 rdf:datatype="http://www.w3.org/2001/XMLSchema#anyURI">https://www.commoncoreontologies.org/InformationEntityOntology</cco:ont00001760>
  </rdf:Description>
  <rdf:Description rdf:about="https://www.commoncoreontologies.org/ont00001976">
    <rdf:type rdf:resource="http://www.w3.org/2002/07/owl#ObjectProperty"/>
    <rdfs:subPropertyOf rdf:resource="https://www.commoncoreontologies.org/ont00001920"/>
    <rdfs:domain rdf:resource="https://www.commoncoreontologies.org/ont00000253"/>
    <rdfs:range rdf:resource="https://www.commoncoreontologies.org/ont00001175"/>
    <rdfs:label xml:lang="en">uses language</rdfs:label>
    <skos:definition xml:lang="en">x uses_language y iff x is an instance of an Information Bearing Entity and y is an instance of a Language such that the literal value of x is a string that is encoded according to the syntax of y.</skos:definition>
    <cco:ont00001760 rdf:datatype="http://www.w3.org/2001/XMLSchema#anyURI">https://www.commoncoreontologies.org/InformationEntityOntology</cco:ont00001760>
  </rdf:Description>
  <rdf:Description rdf:about="https://www.commoncoreontologies.org/ont00001942">
    <rdf:type rdf:resource="http://www.w3.org/2002/07/owl#ObjectProperty"/>
    <rdfs:subPropertyOf rdf:resource="https://www.commoncoreontologies.org/ont00001808"/>
    <rdfs:domain rdf:resource="https://www.commoncoreontologies.org/ont00000965"/>
    <rdfs:range rdf:resource="http://purl.obolibrary.org/obo/BFO_0000001"/>
    <rdfs:label xml:lang="en">prescribes</rdfs:label>
    <skos:definition xml:lang="en">x prescribes y iff x is an instance of Information Content Entity and y is an instance of Entity, such that x serves as a rule or guide for y if y an Occurrent, or x serves as a model for y if y is a Continuant.</skos:definition>
    <skos:example>A blueprint prescribes some artifact or facility by being a model for it.</skos:example>
    <skos:example>A professional code of conduct prescribes some realizations of a profession (role) by giving rules for how the bearer should act in those realizations.</skos:example>
    <skos:example>An operations plan prescribes an operation by enumerating the tasks that need to be performed in order to achieve the objectives of the operation.</skos:example>
    <cco:ont00001760 rdf:datatype="http://www.w3.org/2001/XMLSchema#anyURI">https://www.commoncoreontologies.org/InformationEntityOntology</cco:ont00001760>
  </rdf:Description>
  <rdf:Description rdf:about="https://www.commoncoreontologies.org/ont00001599">
    <rdf:type rdf:resource="http://www.w3.org/2002/07/owl#NamedIndividual"/>
    <rdf:type rdf:resource="https://www.commoncoreontologies.org/ont00001352"/>
    <rdfs:label xml:lang="en">GMT+3:30</rdfs:label>
    <skos:altLabel xml:lang="en">Iran Standard Time</skos:altLabel>
    <skos:altLabel xml:lang="en">Iran Time</skos:altLabel>
    <cco:ont00001753>IRST</cco:ont00001753>
    <cco:ont00001753>IT</cco:ont00001753>
    <cco:ont00001760 rdf:datatype="http://www.w3.org/2001/XMLSchema#anyURI">https://www.commoncoreontologies.org/InformationEntityOntology</cco:ont00001760>
  </rdf:Description>
  <rdf:Description rdf:about="https://www.commoncoreontologies.org/ont00001765">
    <rdf:type rdf:resource="http://www.w3.org/2002/07/owl#DatatypeProperty"/>
    <rdfs:domain rdf:resource="https://www.commoncoreontologies.org/ont00000253"/>
    <rdfs:label xml:lang="en">has text value</rdfs:label>
    <skos:definition xml:lang="en">A data property that has as its range a string value.</skos:definition>
    <cco:ont00001760 rdf:datatype="http://www.w3.org/2001/XMLSchema#anyURI">https://www.commoncoreontologies.org/InformationEntityOntology</cco:ont00001760>
  </rdf:Description>
  <rdf:Description rdf:about="https://www.commoncoreontologies.org/ont00001430">
    <rdf:type rdf:resource="http://www.w3.org/2002/07/owl#NamedIndividual"/>
    <rdf:type rdf:resource="https://www.commoncoreontologies.org/ont00001235"/>
    <rdfs:comment xml:lang="en">Offset from Universal Coordinated Time = UTC+6</rdfs:comment>
    <rdfs:label xml:lang="en">Foxtrot Time Zone</rdfs:label>
    <cco:ont00001753>F</cco:ont00001753>
    <cco:ont00001760 rdf:datatype="http://www.w3.org/2001/XMLSchema#anyURI">https://www.commoncoreontologies.org/InformationEntityOntology</cco:ont00001760>
  </rdf:Description>
  <rdf:Description rdf:nodeID="na8580e9876f64da8bd2fccebf064ee6cb3">
    <rdf:first rdf:resource="http://purl.obolibrary.org/obo/BFO_0000178"/>
    <rdf:rest rdf:nodeID="na8580e9876f64da8bd2fccebf064ee6cb4"/>
  </rdf:Description>
  <rdf:Description rdf:about="https://www.commoncoreontologies.org/ont00001879">
    <rdf:type rdf:resource="http://www.w3.org/2002/07/owl#ObjectProperty"/>
    <rdfs:subPropertyOf rdf:resource="https://www.commoncoreontologies.org/ont00001801"/>
    <owl:inverseOf rdf:resource="https://www.commoncoreontologies.org/ont00001916"/>
    <rdfs:domain rdf:resource="http://purl.obolibrary.org/obo/BFO_0000001"/>
    <rdfs:range rdf:resource="https://www.commoncoreontologies.org/ont00000686"/>
    <rdfs:label xml:lang="en">designated by</rdfs:label>
    <skos:definition xml:lang="en">x designated_by y iff y is an instance of Designative Information Content Entity and x is an instance of Entity and y designates x.</skos:definition>
    <cco:ont00001760 rdf:datatype="http://www.w3.org/2001/XMLSchema#anyURI">https://www.commoncoreontologies.org/InformationEntityOntology</cco:ont00001760>
  </rdf:Description>
  <rdf:Description rdf:about="https://www.commoncoreontologies.org/ont00000626">
    <rdf:type rdf:resource="http://www.w3.org/2002/07/owl#Class"/>
    <rdfs:subClassOf rdf:resource="https://www.commoncoreontologies.org/ont00000853"/>
    <rdfs:comment xml:lang="en">Since predictions are inherently about not-yet-existant things, the Modal Relation Ontology term 'describes' (i.e. mro:describes) should be used (instead of the standard cco:describes) to relate instances of Predictive Information Content Entity to the entities they are about.</rdfs:comment>
    <rdfs:label xml:lang="en">Predictive Information Content Entity</rdfs:label>
    <skos:altLabel xml:lang="en">Prediction</skos:altLabel>
    <skos:altLabel xml:lang="en">Prediction Information Content Entity</skos:altLabel>
    <skos:definition xml:lang="en">A Descriptive Information Content Entity that describes an uncertain future event.</skos:definition>
    <cco:ont00001760 rdf:datatype="http://www.w3.org/2001/XMLSchema#anyURI">https://www.commoncoreontologies.org/InformationEntityOntology</cco:ont00001760>
  </rdf:Description>
  <rdf:Description rdf:about="https://www.commoncoreontologies.org/ont00001590">
    <rdf:type rdf:resource="http://www.w3.org/2002/07/owl#NamedIndividual"/>
    <rdf:type rdf:resource="https://www.commoncoreontologies.org/ont00001328"/>
    <rdfs:comment xml:lang="en">TAI is a time standard the values of which are generated by calculating the weighted average of the measurements of more than 400 atomic clocks and is based on the International System of Units (SI) definition of one second equals the time it takes a Cesium-133 atom at the ground state to oscillate exactly 9,192,631,770 times. TAI is extremely precise, but does not perfectly synchronize with Earth times, which is why TAI and UT1 are both used to determine UTC. TAI serves as the main realization of TT.</rdfs:comment>
    <rdfs:label xml:lang="en">International Atomic Time</rdfs:label>
    <cco:ont00001753>TAI</cco:ont00001753>
    <cco:ont00001760 rdf:datatype="http://www.w3.org/2001/XMLSchema#anyURI">https://www.commoncoreontologies.org/InformationEntityOntology</cco:ont00001760>
  </rdf:Description>
  <rdf:Description rdf:about="https://www.commoncoreontologies.org/ont00001716">
    <rdf:type rdf:resource="http://www.w3.org/2002/07/owl#NamedIndividual"/>
    <rdf:type rdf:resource="https://www.commoncoreontologies.org/ont00000630"/>
    <rdfs:comment xml:lang="en">UT1 is a derivation of UT0 that takes into account distortions caused by polar motion and is proportional to the rotation angle of the Earth with respect to distant quasars, specifically, the International Celestial Reference Frame (ICRF). UT1 is currently the most widely used variant of Universal Time and has the same value everywhere on Earth.</rdfs:comment>
    <rdfs:label xml:lang="en">Universal Time 1</rdfs:label>
    <skos:altLabel xml:lang="en">Astronomical Time</skos:altLabel>
    <cco:ont00001753>UT1</cco:ont00001753>
    <cco:ont00001760 rdf:datatype="http://www.w3.org/2001/XMLSchema#anyURI">https://www.commoncoreontologies.org/InformationEntityOntology</cco:ont00001760>
  </rdf:Description>
  <rdf:Description rdf:about="https://www.commoncoreontologies.org/ont00000735">
    <rdf:type rdf:resource="http://www.w3.org/2002/07/owl#Class"/>
    <rdfs:subClassOf rdf:resource="https://www.commoncoreontologies.org/ont00000406"/>
    <rdfs:label xml:lang="en">Geospatial Region Bounding Box Identifier List</rdfs:label>
    <skos:definition xml:lang="en">A Measurement Unit of Geocoordinate that is comprised of 4 pairs of coordinates, one for each of the 4 defining points (North, West, South, East) of a Geospatial Region Bounding Box.</skos:definition>
    <cco:ont00001760 rdf:datatype="http://www.w3.org/2001/XMLSchema#anyURI">https://www.commoncoreontologies.org/InformationEntityOntology</cco:ont00001760>
  </rdf:Description>
  <rdf:Description rdf:about="https://www.commoncoreontologies.org/ont00000067">
    <rdf:type rdf:resource="http://www.w3.org/2002/07/owl#Class"/>
    <rdfs:subClassOf rdf:resource="https://www.commoncoreontologies.org/ont00001328"/>
    <rdfs:comment xml:lang="en">In traditional astronomical usage, civil time is mean solar time as calculated from midnight as the beginning of the Civil Day.</rdfs:comment>
    <rdfs:comment xml:lang="en">Note that Civil Time Reference System is more accurately represented as a Temporal Reference System that participates in an act of usage that is sanctioned by an appropriate civil authority. As such, it should be represented as a defined class.</rdfs:comment>
    <rdfs:label xml:lang="en">Civil Time Reference System</rdfs:label>
    <skos:definition xml:lang="en">A Temporal Reference System that is a statutory time scale as designated by civilian authorities to determine local time(s).</skos:definition>
    <cco:ont00001760 rdf:datatype="http://www.w3.org/2001/XMLSchema#anyURI">https://www.commoncoreontologies.org/InformationEntityOntology</cco:ont00001760>
  </rdf:Description>
  <rdf:Description rdf:about="https://www.commoncoreontologies.org/ont00001403">
    <rdf:type rdf:resource="http://www.w3.org/2002/07/owl#NamedIndividual"/>
    <rdf:type rdf:resource="https://www.commoncoreontologies.org/ont00001235"/>
    <rdfs:comment xml:lang="en">Offset from Universal Coordinated Time = UTC+2</rdfs:comment>
    <rdfs:label xml:lang="en">Bravo Time Zone</rdfs:label>
    <cco:ont00001753>B</cco:ont00001753>
    <cco:ont00001760 rdf:datatype="http://www.w3.org/2001/XMLSchema#anyURI">https://www.commoncoreontologies.org/InformationEntityOntology</cco:ont00001760>
  </rdf:Description>
  <rdf:Description rdf:about="https://www.commoncoreontologies.org/ont00001863">
    <rdf:type rdf:resource="http://www.w3.org/2002/07/owl#ObjectProperty"/>
    <rdfs:subPropertyOf rdf:resource="http://purl.obolibrary.org/obo/BFO_0000101"/>
    <owl:inverseOf rdf:resource="https://www.commoncoreontologies.org/ont00001961"/>
    <rdfs:domain rdf:resource="https://www.commoncoreontologies.org/ont00000253"/>
    <rdfs:range rdf:resource="https://www.commoncoreontologies.org/ont00000120"/>
    <rdfs:label xml:lang="en">uses measurement unit</rdfs:label>
    <skos:definition xml:lang="en">y uses_measurement_unit x iff y is an instance of Information Bearing Entity and x is an instance of Measurement Unit, such that x describes the magnitude of measured physical quantity mentioned in y.</skos:definition>
    <cco:ont00001760 rdf:datatype="http://www.w3.org/2001/XMLSchema#anyURI">https://www.commoncoreontologies.org/InformationEntityOntology</cco:ont00001760>
  </rdf:Description>
  <rdf:Description rdf:about="https://www.commoncoreontologies.org/ont00001439">
    <rdf:type rdf:resource="http://www.w3.org/2002/07/owl#NamedIndividual"/>
    <rdf:type rdf:resource="https://www.commoncoreontologies.org/ont00000263"/>
    <rdfs:label xml:lang="en">Twenty-Four-Hour Clock Time System</rdfs:label>
    <skos:altLabel xml:lang="en">24-Hour Clock</skos:altLabel>
    <skos:altLabel xml:lang="en">24-Hour Clock Time System</skos:altLabel>
    <skos:altLabel xml:lang="en">Military Time</skos:altLabel>
    <skos:altLabel xml:lang="en">Military Time System</skos:altLabel>
    <skos:altLabel xml:lang="en">Twenty-Four Hour Clock Time System</skos:altLabel>
    <skos:altLabel xml:lang="en">Twenty-Four-Hour Clock</skos:altLabel>
    <skos:definition xml:lang="en">A Clock Time System for time keeping in which the Day runs from midnight to midnight and is divided into 24 Hours, indicated by the Hours passed since midnight, from 0 to 23.</skos:definition>
    <cco:ont00001754 rdf:datatype="http://www.w3.org/2001/XMLSchema#anyURI">https://en.wikipedia.org/w/index.php?title=24-hour_clock&amp;oldid=1063744105</cco:ont00001754>
    <cco:ont00001760 rdf:datatype="http://www.w3.org/2001/XMLSchema#anyURI">https://www.commoncoreontologies.org/InformationEntityOntology</cco:ont00001760>
  </rdf:Description>
  <rdf:Description rdf:about="https://www.commoncoreontologies.org/ont00001695">
    <rdf:type rdf:resource="http://www.w3.org/2002/07/owl#NamedIndividual"/>
    <rdf:type rdf:resource="https://www.commoncoreontologies.org/ont00000630"/>
    <rdfs:comment xml:lang="en">UT2 is a variant of Universal Time that smooths UT1 by accounting for both polar motion and variations in Earth's rotation due to seasonal factors, such as changes in vegetation and water or snow distribution.</rdfs:comment>
    <rdfs:label xml:lang="en">Universal Time 2</rdfs:label>
    <cco:ont00001753>UT2</cco:ont00001753>
    <cco:ont00001760 rdf:datatype="http://www.w3.org/2001/XMLSchema#anyURI">https://www.commoncoreontologies.org/InformationEntityOntology</cco:ont00001760>
  </rdf:Description>
  <rdf:Description rdf:about="https://www.commoncoreontologies.org/ont00000829">
    <rdf:type rdf:resource="http://www.w3.org/2002/07/owl#Class"/>
    <rdfs:subClassOf rdf:resource="https://www.commoncoreontologies.org/ont00000390"/>
    <rdfs:comment xml:lang="en">Standards of date, time, and time zone data formats:
ISO/WD 8601-2 (http://www.loc.gov/standards/datetime/iso-tc154-wg5_n0039_iso_wd_8601-2_2016-02-16.pdf)
W3C (https://www.w3.org/TR/NOTE-datetime)</rdfs:comment>
    <rdfs:comment xml:lang="en">There is no class 'Time Zone' (the region), only 'Time Zone Identifier' (the designator for some region). Instances of 'Time Zone Identifier' should be related to instances of 'Information Bearing Entity' by means of the object properites 'uses time zone identifier' and 'time zone identifier used by' as appropriate. This is supposed to be analogous to the way we represent the relationship between measurement values and measurement units, where the relevant instance of Information Bearing Entity 'uses measurement unit' some instance of Measurement Unit (i.e., an instance of Information Content Entity).</rdfs:comment>
    <rdfs:label xml:lang="en">Time Zone Identifier</rdfs:label>
    <skos:definition xml:lang="en">A Spatial Region Identifier that designates the region associated with some uniform standard time for legal, commercial, or social purposes.</skos:definition>
    <cco:ont00001760 rdf:datatype="http://www.w3.org/2001/XMLSchema#anyURI">https://www.commoncoreontologies.org/InformationEntityOntology</cco:ont00001760>
  </rdf:Description>
  <rdf:Description rdf:about="https://www.commoncoreontologies.org/ont00000029">
    <rdf:type rdf:resource="http://www.w3.org/2002/07/owl#Class"/>
    <rdfs:subClassOf rdf:resource="https://www.commoncoreontologies.org/ont00000745"/>
    <rdfs:label xml:lang="en">Median Point Estimate Information Content Entity</rdfs:label>
    <skos:altLabel xml:lang="en">Median</skos:altLabel>
    <skos:definition xml:lang="en">A Point Estimate Information Content Entity that is a measurement of a set of values and is equal to either the middle value or the average of the two values which separate the set into two equally populated upper and lower sets.</skos:definition>
    <cco:ont00001760 rdf:datatype="http://www.w3.org/2001/XMLSchema#anyURI">https://www.commoncoreontologies.org/InformationEntityOntology</cco:ont00001760>
  </rdf:Description>
  <rdf:Description rdf:about="https://www.commoncoreontologies.org/ont00001405">
    <rdf:type rdf:resource="http://www.w3.org/2002/07/owl#NamedIndividual"/>
    <rdf:type rdf:resource="https://www.commoncoreontologies.org/ont00001352"/>
    <rdfs:label xml:lang="en">GMT-2</rdfs:label>
    <skos:altLabel xml:lang="en">BET</skos:altLabel>
    <skos:altLabel xml:lang="en">Brazil Eastern Time</skos:altLabel>
    <cco:ont00001760 rdf:datatype="http://www.w3.org/2001/XMLSchema#anyURI">https://www.commoncoreontologies.org/InformationEntityOntology</cco:ont00001760>
  </rdf:Description>
  <rdf:Description rdf:about="https://www.commoncoreontologies.org/ont00000399">
    <rdf:type rdf:resource="http://www.w3.org/2002/07/owl#Class"/>
    <owl:equivalentClass rdf:nodeID="na8580e9876f64da8bd2fccebf064ee6cb23"/>
    <rdfs:subClassOf rdf:resource="https://www.commoncoreontologies.org/ont00000686"/>
    <rdfs:label xml:lang="en">Temporal Region Identifier</rdfs:label>
    <skos:definition xml:lang="en">A Designative Information Content Entity that designates some Temporal Region.</skos:definition>
    <cco:ont00001760 rdf:datatype="http://www.w3.org/2001/XMLSchema#anyURI">https://www.commoncoreontologies.org/InformationEntityOntology</cco:ont00001760>
  </rdf:Description>
  <rdf:Description rdf:about="https://www.commoncoreontologies.org/ont00001919">
    <rdf:type rdf:resource="http://www.w3.org/2002/07/owl#ObjectProperty"/>
    <rdfs:domain rdf:resource="http://purl.obolibrary.org/obo/BFO_0000001"/>
    <rdfs:range rdf:resource="https://www.commoncoreontologies.org/ont00000253"/>
    <rdfs:label xml:lang="en">is mentioned by</rdfs:label>
    <skos:definition xml:lang="en">x is_mentioned_by y iff y is an instance of Information Bearing Entity and x is an instance of Entity, such that y is used as a reference to x.</skos:definition>
    <cco:ont00001760 rdf:datatype="http://www.w3.org/2001/XMLSchema#anyURI">https://www.commoncoreontologies.org/InformationEntityOntology</cco:ont00001760>
  </rdf:Description>
  <rdf:Description rdf:about="https://www.commoncoreontologies.org/ont00002034">
    <rdf:type rdf:resource="http://www.w3.org/2002/07/owl#Class"/>
    <rdfs:subClassOf rdf:resource="https://www.commoncoreontologies.org/ont00002020"/>
    <rdfs:label xml:lang="en">UPC Barcode</rdfs:label>
    <skos:definition xml:lang="en">A One-Dimensional Barcode that represents 6 or 12 numerical digits and is used to scan consumer goods.</skos:definition>
    <cco:ont00001760 rdf:datatype="http://www.w3.org/2001/XMLSchema#anyURI">https://www.commoncoreontologies.org/InformationEntityOntology</cco:ont00001760>
  </rdf:Description>
  <rdf:Description rdf:about="https://www.commoncoreontologies.org/ont00000923">
    <rdf:type rdf:resource="http://www.w3.org/2002/07/owl#Class"/>
    <rdfs:subClassOf rdf:resource="https://www.commoncoreontologies.org/ont00000649"/>
    <rdfs:label xml:lang="en">Arbitrary Identifier</rdfs:label>
    <skos:altLabel xml:lang="en">Arbitrary ID</skos:altLabel>
    <skos:definition xml:lang="en">A Non-Name Identifier that consists of a string of characters that does not follow an encoding system.</skos:definition>
    <cco:ont00001760 rdf:datatype="http://www.w3.org/2001/XMLSchema#anyURI">https://www.commoncoreontologies.org/InformationEntityOntology</cco:ont00001760>
  </rdf:Description>
  <rdf:Description rdf:about="https://www.commoncoreontologies.org/ont00001801">
    <rdf:type rdf:resource="http://www.w3.org/2002/07/owl#ObjectProperty"/>
    <owl:inverseOf rdf:resource="https://www.commoncoreontologies.org/ont00001808"/>
    <rdfs:domain rdf:resource="http://purl.obolibrary.org/obo/BFO_0000001"/>
    <rdfs:range rdf:resource="https://www.commoncoreontologies.org/ont00000958"/>
    <rdfs:label xml:lang="en">is subject of</rdfs:label>
    <skos:definition xml:lang="en">x is_subject_of y iff x is an instance of Entity and y is an instance of Information Content Entity and y is_about x.</skos:definition>
    <cco:ont00001760 rdf:datatype="http://www.w3.org/2001/XMLSchema#anyURI">https://www.commoncoreontologies.org/InformationEntityOntology</cco:ont00001760>
  </rdf:Description>
  <rdf:Description rdf:nodeID="na8580e9876f64da8bd2fccebf064ee6cb21">
    <rdf:first rdf:resource="https://www.commoncoreontologies.org/ont00000686"/>
    <rdf:rest rdf:nodeID="na8580e9876f64da8bd2fccebf064ee6cb22"/>
  </rdf:Description>
  <rdf:Description rdf:about="https://www.commoncoreontologies.org/ont00001163">
    <rdf:type rdf:resource="http://www.w3.org/2002/07/owl#Class"/>
    <owl:equivalentClass rdf:nodeID="na8580e9876f64da8bd2fccebf064ee6cb71"/>
    <rdfs:subClassOf rdf:resource="https://www.commoncoreontologies.org/ont00000853"/>
    <rdfs:label xml:lang="en">Measurement Information Content Entity</rdfs:label>
    <skos:altLabel xml:lang="en">Measurement ICE</skos:altLabel>
    <skos:definition xml:lang="en">A Descriptive Information Content Entity that describes the extent, dimensions, quantity, or quality of an Entity relative to some standard.</skos:definition>
    <cco:ont00001760 rdf:datatype="http://www.w3.org/2001/XMLSchema#anyURI">https://www.commoncoreontologies.org/InformationEntityOntology</cco:ont00001760>
  </rdf:Description>
  <rdf:Description rdf:about="https://www.commoncoreontologies.org/ont00000253">
    <rdf:type rdf:resource="http://www.w3.org/2002/07/owl#Class"/>
    <owl:equivalentClass rdf:nodeID="na8580e9876f64da8bd2fccebf064ee6cb10"/>
    <rdfs:subClassOf rdf:resource="http://purl.obolibrary.org/obo/BFO_0000030"/>
    <rdfs:comment xml:lang="en">This class continues to use the word bearing in its rdfslabel because of potential confusion with the acronym ICE, which is widely used for information content entity.</rdfs:comment>
    <rdfs:label xml:lang="en">Information Bearing Entity</rdfs:label>
    <skos:altLabel xml:lang="en">IBE</skos:altLabel>
    <skos:altLabel xml:lang="en">Information Carrying Entity</skos:altLabel>
    <skos:definition xml:lang="en">An Object upon which an Information Content Entity generically depends.</skos:definition>
    <cco:ont00001754 rdf:datatype="http://www.w3.org/2001/XMLSchema#anyURI">http://purl.obolibrary.org/obo/IAO_0000178</cco:ont00001754>
    <cco:ont00001760 rdf:datatype="http://www.w3.org/2001/XMLSchema#anyURI">https://www.commoncoreontologies.org/InformationEntityOntology</cco:ont00001760>
  </rdf:Description>
  <rdf:Description rdf:nodeID="na8580e9876f64da8bd2fccebf064ee6cb76">
    <rdf:type rdf:resource="http://www.w3.org/2002/07/owl#Restriction"/>
    <owl:onProperty rdf:resource="https://www.commoncoreontologies.org/ont00001877"/>
    <owl:someValuesFrom rdf:resource="http://purl.obolibrary.org/obo/BFO_0000001"/>
  </rdf:Description>
  <rdf:Description rdf:about="https://www.commoncoreontologies.org/ont00002005">
    <rdf:type rdf:resource="http://www.w3.org/2002/07/owl#Class"/>
    <rdfs:subClassOf rdf:resource="https://www.commoncoreontologies.org/ont00002004"/>
    <rdfs:label xml:lang="en">Chart</rdfs:label>
    <skos:definition xml:lang="en">An Image that is prescribed by some canonical visual format.</skos:definition>
    <cco:ont00001754>Adapted from Chart. Merriam-Webster.com Dictionary, Merriam-Webster, https://www.merriam-webster.com/dictionary/chart. Accessed 4 Aug. 2024.</cco:ont00001754>
    <cco:ont00001760 rdf:datatype="http://www.w3.org/2001/XMLSchema#anyURI">https://www.commoncoreontologies.org/InformationEntityOntology</cco:ont00001760>
  </rdf:Description>
  <rdf:Description rdf:about="https://www.commoncoreontologies.org/ont00002022">
    <rdf:type rdf:resource="http://www.w3.org/2002/07/owl#Class"/>
    <rdfs:subClassOf rdf:resource="https://www.commoncoreontologies.org/ont00002020"/>
    <rdfs:label xml:lang="en">Code 93 Barcode</rdfs:label>
    <skos:definition xml:lang="en">A One-Dimensional Barcode that represents 93 ASCII characters and is used in logistics to identify packages in retail inventory, lable electornic components, and provide supplementary delivery information.</skos:definition>
    <cco:ont00001760 rdf:datatype="http://www.w3.org/2001/XMLSchema#anyURI">https://www.commoncoreontologies.org/InformationEntityOntology</cco:ont00001760>
  </rdf:Description>
  <rdf:Description rdf:about="https://www.commoncoreontologies.org/ont00000958">
    <rdf:type rdf:resource="http://www.w3.org/2002/07/owl#Class"/>
    <owl:equivalentClass rdf:nodeID="na8580e9876f64da8bd2fccebf064ee6cb51"/>
    <rdfs:subClassOf rdf:resource="http://purl.obolibrary.org/obo/BFO_0000031"/>
    <rdfs:label xml:lang="en">Information Content Entity</rdfs:label>
    <skos:altLabel xml:lang="en">ICE</skos:altLabel>
    <skos:definition xml:lang="en">A Generically Dependent Continuant that generically depends on some Information Bearing Entity and stands in relation of aboutness to some Entity.</skos:definition>
    <skos:scopeNote xml:lang="en">Information Content Entity is here intended to be a class of Entities whose instances are the informational content of Information Bearing Entities. For example, three instances of information bearers -- such as a bar chart, color-coded map, and a written report -- each of which lists the GDP of Countries for the year 2010 are each different carriers of the same information content. It is this content that is generically dependent upon its carrier. This treatment of Informational Content Entity (cf. the Information Artifact Ontology) leads to a principle of subtyping based upon the relationship that ICE's have with the Entity they are about rather than characteristics such as format, language, measurement scale, or media. The latter are treated here as being Qualities of bearers.</skos:scopeNote>
    <cco:ont00001754>http://purl.obolibrary.org/obo/IAO_0000030</cco:ont00001754>
    <cco:ont00001760 rdf:datatype="http://www.w3.org/2001/XMLSchema#anyURI">https://www.commoncoreontologies.org/InformationEntityOntology</cco:ont00001760>
  </rdf:Description>
  <rdf:Description rdf:about="https://www.commoncoreontologies.org/ont00000146">
    <rdf:type rdf:resource="http://www.w3.org/2002/07/owl#Class"/>
    <rdfs:subClassOf rdf:resource="https://www.commoncoreontologies.org/ont00001175"/>
    <owl:disjointWith rdf:resource="https://www.commoncoreontologies.org/ont00000496"/>
    <rdfs:label xml:lang="en">Artificial Language</rdfs:label>
    <skos:definition xml:lang="en">A Language that is developed through conscious planning and premeditation, rather than one that was developed through use and repetition.</skos:definition>
    <skos:example>Esperanto</skos:example>
    <skos:example>Python Programming Language</skos:example>
    <cco:ont00001754 rdf:datatype="http://www.w3.org/2001/XMLSchema#anyURI">https://en.wikipedia.org/w/index.php?title=Constructed_language&amp;oldid=1062733589</cco:ont00001754>
    <cco:ont00001760 rdf:datatype="http://www.w3.org/2001/XMLSchema#anyURI">https://www.commoncoreontologies.org/InformationEntityOntology</cco:ont00001760>
  </rdf:Description>
  <rdf:Description rdf:about="https://www.commoncoreontologies.org/ont00001660">
    <rdf:type rdf:resource="http://www.w3.org/2002/07/owl#NamedIndividual"/>
    <rdf:type rdf:resource="https://www.commoncoreontologies.org/ont00000469"/>
    <rdfs:comment xml:lang="en">This global main field model provides magnetic field values for any location on Earth, e.g. for  navigational purposes (declination) or as a standard for core field subtraction for aeromagnetic surveys. An updated version is adopted by International Association of Geomagnetism and Aeronomy (IAGA) every 5 years).</rdfs:comment>
    <rdfs:label xml:lang="en">International Geomagnetic Reference Field</rdfs:label>
    <cco:ont00001754>Alken, P., Thbault, E., Beggan, C.D. et al. International Geomagnetic Reference Field: the thirteenth generation. Earth Planets Space 73, 49 (2021). https://doi.org/10.1186/s40623-020-01288-x , https://www.iaga-aiga.org/</cco:ont00001754>
  </rdf:Description>
  <rdf:Description rdf:about="https://www.commoncoreontologies.org/ont00001331">
    <rdf:type rdf:resource="http://www.w3.org/2002/07/owl#Class"/>
    <rdfs:subClassOf rdf:resource="https://www.commoncoreontologies.org/ont00001014"/>
    <rdfs:label xml:lang="en">Legal Name</rdfs:label>
    <skos:definition xml:lang="en">A Proper Name that is an official name for the designated entity as determined by a Government or court of law.</skos:definition>
    <cco:ont00001760 rdf:datatype="http://www.w3.org/2001/XMLSchema#anyURI">https://www.commoncoreontologies.org/InformationEntityOntology</cco:ont00001760>
  </rdf:Description>
  <rdf:Description rdf:about="https://www.commoncoreontologies.org/ont00001912">
    <rdf:type rdf:resource="http://www.w3.org/2002/07/owl#ObjectProperty"/>
    <rdfs:subPropertyOf rdf:resource="http://purl.obolibrary.org/obo/BFO_0000101"/>
    <owl:inverseOf rdf:resource="https://www.commoncoreontologies.org/ont00001997"/>
    <rdfs:domain rdf:resource="https://www.commoncoreontologies.org/ont00000253"/>
    <rdfs:range rdf:resource="https://www.commoncoreontologies.org/ont00000398"/>
    <rdfs:label xml:lang="en">uses reference system</rdfs:label>
    <skos:definition xml:lang="en">y uses_reference_system x iff y is an instance of Information Bearing Entity and x is an instance of Reference System, such that x describes the set of standards mentioned in y.</skos:definition>
    <cco:ont00001760 rdf:datatype="http://www.w3.org/2001/XMLSchema#anyURI">https://www.commoncoreontologies.org/InformationEntityOntology</cco:ont00001760>
  </rdf:Description>
  <rdf:Description rdf:about="https://www.commoncoreontologies.org/ont00000589">
    <rdf:type rdf:resource="http://www.w3.org/2002/07/owl#Class"/>
    <rdfs:subClassOf rdf:resource="https://www.commoncoreontologies.org/ont00000973"/>
    <rdfs:label xml:lang="en">Julian Date Fraction</rdfs:label>
    <skos:altLabel xml:lang="en">Julian Date Time Identifier</skos:altLabel>
    <skos:altLabel xml:lang="en">Julian Day Fraction</skos:altLabel>
    <skos:definition xml:lang="en">A Decimal Time of Day Identifier that designates an approximate Temporal Instant that is part of some Julian Day.</skos:definition>
    <cco:ont00001760 rdf:datatype="http://www.w3.org/2001/XMLSchema#anyURI">https://www.commoncoreontologies.org/InformationEntityOntology</cco:ont00001760>
  </rdf:Description>
  <rdf:Description rdf:about="https://www.commoncoreontologies.org/ont00001917">
    <rdf:type rdf:resource="http://www.w3.org/2002/07/owl#ObjectProperty"/>
    <rdfs:subPropertyOf rdf:resource="https://www.commoncoreontologies.org/ont00001801"/>
    <owl:inverseOf rdf:resource="https://www.commoncoreontologies.org/ont00001982"/>
    <rdfs:domain rdf:resource="http://purl.obolibrary.org/obo/BFO_0000001"/>
    <rdfs:range rdf:resource="https://www.commoncoreontologies.org/ont00000853"/>
    <rdfs:label xml:lang="en">described by</rdfs:label>
    <skos:definition xml:lang="en">x described_by y iff y is an instance of Descriptive Information Content Entity and x is an instance of Entity and y describes x.</skos:definition>
    <cco:ont00001760 rdf:datatype="http://www.w3.org/2001/XMLSchema#anyURI">https://www.commoncoreontologies.org/InformationEntityOntology</cco:ont00001760>
  </rdf:Description>
  <rdf:Description rdf:about="https://www.commoncoreontologies.org/ont00001176">
    <rdf:type rdf:resource="http://www.w3.org/2002/07/owl#Class"/>
    <rdfs:subClassOf rdf:resource="https://www.commoncoreontologies.org/ont00001163"/>
    <rdfs:label xml:lang="en">Estimate Information Content Entity</rdfs:label>
    <skos:altLabel xml:lang="en">Estimate</skos:altLabel>
    <skos:altLabel xml:lang="en">Estimate Measurement Information Content Entity</skos:altLabel>
    <skos:altLabel xml:lang="en">Estimated Value</skos:altLabel>
    <skos:definition xml:lang="en">A Measurement Information Content Entity that is a measurement of an entity based on partial information about that entity or an appropriately similar entity.</skos:definition>
    <cco:ont00001760 rdf:datatype="http://www.w3.org/2001/XMLSchema#anyURI">https://www.commoncoreontologies.org/InformationEntityOntology</cco:ont00001760>
  </rdf:Description>
  <rdf:Description rdf:about="https://www.commoncoreontologies.org/ont00001628">
    <rdf:type rdf:resource="http://www.w3.org/2002/07/owl#NamedIndividual"/>
    <rdf:type rdf:resource="https://www.commoncoreontologies.org/ont00001235"/>
    <rdfs:comment xml:lang="en">Offset from Universal Coordinated Time = UTC-12</rdfs:comment>
    <rdfs:comment xml:lang="en">Yankee Time Zone is the same local time as Mike Time Zone, but is 1 Day (i.e. 24 Hours) behind Mike Time Zone as they are on opposite sides of the International Date Line.</rdfs:comment>
    <rdfs:label xml:lang="en">Yankee Time Zone</rdfs:label>
    <cco:ont00001753>Y</cco:ont00001753>
    <cco:ont00001760 rdf:datatype="http://www.w3.org/2001/XMLSchema#anyURI">https://www.commoncoreontologies.org/InformationEntityOntology</cco:ont00001760>
  </rdf:Description>
  <rdf:Description rdf:about="https://www.commoncoreontologies.org/ont00001997">
    <rdf:type rdf:resource="http://www.w3.org/2002/07/owl#ObjectProperty"/>
    <rdfs:subPropertyOf rdf:resource="http://purl.obolibrary.org/obo/BFO_0000084"/>
    <rdfs:domain rdf:resource="https://www.commoncoreontologies.org/ont00000398"/>
    <rdfs:range rdf:resource="https://www.commoncoreontologies.org/ont00000253"/>
    <rdfs:label xml:lang="en">is reference system of</rdfs:label>
    <skos:definition xml:lang="en">x is_reference_system_of y iff y is an instance of Information Bearing Entity and x is an instance of Reference System, such that x describes the set of standards mentioned in y.</skos:definition>
    <cco:ont00001760 rdf:datatype="http://www.w3.org/2001/XMLSchema#anyURI">https://www.commoncoreontologies.org/InformationEntityOntology</cco:ont00001760>
  </rdf:Description>
  <rdf:Description rdf:about="https://www.commoncoreontologies.org/ont00001824">
    <rdf:type rdf:resource="http://www.w3.org/2002/07/owl#ObjectProperty"/>
    <rdfs:domain rdf:resource="https://www.commoncoreontologies.org/ont00000253"/>
    <rdfs:range rdf:resource="https://www.commoncoreontologies.org/ont00000253"/>
    <rdfs:label xml:lang="en">is excerpted from</rdfs:label>
    <skos:definition xml:lang="en">An Information Bearing Entity b1 is excerpted from another Information Bearing Entity B2 iff b1 is part of some Information Bearing Entity B1 that is carrier of some Information Content Entity C1, B2 is carrier of some Information Content Entity C2, C1 is not identical with C2, b1 is carrier of some Information Content Entity c1, b2 is an Information Bearing Entity that is part of B2 and b2 is carrier of c1 (i.e. the same Information Content Entity as borne by b1).</skos:definition>
    <cco:ont00001760 rdf:datatype="http://www.w3.org/2001/XMLSchema#anyURI">https://www.commoncoreontologies.org/InformationEntityOntology</cco:ont00001760>
  </rdf:Description>
  <rdf:Description rdf:about="https://www.commoncoreontologies.org/ont00001908">
    <rdf:type rdf:resource="http://www.w3.org/2002/07/owl#ObjectProperty"/>
    <rdfs:subPropertyOf rdf:resource="http://purl.obolibrary.org/obo/BFO_0000101"/>
    <rdfs:domain rdf:resource="https://www.commoncoreontologies.org/ont00000253"/>
    <rdfs:range rdf:resource="https://www.commoncoreontologies.org/ont00000829"/>
    <rdfs:label xml:lang="en">uses time zone identifier</rdfs:label>
    <skos:definition xml:lang="en">x uses_time_zone_identifier y iff x is an instance of Information Bearing Entity and y is an instance of Time Zone Identifier, such that y designates the spatial region associated with the time zone mentioned in x.</skos:definition>
    <cco:ont00001760 rdf:datatype="http://www.w3.org/2001/XMLSchema#anyURI">https://www.commoncoreontologies.org/InformationEntityOntology</cco:ont00001760>
  </rdf:Description>
  <rdf:Description rdf:about="https://www.commoncoreontologies.org/ont00000686">
    <rdf:type rdf:resource="http://www.w3.org/2002/07/owl#Class"/>
    <owl:equivalentClass rdf:nodeID="na8580e9876f64da8bd2fccebf064ee6cb35"/>
    <rdfs:subClassOf rdf:resource="https://www.commoncoreontologies.org/ont00000958"/>
    <owl:disjointWith rdf:resource="https://www.commoncoreontologies.org/ont00000853"/>
    <owl:disjointWith rdf:resource="https://www.commoncoreontologies.org/ont00000965"/>
    <rdfs:label xml:lang="en">Designative Information Content Entity</rdfs:label>
    <skos:altLabel xml:lang="en">Designative ICE</skos:altLabel>
    <skos:definition xml:lang="en">An Information Content Entity that consists of a set of symbols that designate some Entity.</skos:definition>
    <cco:ont00001760 rdf:datatype="http://www.w3.org/2001/XMLSchema#anyURI">https://www.commoncoreontologies.org/InformationEntityOntology</cco:ont00001760>
  </rdf:Description>
  <rdf:Description rdf:about="https://www.commoncoreontologies.org/ont00001454">
    <rdf:type rdf:resource="http://www.w3.org/2002/07/owl#NamedIndividual"/>
    <rdf:type rdf:resource="https://www.commoncoreontologies.org/ont00001235"/>
    <rdfs:comment xml:lang="en">Offset from Universal Coordinated Time = UTC+11</rdfs:comment>
    <rdfs:label xml:lang="en">Lima Time Zone</rdfs:label>
    <cco:ont00001753>L</cco:ont00001753>
    <cco:ont00001760 rdf:datatype="http://www.w3.org/2001/XMLSchema#anyURI">https://www.commoncoreontologies.org/InformationEntityOntology</cco:ont00001760>
  </rdf:Description>
  <rdf:Description rdf:about="https://www.commoncoreontologies.org/ont00000916">
    <rdf:type rdf:resource="http://www.w3.org/2002/07/owl#Class"/>
    <rdfs:subClassOf rdf:resource="https://www.commoncoreontologies.org/ont00000891"/>
    <rdfs:label xml:lang="en">Lunar Calendar System</rdfs:label>
    <skos:definition xml:lang="en">A Calendar System that is designed to organize and identify dates based on the cycles of the Moon's phases.</skos:definition>
    <cco:ont00001754 rdf:datatype="http://www.w3.org/2001/XMLSchema#anyURI">https://en.wikipedia.org/w/index.php?title=Lunar_calendar&amp;oldid=1055396837</cco:ont00001754>
    <cco:ont00001760 rdf:datatype="http://www.w3.org/2001/XMLSchema#anyURI">https://www.commoncoreontologies.org/InformationEntityOntology</cco:ont00001760>
  </rdf:Description>
  <rdf:Description rdf:about="https://www.commoncoreontologies.org/ont00001693">
    <rdf:type rdf:resource="http://www.w3.org/2002/07/owl#NamedIndividual"/>
    <rdf:type rdf:resource="https://www.commoncoreontologies.org/ont00001235"/>
    <rdfs:comment xml:lang="en">Offset from Universal Coordinated Time = UTC+0</rdfs:comment>
    <rdfs:label xml:lang="en">Zulu Time Zone</rdfs:label>
    <cco:ont00001753>Z</cco:ont00001753>
    <cco:ont00001760 rdf:datatype="http://www.w3.org/2001/XMLSchema#anyURI">https://www.commoncoreontologies.org/InformationEntityOntology</cco:ont00001760>
  </rdf:Description>
  <rdf:Description rdf:about="https://www.commoncoreontologies.org/ont00001884">
    <rdf:type rdf:resource="http://www.w3.org/2002/07/owl#ObjectProperty"/>
    <rdfs:subPropertyOf rdf:resource="https://www.commoncoreontologies.org/ont00001801"/>
    <owl:inverseOf rdf:resource="https://www.commoncoreontologies.org/ont00001980"/>
    <rdfs:domain rdf:resource="http://purl.obolibrary.org/obo/BFO_0000001"/>
    <rdfs:range rdf:resource="https://www.commoncoreontologies.org/ont00000127"/>
    <owl:propertyChainAxiom rdf:nodeID="na8580e9876f64da8bd2fccebf064ee6cb1"/>
    <rdfs:label xml:lang="en">condition described by</rdfs:label>
    <skos:definition xml:lang="en">x condition_described_by y iff y is an instance of Performance Specification and x is an instance of Entity and y describes_condition x.</skos:definition>
    <cco:ont00001760 rdf:datatype="http://www.w3.org/2001/XMLSchema#anyURI">https://www.commoncoreontologies.org/InformationEntityOntology</cco:ont00001760>
  </rdf:Description>
  <rdf:Description rdf:about="https://www.commoncoreontologies.org/ont00001980">
    <rdf:type rdf:resource="http://www.w3.org/2002/07/owl#ObjectProperty"/>
    <rdfs:subPropertyOf rdf:resource="https://www.commoncoreontologies.org/ont00001808"/>
    <rdfs:domain rdf:resource="https://www.commoncoreontologies.org/ont00000127"/>
    <rdfs:range rdf:resource="http://purl.obolibrary.org/obo/BFO_0000001"/>
    <owl:propertyChainAxiom rdf:nodeID="na8580e9876f64da8bd2fccebf064ee6cb3"/>
    <rdfs:label xml:lang="en">describes condition</rdfs:label>
    <skos:definition xml:lang="en">p describes_condition c iff p is an instance of a Performance Specification and c is an instance of Entity and p has part d, and d is an instance of a Descriptive Information Content Entity, and p prescribes an entity s, and d describes c, and c is an entity that is causally relevant to s existing as prescribed by p.</skos:definition>
    <cco:ont00001760 rdf:datatype="http://www.w3.org/2001/XMLSchema#anyURI">https://www.commoncoreontologies.org/InformationEntityOntology</cco:ont00001760>
  </rdf:Description>
  <rdf:Description rdf:about="https://www.commoncoreontologies.org/ont00001754">
    <rdf:type rdf:resource="http://www.w3.org/2002/07/owl#AnnotationProperty"/>
  </rdf:Description>
  <rdf:Description rdf:about="https://www.commoncoreontologies.org/ont00001022">
    <rdf:type rdf:resource="http://www.w3.org/2002/07/owl#Class"/>
    <owl:equivalentClass rdf:nodeID="na8580e9876f64da8bd2fccebf064ee6cb63"/>
    <rdfs:subClassOf rdf:resource="https://www.commoncoreontologies.org/ont00001163"/>
    <owl:disjointWith rdf:resource="https://www.commoncoreontologies.org/ont00001364"/>
    <rdfs:comment xml:lang="en">Four of the subtypes of measurements used here (Interval, Nominal, Ordinal, and Ratio) were originally defined by S.S. Stevens in the article "On the Theory of Scales of Measurement" in Science, Vol. 103 No. 2684 on June 7, 1946. For an introductory article with links to additional content including criticisms and alternate classifications of measurements see https://en.wikipedia.org/wiki/Level_of_measurement</rdfs:comment>
    <rdfs:label xml:lang="en">Ratio Measurement Information Content Entity</rdfs:label>
    <skos:definition xml:lang="en">A Measurement Information Content Entity that consists of a symbol that places a Quality of an Entity onto an interval scale having a true zero value.</skos:definition>
    <skos:example xml:lang="en">The sentence "The temperature reached 240.372 degrees Kelvin on January 20, 1985 in Chicago, IL." is the carrier of a ratio measurement as 0 degrees on the Kelvin scale does describe absolute zero.</skos:example>
    <skos:example>a measurement of the barometric pressure at 1,000 feet above sea level</skos:example>
    <skos:example>a measurement of the measure of air temperature on the Kelvin scale</skos:example>
    <skos:example>a measurement of the number of members in an Organization</skos:example>
    <cco:ont00001760 rdf:datatype="http://www.w3.org/2001/XMLSchema#anyURI">https://www.commoncoreontologies.org/InformationEntityOntology</cco:ont00001760>
  </rdf:Description>
  <rdf:Description rdf:about="https://www.commoncoreontologies.org/ont00000604">
    <rdf:type rdf:resource="http://www.w3.org/2002/07/owl#Class"/>
    <rdfs:subClassOf rdf:resource="https://www.commoncoreontologies.org/ont00001010"/>
    <rdfs:label xml:lang="en">Maximum Ordinal Measurement Information Content Entity</rdfs:label>
    <skos:definition xml:lang="en">An Ordinal Measurement Information Content Entity that is a measurement of some entity in virtue of it being the largest or having the greatest amount relative to a nominally described set of like entities.</skos:definition>
    <cco:ont00001760 rdf:datatype="http://www.w3.org/2001/XMLSchema#anyURI">https://www.commoncoreontologies.org/InformationEntityOntology</cco:ont00001760>
  </rdf:Description>
  <rdf:Description rdf:about="https://www.commoncoreontologies.org/ont00002002">
    <rdf:type rdf:resource="http://www.w3.org/2002/07/owl#Class"/>
    <rdfs:subClassOf rdf:resource="https://www.commoncoreontologies.org/ont00002001"/>
    <rdfs:label xml:lang="en">Certificate</rdfs:label>
    <skos:definition xml:lang="en">A Media Content Entity that attests to certain demonstrated characteristics of an Object, Person, or Organization.</skos:definition>
    <cco:ont00001754>http://www.dictionary.com/browse/degree</cco:ont00001754>
    <cco:ont00001760 rdf:datatype="http://www.w3.org/2001/XMLSchema#anyURI">https://www.commoncoreontologies.org/InformationEntityOntology</cco:ont00001760>
  </rdf:Description>
  <rdf:Description rdf:about="https://www.commoncoreontologies.org/ont00001516">
    <rdf:type rdf:resource="http://www.w3.org/2002/07/owl#NamedIndividual"/>
    <rdf:type rdf:resource="https://www.commoncoreontologies.org/ont00001235"/>
    <rdfs:comment xml:lang="en">Offset from Universal Coordinated Time = UTC-2</rdfs:comment>
    <rdfs:label xml:lang="en">Oscar Time Zone</rdfs:label>
    <cco:ont00001753>O</cco:ont00001753>
    <cco:ont00001760 rdf:datatype="http://www.w3.org/2001/XMLSchema#anyURI">https://www.commoncoreontologies.org/InformationEntityOntology</cco:ont00001760>
  </rdf:Description>
  <rdf:Description rdf:about="https://www.commoncoreontologies.org/ont00000539">
    <rdf:type rdf:resource="http://www.w3.org/2002/07/owl#Class"/>
    <rdfs:subClassOf rdf:resource="https://www.commoncoreontologies.org/ont00001022"/>
    <rdfs:label xml:lang="en">Count Measurement Information Content Entity</rdfs:label>
    <skos:definition xml:lang="en">A Ratio Measurement Information Content Entity that is a measurement of the number of members of some aggregate.</skos:definition>
    <cco:ont00001760 rdf:datatype="http://www.w3.org/2001/XMLSchema#anyURI">https://www.commoncoreontologies.org/InformationEntityOntology</cco:ont00001760>
  </rdf:Description>
  <rdf:Description rdf:about="https://www.commoncoreontologies.org/ont00001527">
    <rdf:type rdf:resource="http://www.w3.org/2002/07/owl#NamedIndividual"/>
    <rdf:type rdf:resource="https://www.commoncoreontologies.org/ont00001235"/>
    <rdfs:comment xml:lang="en">Offset from Universal Coordinated Time = UTC+8</rdfs:comment>
    <rdfs:label xml:lang="en">Hotel Time Zone</rdfs:label>
    <cco:ont00001753>H</cco:ont00001753>
    <cco:ont00001760 rdf:datatype="http://www.w3.org/2001/XMLSchema#anyURI">https://www.commoncoreontologies.org/InformationEntityOntology</cco:ont00001760>
  </rdf:Description>
  <rdf:Description rdf:about="https://www.commoncoreontologies.org/ont00000276">
    <rdf:type rdf:resource="http://www.w3.org/2002/07/owl#Class"/>
    <rdfs:subClassOf rdf:resource="https://www.commoncoreontologies.org/ont00000891"/>
    <rdfs:label xml:lang="en">Solar Calendar System</rdfs:label>
    <skos:definition xml:lang="en">A Calendar System that is designed to organize and identify dates based on the cycles of an Astronomical Body's Orbit around the Sun.</skos:definition>
    <skos:scopeNote xml:lang="en">Unless otherwise specified, a Solar Calendar System is assumed to be relative to the Orbit of the Earth around the Sun.</skos:scopeNote>
    <cco:ont00001754 rdf:datatype="http://www.w3.org/2001/XMLSchema#anyURI">https://en.wikipedia.org/w/index.php?title=Solar_calendar&amp;oldid=1058016588</cco:ont00001754>
    <cco:ont00001760 rdf:datatype="http://www.w3.org/2001/XMLSchema#anyURI">https://www.commoncoreontologies.org/InformationEntityOntology</cco:ont00001760>
  </rdf:Description>
  <rdf:Description rdf:about="https://www.commoncoreontologies.org/ont00001692">
    <rdf:type rdf:resource="http://www.w3.org/2002/07/owl#NamedIndividual"/>
    <rdf:type rdf:resource="https://www.commoncoreontologies.org/ont00001328"/>
    <rdfs:comment xml:lang="en">Unix Time is a Temporal Reference System for describing a point in time, defined as the number of seconds that have elapsed since 00:00:00 Coordinated Universal Time (UTC) Thursday, 1 January 1970 minus the number of leap seconds that have taken place since then.
(See: https://en.wikipedia.org/wiki/Unix_time)</rdfs:comment>
    <rdfs:label xml:lang="en">Unix Time</rdfs:label>
    <cco:ont00001760 rdf:datatype="http://www.w3.org/2001/XMLSchema#anyURI">https://www.commoncoreontologies.org/InformationEntityOntology</cco:ont00001760>
  </rdf:Description>
  <rdf:Description rdf:about="https://www.commoncoreontologies.org/ont00001500">
    <rdf:type rdf:resource="http://www.w3.org/2002/07/owl#NamedIndividual"/>
    <rdf:type rdf:resource="https://www.commoncoreontologies.org/ont00001235"/>
    <rdfs:comment xml:lang="en">Offset from Universal Coordinated Time = UTC+5</rdfs:comment>
    <rdfs:label xml:lang="en">Echo Time Zone</rdfs:label>
    <cco:ont00001753>E</cco:ont00001753>
    <cco:ont00001760 rdf:datatype="http://www.w3.org/2001/XMLSchema#anyURI">https://www.commoncoreontologies.org/InformationEntityOntology</cco:ont00001760>
  </rdf:Description>
  <rdf:Description rdf:nodeID="na8580e9876f64da8bd2fccebf064ee6cb65">
    <rdf:first rdf:resource="https://www.commoncoreontologies.org/ont00001163"/>
    <rdf:rest rdf:nodeID="na8580e9876f64da8bd2fccebf064ee6cb66"/>
  </rdf:Description>
  <rdf:Description rdf:about="https://www.commoncoreontologies.org/ont00000853">
    <rdf:type rdf:resource="http://www.w3.org/2002/07/owl#Class"/>
    <owl:equivalentClass rdf:nodeID="na8580e9876f64da8bd2fccebf064ee6cb47"/>
    <rdfs:subClassOf rdf:resource="https://www.commoncoreontologies.org/ont00000958"/>
    <owl:disjointWith rdf:resource="https://www.commoncoreontologies.org/ont00000965"/>
    <rdfs:label xml:lang="en">Descriptive Information Content Entity</rdfs:label>
    <skos:altLabel xml:lang="en">Descriptive ICE</skos:altLabel>
    <skos:definition xml:lang="en">An Information Content Entity that consists of a set of propositions that describe some Entity.</skos:definition>
    <cco:ont00001760 rdf:datatype="http://www.w3.org/2001/XMLSchema#anyURI">https://www.commoncoreontologies.org/InformationEntityOntology</cco:ont00001760>
  </rdf:Description>
  <rdf:Description rdf:about="https://www.commoncoreontologies.org/ont00001808">
    <rdf:type rdf:resource="http://www.w3.org/2002/07/owl#ObjectProperty"/>
    <rdfs:domain rdf:resource="https://www.commoncoreontologies.org/ont00000958"/>
    <rdfs:range rdf:resource="http://purl.obolibrary.org/obo/BFO_0000001"/>
    <rdfs:label xml:lang="en">is about</rdfs:label>
    <skos:definition xml:lang="en">x is_about y is a primitive relationship between an instance of Information Content Entity x and an instance of Entity y.</skos:definition>
    <cco:ont00001754>http://purl.obolibrary.org/obo/IAO_0000136</cco:ont00001754>
    <cco:ont00001760 rdf:datatype="http://www.w3.org/2001/XMLSchema#anyURI">https://www.commoncoreontologies.org/InformationEntityOntology</cco:ont00001760>
  </rdf:Description>
  <rdf:Description rdf:about="https://www.commoncoreontologies.org/ont00001964">
    <rdf:type rdf:resource="http://www.w3.org/2002/07/owl#ObjectProperty"/>
    <rdfs:subPropertyOf rdf:resource="https://www.commoncoreontologies.org/ont00001904"/>
    <rdfs:domain rdf:resource="http://purl.obolibrary.org/obo/BFO_0000001"/>
    <rdfs:range rdf:resource="https://www.commoncoreontologies.org/ont00001364"/>
    <rdfs:label xml:lang="en">is measured by interval</rdfs:label>
    <skos:definition xml:lang="en">y is_measured_by_interval x iff x is an instance of Interval Measurement Information Content Entity and y is an instance of Entity, such that x describes some attribute of y relative to a scale which has uniform intervals but has a zero value that does not correspond to an absence of the attribute being measured.</skos:definition>
    <cco:ont00001760 rdf:datatype="http://www.w3.org/2001/XMLSchema#anyURI">https://www.commoncoreontologies.org/InformationEntityOntology</cco:ont00001760>
  </rdf:Description>
  <rdf:Description rdf:about="https://www.commoncoreontologies.org/ont00001351">
    <rdf:type rdf:resource="http://www.w3.org/2002/07/owl#Class"/>
    <rdfs:subClassOf rdf:resource="https://www.commoncoreontologies.org/ont00000275"/>
    <rdfs:label xml:lang="en">Cartesian Coordinate System</rdfs:label>
    <skos:altLabel xml:lang="en">Rectangular Coordinate System</skos:altLabel>
    <skos:definition xml:lang="en">A Spatial Reference System that identifies each point in a spatial region of n-dimensions using an ordered n-tuple of numerical coordinates that are the signed (i.e. positive or negative) distances measured in the same unit of length from the zero point where the fixed perpendicular Coordinate System Axes meet.</skos:definition>
    <cco:ont00001754 rdf:datatype="http://www.w3.org/2001/XMLSchema#anyURI">https://en.wikipedia.org/w/index.php?title=Cartesian_coordinate_system&amp;oldid=1058613323</cco:ont00001754>
    <cco:ont00001760 rdf:datatype="http://www.w3.org/2001/XMLSchema#anyURI">https://www.commoncoreontologies.org/InformationEntityOntology</cco:ont00001760>
  </rdf:Description>
  <rdf:Description rdf:about="https://www.commoncoreontologies.org/ont00000164">
    <rdf:type rdf:resource="http://www.w3.org/2002/07/owl#Class"/>
    <rdfs:subClassOf rdf:resource="https://www.commoncoreontologies.org/ont00001010"/>
    <rdfs:label xml:lang="en">Minimum Ordinal Measurement Information Content Entity</rdfs:label>
    <skos:definition xml:lang="en">An Ordinal Measurement Information Content Entity that is a measurement of some entity in virtue of it being the smallest or having the least amount relative to a nominally described set of like entities.</skos:definition>
    <cco:ont00001760 rdf:datatype="http://www.w3.org/2001/XMLSchema#anyURI">https://www.commoncoreontologies.org/InformationEntityOntology</cco:ont00001760>
  </rdf:Description>
  <rdf:Description rdf:nodeID="na8580e9876f64da8bd2fccebf064ee6cb54">
    <rdf:first rdf:nodeID="na8580e9876f64da8bd2fccebf064ee6cb52"/>
    <rdf:rest rdf:resource="http://www.w3.org/1999/02/22-rdf-syntax-ns#nil"/>
  </rdf:Description>
  <rdf:Description rdf:about="https://www.commoncoreontologies.org/ont00001701">
    <rdf:type rdf:resource="http://www.w3.org/2002/07/owl#NamedIndividual"/>
    <rdf:type rdf:resource="https://www.commoncoreontologies.org/ont00001352"/>
    <rdfs:label xml:lang="en">GMT-3</rdfs:label>
    <skos:altLabel xml:lang="en">AGT</skos:altLabel>
    <skos:altLabel xml:lang="en">Argentina Standard Time</skos:altLabel>
    <cco:ont00001760 rdf:datatype="http://www.w3.org/2001/XMLSchema#anyURI">https://www.commoncoreontologies.org/InformationEntityOntology</cco:ont00001760>
  </rdf:Description>
  <rdf:Description rdf:about="https://www.commoncoreontologies.org/ont00001406">
    <rdf:type rdf:resource="http://www.w3.org/2002/07/owl#NamedIndividual"/>
    <rdf:type rdf:resource="https://www.commoncoreontologies.org/ont00001352"/>
    <rdfs:label xml:lang="en">GMT+9:30</rdfs:label>
    <skos:altLabel xml:lang="en">Australian Central Standard Time</skos:altLabel>
    <cco:ont00001753>ACST</cco:ont00001753>
    <cco:ont00001760 rdf:datatype="http://www.w3.org/2001/XMLSchema#anyURI">https://www.commoncoreontologies.org/InformationEntityOntology</cco:ont00001760>
  </rdf:Description>
  <rdf:Description rdf:about="https://www.commoncoreontologies.org/ont00000896">
    <rdf:type rdf:resource="http://www.w3.org/2002/07/owl#Class"/>
    <rdfs:subClassOf rdf:resource="https://www.commoncoreontologies.org/ont00000745"/>
    <rdfs:label xml:lang="en">Mean Point Estimate Information Content Entity</rdfs:label>
    <skos:altLabel xml:lang="en">Arithmetic Mean</skos:altLabel>
    <skos:altLabel xml:lang="en">Average</skos:altLabel>
    <skos:altLabel xml:lang="en">Mean</skos:altLabel>
    <skos:definition xml:lang="en">A Point Estimate Information Content Entity that is a measurement of a set of values and is equal to the sum of all the values in the set divided by the total number of values in the set.</skos:definition>
    <cco:ont00001760 rdf:datatype="http://www.w3.org/2001/XMLSchema#anyURI">https://www.commoncoreontologies.org/InformationEntityOntology</cco:ont00001760>
  </rdf:Description>
  <rdf:Description rdf:about="https://www.commoncoreontologies.org/ont00000003">
    <rdf:type rdf:resource="http://www.w3.org/2002/07/owl#Class"/>
    <rdfs:subClassOf rdf:resource="https://www.commoncoreontologies.org/ont00000686"/>
    <owl:disjointWith rdf:resource="https://www.commoncoreontologies.org/ont00000649"/>
    <rdfs:label xml:lang="en">Designative Name</rdfs:label>
    <skos:altLabel xml:lang="en">Name</skos:altLabel>
    <skos:definition xml:lang="en">A Designative Information Content Entity that consists of a string of characters that designates an entity within a specified cultural or social namespace and which is typically a word or phrase in a natural language that has an accepted cultural or social significance.</skos:definition>
    <cco:ont00001760 rdf:datatype="http://www.w3.org/2001/XMLSchema#anyURI">https://www.commoncoreontologies.org/InformationEntityOntology</cco:ont00001760>
  </rdf:Description>
  <rdf:Description rdf:about="https://www.commoncoreontologies.org/ont00001238">
    <rdf:type rdf:resource="http://www.w3.org/2002/07/owl#Class"/>
    <rdfs:subClassOf rdf:resource="https://www.commoncoreontologies.org/ont00000605"/>
    <rdfs:label xml:lang="en">Initialism</rdfs:label>
    <skos:definition xml:lang="en">An Abbreviated Name that consists of the initial letters of some words (or syllables) in a Designative Name, and in which each letter is pronounced separately.</skos:definition>
    <skos:example>USA, CPU, BBC</skos:example>
    <cco:ont00001760 rdf:datatype="http://www.w3.org/2001/XMLSchema#anyURI">https://www.commoncoreontologies.org/InformationEntityOntology</cco:ont00001760>
  </rdf:Description>
  <rdf:Description rdf:nodeID="na8580e9876f64da8bd2fccebf064ee6cb16">
    <rdf:first rdf:resource="https://www.commoncoreontologies.org/ont00001163"/>
    <rdf:rest rdf:nodeID="na8580e9876f64da8bd2fccebf064ee6cb17"/>
  </rdf:Description>
  <rdf:Description rdf:about="https://www.commoncoreontologies.org/ont00000398">
    <rdf:type rdf:resource="http://www.w3.org/2002/07/owl#Class"/>
    <rdfs:subClassOf rdf:resource="https://www.commoncoreontologies.org/ont00000853"/>
    <rdfs:label xml:lang="en">Reference System</rdfs:label>
    <skos:definition xml:lang="en">A Descriptive Information Content Entity that describes a set of standards for organizing and understanding data of the specified type or domain.</skos:definition>
    <cco:ont00001760 rdf:datatype="http://www.w3.org/2001/XMLSchema#anyURI">https://www.commoncoreontologies.org/InformationEntityOntology</cco:ont00001760>
  </rdf:Description>
  <rdf:Description rdf:about="https://www.commoncoreontologies.org/ont00001588">
    <rdf:type rdf:resource="http://www.w3.org/2002/07/owl#NamedIndividual"/>
    <rdf:type rdf:resource="https://www.commoncoreontologies.org/ont00001352"/>
    <rdfs:label xml:lang="en">GMT+9</rdfs:label>
    <skos:altLabel xml:lang="en">JST</skos:altLabel>
    <skos:altLabel xml:lang="en">Japan Standard Time</skos:altLabel>
    <cco:ont00001760 rdf:datatype="http://www.w3.org/2001/XMLSchema#anyURI">https://www.commoncoreontologies.org/InformationEntityOntology</cco:ont00001760>
  </rdf:Description>
  <rdf:Description rdf:about="https://www.commoncoreontologies.org/ont00001414">
    <rdf:type rdf:resource="http://www.w3.org/2002/07/owl#NamedIndividual"/>
    <rdf:type rdf:resource="https://www.commoncoreontologies.org/ont00001328"/>
    <rdfs:comment xml:lang="en">TT is an astronomical time standard that is a theoretical ideal designed to be free of the irregularities in Earth's rotation and is primarily used for time measurements of astronomical observations made from the surface of Earth. It was formerly called Terrestrial Dynamical Time (TDT), which was formulated to replace Ephemeris Time (ET).</rdfs:comment>
    <rdfs:label xml:lang="en">Terrestrial Time</rdfs:label>
    <cco:ont00001753>TT</cco:ont00001753>
    <cco:ont00001760 rdf:datatype="http://www.w3.org/2001/XMLSchema#anyURI">https://www.commoncoreontologies.org/InformationEntityOntology</cco:ont00001760>
  </rdf:Description>
  <rdf:Description rdf:about="https://www.commoncoreontologies.org/ont00001309">
    <rdf:type rdf:resource="http://www.w3.org/2002/07/owl#Class"/>
    <rdfs:subClassOf rdf:resource="https://www.commoncoreontologies.org/ont00000077"/>
    <rdfs:label xml:lang="en">Lot Number</rdfs:label>
    <skos:definition xml:lang="en">A Code Identifier that designates a particular quantity or lot of material from a single manufacturer.</skos:definition>
    <cco:ont00001754 rdf:datatype="http://www.w3.org/2001/XMLSchema#anyURI">https://en.wikipedia.org/w/index.php?title=Lot_number&amp;oldid=1061846325</cco:ont00001754>
    <cco:ont00001760 rdf:datatype="http://www.w3.org/2001/XMLSchema#anyURI">https://www.commoncoreontologies.org/InformationEntityOntology</cco:ont00001760>
  </rdf:Description>
  <rdf:Description rdf:about="https://www.commoncoreontologies.org/ont00002039">
    <rdf:type rdf:resource="http://www.w3.org/2002/07/owl#Class"/>
    <rdfs:subClassOf rdf:resource="https://www.commoncoreontologies.org/ont00002001"/>
    <rdfs:label xml:lang="en">Document Content Entity</rdfs:label>
    <skos:altLabel xml:lang="en">Document</skos:altLabel>
    <skos:definition xml:lang="en">A Media Content Entity that consists of a series of paragraphs of text or diagrams that are intended to be carried by physical pieces of paper or an electronic word processor file.</skos:definition>
    <cco:ont00001754 rdf:datatype="http://www.w3.org/2001/XMLSchema#anyURI">https://en.wikipedia.org/w/index.php?title=Document&amp;oldid=1057829688</cco:ont00001754>
    <cco:ont00001760 rdf:datatype="http://www.w3.org/2001/XMLSchema#anyURI">https://www.commoncoreontologies.org/InformationEntityOntology</cco:ont00001760>
  </rdf:Description>
  <rdf:Description rdf:about="https://www.commoncoreontologies.org/ont00002023">
    <rdf:type rdf:resource="http://www.w3.org/2002/07/owl#Class"/>
    <rdfs:subClassOf rdf:resource="https://www.commoncoreontologies.org/ont00002020"/>
    <rdfs:label xml:lang="en">ITF Barcode</rdfs:label>
    <skos:definition xml:lang="en">A One-Dimensional Barcode that represents an even number of numerical characters and is used primarily in packaging and distribution.</skos:definition>
    <cco:ont00001760 rdf:datatype="http://www.w3.org/2001/XMLSchema#anyURI">https://www.commoncoreontologies.org/InformationEntityOntology</cco:ont00001760>
  </rdf:Description>
  <rdf:Description rdf:about="https://www.commoncoreontologies.org/ont00001767">
    <rdf:type rdf:resource="http://www.w3.org/2002/07/owl#DatatypeProperty"/>
    <rdfs:domain rdf:resource="https://www.commoncoreontologies.org/ont00000253"/>
    <rdfs:range rdf:resource="http://www.w3.org/2001/XMLSchema#dateTime"/>
    <rdfs:label xml:lang="en">has datetime value</rdfs:label>
    <skos:definition xml:lang="en">A data property that has as its value a datetime value.</skos:definition>
    <cco:ont00001760 rdf:datatype="http://www.w3.org/2001/XMLSchema#anyURI">https://www.commoncoreontologies.org/InformationEntityOntology</cco:ont00001760>
  </rdf:Description>
  <rdf:Description rdf:about="https://www.commoncoreontologies.org/ont00001666">
    <rdf:type rdf:resource="http://www.w3.org/2002/07/owl#NamedIndividual"/>
    <rdf:type rdf:resource="https://www.commoncoreontologies.org/ont00001328"/>
    <rdfs:comment xml:lang="en">"Barycentric Coordinate Time (TCB, from the French Temps-coordonne barycentrique) is a coordinate time standard intended to be used as the independent variable of time for all calculations pertaining to orbits of planets, asteroids, comets, and interplanetary spacecraft in the Solar system. It is equivalent to the proper time experienced by a clock at rest in a coordinate frame co-moving with the barycenter of the Solar system: that is, a clock that performs exactly the same movements as the Solar system but is outside the system's gravity well. It is therefore not influenced by the gravitational time dilation caused by the Sun and the rest of the system."
From: (https://en.wikipedia.org/wiki/Barycentric_Coordinate_Time)</rdfs:comment>
    <rdfs:label xml:lang="en">Barycentric Coordinate Time</rdfs:label>
    <cco:ont00001753>TCB</cco:ont00001753>
    <cco:ont00001760 rdf:datatype="http://www.w3.org/2001/XMLSchema#anyURI">https://www.commoncoreontologies.org/InformationEntityOntology</cco:ont00001760>
  </rdf:Description>
  <rdf:Description rdf:nodeID="na8580e9876f64da8bd2fccebf064ee6cb32">
    <rdf:type rdf:resource="http://www.w3.org/2002/07/owl#Restriction"/>
    <owl:onProperty rdf:resource="https://www.commoncoreontologies.org/ont00001916"/>
    <owl:someValuesFrom rdf:resource="http://purl.obolibrary.org/obo/BFO_0000203"/>
  </rdf:Description>
  <rdf:Description rdf:about="https://www.commoncoreontologies.org/ont00001591">
    <rdf:type rdf:resource="http://www.w3.org/2002/07/owl#NamedIndividual"/>
    <rdf:type rdf:resource="https://www.commoncoreontologies.org/ont00001235"/>
    <rdfs:comment xml:lang="en">Offset from Universal Coordinated Time = UTC-8</rdfs:comment>
    <rdfs:label xml:lang="en">Uniform Time Zone</rdfs:label>
    <cco:ont00001753>U</cco:ont00001753>
    <cco:ont00001760 rdf:datatype="http://www.w3.org/2001/XMLSchema#anyURI">https://www.commoncoreontologies.org/InformationEntityOntology</cco:ont00001760>
  </rdf:Description>
  <rdf:Description rdf:about="https://www.commoncoreontologies.org/ont00001626">
    <rdf:type rdf:resource="http://www.w3.org/2002/07/owl#NamedIndividual"/>
    <rdf:type rdf:resource="https://www.commoncoreontologies.org/ont00000263"/>
    <rdfs:label xml:lang="en">Twelve-Hour Clock Time System</rdfs:label>
    <skos:altLabel xml:lang="en">12-Hour Clock</skos:altLabel>
    <skos:altLabel xml:lang="en">12-Hour Clock Time System</skos:altLabel>
    <skos:altLabel xml:lang="en">Twelve Hour Clock</skos:altLabel>
    <skos:altLabel xml:lang="en">Twelve Hour Clock Time System</skos:altLabel>
    <skos:altLabel xml:lang="en">Twelve-Hour Clock</skos:altLabel>
    <skos:definition xml:lang="en">A Clock Time System for keeping the Time of Day in which the Day runs from midnight to midnight and is divided into two intervals of 12 Hours each, where: the first interval begins at midnight, ends at noon, and is indicated by the suffix 'a.m.'; the second interval begins at noon, ends at midnight, and is indicated by the suffix 'p.m.'; and the midnight and noon Hours are numbered 12 with subsequent Hours numbered 1-11.</skos:definition>
    <cco:ont00001754 rdf:datatype="http://www.w3.org/2001/XMLSchema#anyURI">https://en.wikipedia.org/w/index.php?title=12-hour_clock&amp;oldid=1057602523</cco:ont00001754>
    <cco:ont00001760 rdf:datatype="http://www.w3.org/2001/XMLSchema#anyURI">https://www.commoncoreontologies.org/InformationEntityOntology</cco:ont00001760>
  </rdf:Description>
  <rdf:Description rdf:about="https://www.commoncoreontologies.org/ont00001625">
    <rdf:type rdf:resource="http://www.w3.org/2002/07/owl#NamedIndividual"/>
    <rdf:type rdf:resource="https://www.commoncoreontologies.org/ont00000630"/>
    <rdfs:comment xml:lang="en">UT0 is a variant of Universal Time that is measured by observing the diurnal motion of stars or extragalactic radio sources at a specific location on Earth. It does not take into consideration distorting factors, in particular polar motion, such that its value will differ based on the location it is measured at.</rdfs:comment>
    <rdfs:label xml:lang="en">Universal Time 0</rdfs:label>
    <cco:ont00001753>UT0</cco:ont00001753>
    <cco:ont00001760 rdf:datatype="http://www.w3.org/2001/XMLSchema#anyURI">https://www.commoncoreontologies.org/InformationEntityOntology</cco:ont00001760>
  </rdf:Description>
  <rdf:Description rdf:nodeID="na8580e9876f64da8bd2fccebf064ee6cb1">
    <rdf:first rdf:resource="https://www.commoncoreontologies.org/ont00001917"/>
    <rdf:rest rdf:nodeID="na8580e9876f64da8bd2fccebf064ee6cb2"/>
  </rdf:Description>
  <rdf:Description rdf:nodeID="na8580e9876f64da8bd2fccebf064ee6cb12">
    <rdf:first rdf:resource="http://purl.obolibrary.org/obo/BFO_0000030"/>
    <rdf:rest rdf:nodeID="na8580e9876f64da8bd2fccebf064ee6cb13"/>
  </rdf:Description>
  <rdf:Description rdf:about="https://www.commoncoreontologies.org/ont00002035">
    <rdf:type rdf:resource="http://www.w3.org/2002/07/owl#Class"/>
    <rdfs:subClassOf rdf:resource="https://www.commoncoreontologies.org/ont00002034"/>
    <rdfs:label xml:lang="en">UPC-A Barcode</rdfs:label>
    <skos:definition xml:lang="en">A UPC Barcode that represents 12 numerical digits.</skos:definition>
    <cco:ont00001760 rdf:datatype="http://www.w3.org/2001/XMLSchema#anyURI">https://www.commoncoreontologies.org/InformationEntityOntology</cco:ont00001760>
  </rdf:Description>
  <rdf:Description rdf:about="https://www.commoncoreontologies.org/ont00001868">
    <rdf:type rdf:resource="http://www.w3.org/2002/07/owl#ObjectProperty"/>
    <rdfs:subPropertyOf rdf:resource="https://www.commoncoreontologies.org/ont00001966"/>
    <owl:inverseOf rdf:resource="https://www.commoncoreontologies.org/ont00001914"/>
    <rdfs:domain rdf:resource="https://www.commoncoreontologies.org/ont00000293"/>
    <rdfs:range rdf:resource="http://purl.obolibrary.org/obo/BFO_0000001"/>
    <rdfs:label xml:lang="en">is a nominal measurement of</rdfs:label>
    <skos:definition xml:lang="en">x is_a_nominal_measurement_of y iff x is an instance of Information Content Entity and y is an instance of Entity, such that x classifies y relative to some set of shared, possibly arbitrary, characteristics.</skos:definition>
    <cco:ont00001760 rdf:datatype="http://www.w3.org/2001/XMLSchema#anyURI">https://www.commoncoreontologies.org/InformationEntityOntology</cco:ont00001760>
  </rdf:Description>
  <rdf:Description rdf:about="https://www.commoncoreontologies.org/ont00001691">
    <rdf:type rdf:resource="http://www.w3.org/2002/07/owl#NamedIndividual"/>
    <rdf:type rdf:resource="https://www.commoncoreontologies.org/ont00001352"/>
    <rdfs:label xml:lang="en">GMT-6</rdfs:label>
    <skos:altLabel xml:lang="en">CST</skos:altLabel>
    <skos:altLabel xml:lang="en">Central Standard Time</skos:altLabel>
    <cco:ont00001760 rdf:datatype="http://www.w3.org/2001/XMLSchema#anyURI">https://www.commoncoreontologies.org/InformationEntityOntology</cco:ont00001760>
  </rdf:Description>
  <rdf:Description rdf:about="https://www.commoncoreontologies.org/ont00000293">
    <rdf:type rdf:resource="http://www.w3.org/2002/07/owl#Class"/>
    <owl:equivalentClass rdf:nodeID="na8580e9876f64da8bd2fccebf064ee6cb14"/>
    <rdfs:subClassOf rdf:resource="https://www.commoncoreontologies.org/ont00001163"/>
    <owl:disjointWith rdf:resource="https://www.commoncoreontologies.org/ont00001010"/>
    <owl:disjointWith rdf:resource="https://www.commoncoreontologies.org/ont00001022"/>
    <owl:disjointWith rdf:resource="https://www.commoncoreontologies.org/ont00001364"/>
    <rdfs:comment xml:lang="en">Four of the subtypes of measurements used here (Interval, Nominal, Ordinal, and Ratio) were originally defined by S.S. Stevens in the article "On the Theory of Scales of Measurement" in Science, Vol. 103 No. 2684 on June 7, 1946. For an introductory article with links to additional content including criticisms and alternate classifications of measurements see https://en.wikipedia.org/wiki/Level_of_measurement</rdfs:comment>
    <rdfs:label xml:lang="en">Nominal Measurement Information Content Entity</rdfs:label>
    <skos:definition xml:lang="en">A Measurement Information Content Entity that consists of a symbol that classifies Entities according to some shared, possibly arbitrary, characteristic.</skos:definition>
    <skos:example xml:lang="en">The sentence "January 20, 1985 was a cold day in Chicago, IL" is the carrier of a nominal measurement.</skos:example>
    <skos:example>a measurement that classifies automobiles as sedans, coupes, hatchbacks, or convertibles</skos:example>
    <skos:example>a measurement that classifies military intelligence as strategic, operational, or tactical</skos:example>
    <skos:example>a measurement that classifies rocks as igneous, sedimentary, or metamorphic</skos:example>
    <cco:ont00001760 rdf:datatype="http://www.w3.org/2001/XMLSchema#anyURI">https://www.commoncoreontologies.org/InformationEntityOntology</cco:ont00001760>
  </rdf:Description>
  <rdf:Description rdf:about="https://www.commoncoreontologies.org/ont00000745">
    <rdf:type rdf:resource="http://www.w3.org/2002/07/owl#Class"/>
    <rdfs:subClassOf rdf:resource="https://www.commoncoreontologies.org/ont00001176"/>
    <rdfs:label xml:lang="en">Point Estimate Information Content Entity</rdfs:label>
    <skos:altLabel xml:lang="en">Best Estimate</skos:altLabel>
    <skos:altLabel xml:lang="en">Point Estimate</skos:altLabel>
    <skos:altLabel xml:lang="en">Point Estimate Measurement Information Content Entity</skos:altLabel>
    <skos:definition xml:lang="en">An Estimate Information Content Entity that consists of a single value for the measured entity.</skos:definition>
    <cco:ont00001760 rdf:datatype="http://www.w3.org/2001/XMLSchema#anyURI">https://www.commoncoreontologies.org/InformationEntityOntology</cco:ont00001760>
  </rdf:Description>
  <rdf:Description rdf:about="https://www.commoncoreontologies.org/ont00000154">
    <rdf:type rdf:resource="http://www.w3.org/2002/07/owl#Class"/>
    <rdfs:subClassOf rdf:resource="https://www.commoncoreontologies.org/ont00000745"/>
    <rdfs:comment xml:lang="en">While there is always at least one Mode for every set of data, it is possible for any given set of data to have multiple Modes. The Mode is typically most useful when the members of the set are all Nominal Measurement Information Content Entities.</rdfs:comment>
    <rdfs:label xml:lang="en">Mode Point Estimate Information Content Entity</rdfs:label>
    <skos:altLabel xml:lang="en">Mode</skos:altLabel>
    <skos:altLabel xml:lang="en">Statistical Mode</skos:altLabel>
    <skos:definition xml:lang="en">A Point Estimate Information Content Entity that is a measurement of a set of values and is equal to the value or values that occur most often in the set.</skos:definition>
    <cco:ont00001760 rdf:datatype="http://www.w3.org/2001/XMLSchema#anyURI">https://www.commoncoreontologies.org/InformationEntityOntology</cco:ont00001760>
  </rdf:Description>
  <rdf:Description rdf:about="https://www.commoncoreontologies.org/ont00000529">
    <rdf:type rdf:resource="http://www.w3.org/2002/07/owl#Class"/>
    <owl:equivalentClass rdf:nodeID="na8580e9876f64da8bd2fccebf064ee6cb27"/>
    <rdfs:subClassOf rdf:resource="https://www.commoncoreontologies.org/ont00000073"/>
    <rdfs:label xml:lang="en">Date Identifier</rdfs:label>
    <skos:altLabel xml:lang="en">Day Identifier</skos:altLabel>
    <skos:definition xml:lang="en">A Temporal Interval Identifier that designates some Day.</skos:definition>
    <cco:ont00001760 rdf:datatype="http://www.w3.org/2001/XMLSchema#anyURI">https://www.commoncoreontologies.org/InformationEntityOntology</cco:ont00001760>
  </rdf:Description>
  <rdf:Description rdf:about="https://www.commoncoreontologies.org/ont00002006">
    <rdf:type rdf:resource="http://www.w3.org/2002/07/owl#Class"/>
    <rdfs:subClassOf rdf:resource="https://www.commoncoreontologies.org/ont00002001"/>
    <rdfs:label xml:lang="en">Database</rdfs:label>
    <skos:definition xml:lang="en">A Media Content Entity that is designed to be rapidly searchable and retrievable.</skos:definition>
    <cco:ont00001754 rdf:datatype="http://www.w3.org/2001/XMLSchema#anyURI">https://en.wikipedia.org/w/index.php?title=Database&amp;oldid=1057024641</cco:ont00001754>
    <cco:ont00001760 rdf:datatype="http://www.w3.org/2001/XMLSchema#anyURI">https://www.commoncoreontologies.org/InformationEntityOntology</cco:ont00001760>
  </rdf:Description>
  <rdf:Description rdf:about="https://www.commoncoreontologies.org/ont00002016">
    <rdf:type rdf:resource="http://www.w3.org/2002/07/owl#Class"/>
    <rdfs:subClassOf rdf:resource="https://www.commoncoreontologies.org/ont00002015"/>
    <rdfs:label xml:lang="en">Aztec Code</rdfs:label>
    <skos:definition xml:lang="en">A Two-Dimensional Barcode that is used by the transportation industry to scan tickets.</skos:definition>
    <cco:ont00001760 rdf:datatype="http://www.w3.org/2001/XMLSchema#anyURI">https://www.commoncoreontologies.org/InformationEntityOntology</cco:ont00001760>
  </rdf:Description>
  <rdf:Description rdf:about="https://www.commoncoreontologies.org/ont00000827">
    <rdf:type rdf:resource="http://www.w3.org/2002/07/owl#Class"/>
    <owl:equivalentClass rdf:nodeID="na8580e9876f64da8bd2fccebf064ee6cb40"/>
    <rdfs:subClassOf rdf:resource="https://www.commoncoreontologies.org/ont00000540"/>
    <rdfs:label xml:lang="en">Time of Day Identifier</rdfs:label>
    <skos:definition xml:lang="en">A Temporal Instant Identifier that designates some Time of Day.</skos:definition>
    <cco:ont00001760 rdf:datatype="http://www.w3.org/2001/XMLSchema#anyURI">https://www.commoncoreontologies.org/InformationEntityOntology</cco:ont00001760>
  </rdf:Description>
  <rdf:Description rdf:about="https://www.commoncoreontologies.org/ont00002043">
    <rdf:type rdf:resource="http://www.w3.org/2002/07/owl#Class"/>
    <rdfs:subClassOf rdf:resource="https://www.commoncoreontologies.org/ont00002039"/>
    <rdfs:label xml:lang="en">Report</rdfs:label>
    <skos:definition xml:lang="en">A Document Content entity that conveys an account of some event, situation, or the result of some observation or inquiry.</skos:definition>
    <cco:ont00001754 rdf:datatype="http://www.w3.org/2001/XMLSchema#anyURI">https://en.wikipedia.org/w/index.php?title=Report&amp;oldid=1063765657</cco:ont00001754>
    <cco:ont00001760 rdf:datatype="http://www.w3.org/2001/XMLSchema#anyURI">https://www.commoncoreontologies.org/InformationEntityOntology</cco:ont00001760>
  </rdf:Description>
  <rdf:Description rdf:about="https://www.commoncoreontologies.org/ont00001010">
    <rdf:type rdf:resource="http://www.w3.org/2002/07/owl#Class"/>
    <owl:equivalentClass rdf:nodeID="na8580e9876f64da8bd2fccebf064ee6cb59"/>
    <rdfs:subClassOf rdf:resource="https://www.commoncoreontologies.org/ont00001163"/>
    <owl:disjointWith rdf:resource="https://www.commoncoreontologies.org/ont00001022"/>
    <owl:disjointWith rdf:resource="https://www.commoncoreontologies.org/ont00001364"/>
    <rdfs:comment xml:lang="en">Four of the subtypes of measurements used here (Interval, Nominal, Ordinal, and Ratio) were originally defined by S.S. Stevens in the article "On the Theory of Scales of Measurement" in Science, Vol. 103 No. 2684 on June 7, 1946. For an introductory article with links to additional content including criticisms and alternate classifications of measurements see https://en.wikipedia.org/wiki/Level_of_measurement</rdfs:comment>
    <rdfs:label xml:lang="en">Ordinal Measurement Information Content Entity</rdfs:label>
    <skos:definition xml:lang="en">A Measurement Information Content Entity that consists of a symbol that places an Entity into some rank order.</skos:definition>
    <skos:example xml:lang="en">The sentence "The coldest day in history in Chicago, IL. is January 20, 1985." is the carrier of an ordinal measurment.</skos:example>
    <skos:example>a measurement that places Geospatial Regions into a rank order of small, medium, large</skos:example>
    <skos:example>a measurement that places military units onto a readiness rank order of red, yellow, green</skos:example>
    <cco:ont00001760 rdf:datatype="http://www.w3.org/2001/XMLSchema#anyURI">https://www.commoncoreontologies.org/InformationEntityOntology</cco:ont00001760>
  </rdf:Description>
  <rdf:Description rdf:about="https://www.commoncoreontologies.org/InformationEntityOntology">
    <rdf:type rdf:resource="http://www.w3.org/2002/07/owl#Ontology"/>
    <owl:versionIRI rdf:resource="https://www.commoncoreontologies.org/2024-11-06/InformationEntityOntology"/>
    <owl:imports rdf:resource="https://www.commoncoreontologies.org/GeospatialOntology"/>
    <owl:imports rdf:resource="https://www.commoncoreontologies.org/TimeOntology"/>
    <dcterms:license xml:lang="en">BSD 3-Clause: https://github.com/CommonCoreOntology/CommonCoreOntologies/blob/master/LICENSE</dcterms:license>
    <dcterms:rights xml:lang="en">CUBRC Inc., see full license.</dcterms:rights>
    <rdfs:comment xml:lang="en">This ontology is designed to represent generic types of information as well as the relationships between information and other entities.</rdfs:comment>
    <rdfs:label xml:lang="en">Information Entity Ontology</rdfs:label>
    <owl:versionInfo xml:lang="en">Version 2.0</owl:versionInfo>
  </rdf:Description>
  <rdf:Description rdf:about="https://www.commoncoreontologies.org/ont00002003">
    <rdf:type rdf:resource="http://www.w3.org/2002/07/owl#Class"/>
    <rdfs:subClassOf rdf:resource="https://www.commoncoreontologies.org/ont00002002"/>
    <rdfs:label xml:lang="en">Academic Degree</rdfs:label>
    <skos:definition xml:lang="en">A Certificate issued by an Educational Organization to a Person to indicate that the Person has satisfactorily completed a course of study, or as an honorary recognition of the Person's achievement.</skos:definition>
    <cco:ont00001754>http://www.dictionary.com/browse/degree</cco:ont00001754>
    <cco:ont00001760 rdf:datatype="http://www.w3.org/2001/XMLSchema#anyURI">https://www.commoncoreontologies.org/InformationEntityOntology</cco:ont00001760>
  </rdf:Description>
  <rdf:Description rdf:about="https://www.commoncoreontologies.org/ont00001541">
    <rdf:type rdf:resource="http://www.w3.org/2002/07/owl#NamedIndividual"/>
    <rdf:type rdf:resource="https://www.commoncoreontologies.org/ont00001352"/>
    <rdfs:label xml:lang="en">GMT+12</rdfs:label>
    <skos:altLabel xml:lang="en">NST</skos:altLabel>
    <skos:altLabel xml:lang="en">New Zealand Standard Time</skos:altLabel>
    <cco:ont00001760 rdf:datatype="http://www.w3.org/2001/XMLSchema#anyURI">https://www.commoncoreontologies.org/InformationEntityOntology</cco:ont00001760>
  </rdf:Description>
  <rdf:Description rdf:nodeID="na8580e9876f64da8bd2fccebf064ee6cb53">
    <rdf:first rdf:resource="http://purl.obolibrary.org/obo/BFO_0000031"/>
    <rdf:rest rdf:nodeID="na8580e9876f64da8bd2fccebf064ee6cb54"/>
  </rdf:Description>
  <rdf:Description rdf:about="https://www.commoncoreontologies.org/ont00001607">
    <rdf:type rdf:resource="http://www.w3.org/2002/07/owl#NamedIndividual"/>
    <rdf:type rdf:resource="https://www.commoncoreontologies.org/ont00001235"/>
    <rdfs:comment xml:lang="en">Offset from Universal Coordinated Time = UTC-9</rdfs:comment>
    <rdfs:label xml:lang="en">Victor Time Zone</rdfs:label>
    <cco:ont00001753>V</cco:ont00001753>
    <cco:ont00001760 rdf:datatype="http://www.w3.org/2001/XMLSchema#anyURI">https://www.commoncoreontologies.org/InformationEntityOntology</cco:ont00001760>
  </rdf:Description>
  <rdf:Description rdf:nodeID="na8580e9876f64da8bd2fccebf064ee6cb22">
    <rdf:first rdf:nodeID="na8580e9876f64da8bd2fccebf064ee6cb20"/>
    <rdf:rest rdf:resource="http://www.w3.org/1999/02/22-rdf-syntax-ns#nil"/>
  </rdf:Description>
  <rdf:Description rdf:about="https://www.commoncoreontologies.org/ont00001899">
    <rdf:type rdf:resource="http://www.w3.org/2002/07/owl#ObjectProperty"/>
    <rdfs:subPropertyOf rdf:resource="https://www.commoncoreontologies.org/ont00001942"/>
    <owl:inverseOf rdf:resource="https://www.commoncoreontologies.org/ont00001976"/>
    <rdfs:domain rdf:resource="https://www.commoncoreontologies.org/ont00001175"/>
    <rdfs:range rdf:resource="https://www.commoncoreontologies.org/ont00000253"/>
    <rdfs:label xml:lang="en">language used in</rdfs:label>
    <skos:definition xml:lang="en">x language_used_by y iff y is an instance of Information Bearing Entity and x is an instance of Language, such that the literal value of y is a string that is encoded according to the syntax of x.</skos:definition>
    <cco:ont00001760 rdf:datatype="http://www.w3.org/2001/XMLSchema#anyURI">https://www.commoncoreontologies.org/InformationEntityOntology</cco:ont00001760>
  </rdf:Description>
  <rdf:Description rdf:about="https://www.commoncoreontologies.org/ont00002012">
    <rdf:type rdf:resource="http://www.w3.org/2002/07/owl#Class"/>
    <rdfs:subClassOf rdf:resource="https://www.commoncoreontologies.org/ont00002010"/>
    <rdfs:label xml:lang="en">Email Message</rdfs:label>
    <skos:definition xml:lang="en">A Message that is transmitted to the recipient's Email Box.</skos:definition>
    <cco:ont00001754 rdf:datatype="http://www.w3.org/2001/XMLSchema#anyURI">https://en.wikipedia.org/w/index.php?title=Email&amp;oldid=1063646749</cco:ont00001754>
    <cco:ont00001760 rdf:datatype="http://www.w3.org/2001/XMLSchema#anyURI">https://www.commoncoreontologies.org/InformationEntityOntology</cco:ont00001760>
  </rdf:Description>
  <rdf:Description rdf:about="https://www.commoncoreontologies.org/ont00001491">
    <rdf:type rdf:resource="http://www.w3.org/2002/07/owl#NamedIndividual"/>
    <rdf:type rdf:resource="https://www.commoncoreontologies.org/ont00000630"/>
    <rdfs:label xml:lang="en">Universal Time 1 A</rdfs:label>
    <cco:ont00001753>UT1A</cco:ont00001753>
    <cco:ont00001760 rdf:datatype="http://www.w3.org/2001/XMLSchema#anyURI">https://www.commoncoreontologies.org/InformationEntityOntology</cco:ont00001760>
  </rdf:Description>
  <rdf:Description rdf:about="https://www.commoncoreontologies.org/ont00002001">
    <rdf:type rdf:resource="http://www.w3.org/2002/07/owl#Class"/>
    <rdfs:subClassOf rdf:resource="https://www.commoncoreontologies.org/ont00000958"/>
    <rdfs:comment>By 'canonical', it is intended that the media format is of a commonly recognized format, such as mass media formats such as books, magazines, and journals, as well as digital media forms (e.g. ebooks), to include, too, file types, such as those recognized by the Internet Assigned Numbers Authority (IANA)'s Media Types standard [RFC2046].</rdfs:comment>
    <rdfs:label>Media Content Entity</rdfs:label>
    <skos:definition xml:lang="en">An information content entity presented in a canonical media format.</skos:definition>
    <cco:ont00001760 rdf:datatype="http://www.w3.org/2001/XMLSchema#anyURI">https://www.commoncoreontologies.org/InformationEntityOntology</cco:ont00001760>
  </rdf:Description>
  <rdf:Description rdf:about="https://www.commoncoreontologies.org/ont00002014">
    <rdf:type rdf:resource="http://www.w3.org/2002/07/owl#Class"/>
    <rdfs:subClassOf rdf:resource="https://www.commoncoreontologies.org/ont00002001"/>
    <rdfs:comment xml:lang="en">For information on types of barcodes, see: https://www.scandit.com/types-barcodes-choosing-right-barcode/</rdfs:comment>
    <rdfs:label xml:lang="en">Barcode</rdfs:label>
    <skos:definition xml:lang="en">A Media Content Entity that represents one or more geometric shapes that have, as part, some Directive Information Content Entity.</skos:definition>
    <cco:ont00001754 rdf:datatype="http://www.w3.org/2001/XMLSchema#anyURI">https://en.wikipedia.org/w/index.php?title=Barcode&amp;oldid=1059844765</cco:ont00001754>
    <cco:ont00001760 rdf:datatype="http://www.w3.org/2001/XMLSchema#anyURI">https://www.commoncoreontologies.org/InformationEntityOntology</cco:ont00001760>
  </rdf:Description>
  <rdf:Description rdf:about="https://www.commoncoreontologies.org/ont00001913">
    <rdf:type rdf:resource="http://www.w3.org/2002/07/owl#ObjectProperty"/>
    <rdfs:subPropertyOf rdf:resource="https://www.commoncoreontologies.org/ont00001912"/>
    <rdfs:domain rdf:resource="https://www.commoncoreontologies.org/ont00000253"/>
    <rdfs:range rdf:resource="https://www.commoncoreontologies.org/ont00000469"/>
    <rdfs:label xml:lang="en">uses geospatial coordinate reference system</rdfs:label>
    <skos:definition xml:lang="en">y uses_geospatial_coordinate_reference_system x iff y is an instance of Information Bearing Entity and x is an instance of Geospatial Coordinate Reference System, such that x describes the set of standards mentioned in y.</skos:definition>
    <cco:ont00001760 rdf:datatype="http://www.w3.org/2001/XMLSchema#anyURI">https://www.commoncoreontologies.org/InformationEntityOntology</cco:ont00001760>
  </rdf:Description>
  <rdf:Description rdf:about="https://www.commoncoreontologies.org/ont00002017">
    <rdf:type rdf:resource="http://www.w3.org/2002/07/owl#Class"/>
    <rdfs:subClassOf rdf:resource="https://www.commoncoreontologies.org/ont00002015"/>
    <rdfs:label xml:lang="en">Data Matrix Code</rdfs:label>
    <skos:definition xml:lang="en">A Two-Dimensional Barcode that represents cells arranged in rectangular patterns and is used for marking small items in logistics and operations.</skos:definition>
    <cco:ont00001760 rdf:datatype="http://www.w3.org/2001/XMLSchema#anyURI">https://www.commoncoreontologies.org/InformationEntityOntology</cco:ont00001760>
  </rdf:Description>
  <rdf:Description rdf:about="https://www.commoncoreontologies.org/ont00002026">
    <rdf:type rdf:resource="http://www.w3.org/2002/07/owl#Class"/>
    <rdfs:subClassOf rdf:resource="https://www.commoncoreontologies.org/ont00002025"/>
    <rdfs:label xml:lang="en">ISSN Barcode</rdfs:label>
    <skos:definition xml:lang="en">An EAN Barcode that is designed to designate a periodical.</skos:definition>
    <cco:ont00001760 rdf:datatype="http://www.w3.org/2001/XMLSchema#anyURI">https://www.commoncoreontologies.org/InformationEntityOntology</cco:ont00001760>
  </rdf:Description>
  <rdf:Description rdf:about="https://www.commoncoreontologies.org/ont00002021">
    <rdf:type rdf:resource="http://www.w3.org/2002/07/owl#Class"/>
    <rdfs:subClassOf rdf:resource="https://www.commoncoreontologies.org/ont00002020"/>
    <rdfs:label xml:lang="en">Codabar Barcode</rdfs:label>
    <skos:definition xml:lang="en">A One-Dimensional Barcode that represents numbers 0-9 and the characters -$:/.+ and is intended for use by logistics and healthcare professionals.</skos:definition>
    <cco:ont00001760 rdf:datatype="http://www.w3.org/2001/XMLSchema#anyURI">https://www.commoncoreontologies.org/InformationEntityOntology</cco:ont00001760>
  </rdf:Description>
  <rdf:Description rdf:about="https://www.commoncoreontologies.org/ont00000203">
    <rdf:type rdf:resource="http://www.w3.org/2002/07/owl#Class"/>
    <rdfs:subClassOf rdf:resource="https://www.commoncoreontologies.org/ont00000293"/>
    <rdfs:label xml:lang="en">Event Status Nominal Information Content Entity</rdfs:label>
    <skos:definition xml:lang="en">A Nominal Measurement Information Content Entity that is a measurement of the current state of a process.</skos:definition>
    <skos:example>proposed, approved, planned, in progress, completed, failed, or successful</skos:example>
    <cco:ont00001760 rdf:datatype="http://www.w3.org/2001/XMLSchema#anyURI">https://www.commoncoreontologies.org/InformationEntityOntology</cco:ont00001760>
  </rdf:Description>
  <rdf:Description rdf:about="https://www.commoncoreontologies.org/ont00001392">
    <rdf:type rdf:resource="http://www.w3.org/2002/07/owl#NamedIndividual"/>
    <rdf:type rdf:resource="https://www.commoncoreontologies.org/ont00001352"/>
    <rdfs:label xml:lang="en">GMT-8</rdfs:label>
    <skos:altLabel xml:lang="en">PST</skos:altLabel>
    <skos:altLabel xml:lang="en">Pacific Standard Time</skos:altLabel>
    <cco:ont00001760 rdf:datatype="http://www.w3.org/2001/XMLSchema#anyURI">https://www.commoncoreontologies.org/InformationEntityOntology</cco:ont00001760>
  </rdf:Description>
  <rdf:Description rdf:nodeID="na8580e9876f64da8bd2fccebf064ee6cb36">
    <rdf:type rdf:resource="http://www.w3.org/2002/07/owl#Restriction"/>
    <owl:onProperty rdf:resource="https://www.commoncoreontologies.org/ont00001916"/>
    <owl:someValuesFrom rdf:resource="http://purl.obolibrary.org/obo/BFO_0000001"/>
  </rdf:Description>
  <rdf:Description rdf:about="https://www.commoncoreontologies.org/ont00001101">
    <rdf:type rdf:resource="http://www.w3.org/2002/07/owl#Class"/>
    <rdfs:subClassOf rdf:resource="https://www.commoncoreontologies.org/ont00001176"/>
    <rdfs:label xml:lang="en">Interval Estimate Information Content Entity</rdfs:label>
    <skos:altLabel xml:lang="en">Interval Estimate</skos:altLabel>
    <skos:altLabel xml:lang="en">Interval Estimate Measurement Information Content Entity</skos:altLabel>
    <skos:definition xml:lang="en">An Estimate Information Content Entity that consists of an interval of possible (or probable) values for the measured entity.</skos:definition>
    <cco:ont00001760 rdf:datatype="http://www.w3.org/2001/XMLSchema#anyURI">https://www.commoncoreontologies.org/InformationEntityOntology</cco:ont00001760>
  </rdf:Description>
  <rdf:Description rdf:about="https://www.commoncoreontologies.org/ont00001069">
    <rdf:type rdf:resource="http://www.w3.org/2002/07/owl#Class"/>
    <owl:equivalentClass rdf:nodeID="na8580e9876f64da8bd2fccebf064ee6cb67"/>
    <rdfs:subClassOf rdf:resource="https://www.commoncoreontologies.org/ont00000958"/>
    <owl:disjointWith rdf:resource="https://www.commoncoreontologies.org/ont00001163"/>
    <rdfs:label xml:lang="en">Representational Information Content Entity</rdfs:label>
    <skos:definition xml:lang="en">An Information Content Entity that represents some Entity.</skos:definition>
    <skos:example>the content of a court transcript represents a courtroom proceeding</skos:example>
    <skos:example>the content of a photograph of the Statue of Liberty represents the Statue of Liberty</skos:example>
    <skos:example>the content of a video of a sporting event represents that sporting event</skos:example>
    <cco:ont00001760 rdf:datatype="http://www.w3.org/2001/XMLSchema#anyURI">https://www.commoncoreontologies.org/InformationEntityOntology</cco:ont00001760>
  </rdf:Description>
  <rdf:Description rdf:about="https://www.commoncoreontologies.org/ont00001963">
    <rdf:type rdf:resource="http://www.w3.org/2002/07/owl#ObjectProperty"/>
    <rdfs:subPropertyOf rdf:resource="https://www.commoncoreontologies.org/ont00001904"/>
    <rdfs:domain rdf:resource="http://purl.obolibrary.org/obo/BFO_0000001"/>
    <rdfs:range rdf:resource="https://www.commoncoreontologies.org/ont00001010"/>
    <rdfs:label xml:lang="en">is measured by ordinal</rdfs:label>
    <skos:definition xml:lang="en">x is_measured_by_ordinal y iff y is an instance of Ordinal Measurement Information Content Entity and x is an instance of Entity, such that y describes some attribute of x relative to a scale ordered by rank.</skos:definition>
    <cco:ont00001760 rdf:datatype="http://www.w3.org/2001/XMLSchema#anyURI">https://www.commoncoreontologies.org/InformationEntityOntology</cco:ont00001760>
  </rdf:Description>
  <rdf:Description rdf:about="https://www.commoncoreontologies.org/ont00002020">
    <rdf:type rdf:resource="http://www.w3.org/2002/07/owl#Class"/>
    <rdfs:subClassOf rdf:resource="https://www.commoncoreontologies.org/ont00002014"/>
    <rdfs:label xml:lang="en">One-Dimensional Barcode</rdfs:label>
    <skos:definition xml:lang="en">A Barcode that represents parallel lines of varying widths and spacing that concretize some Directive Information Content Entity.</skos:definition>
    <cco:ont00001760 rdf:datatype="http://www.w3.org/2001/XMLSchema#anyURI">https://www.commoncoreontologies.org/InformationEntityOntology</cco:ont00001760>
  </rdf:Description>
  <rdf:Description rdf:nodeID="na8580e9876f64da8bd2fccebf064ee6cb23">
    <owl:intersectionOf rdf:nodeID="na8580e9876f64da8bd2fccebf064ee6cb25"/>
    <rdf:type rdf:resource="http://www.w3.org/2002/07/owl#Class"/>
  </rdf:Description>
  <rdf:Description rdf:about="https://www.commoncoreontologies.org/ont00001468">
    <rdf:type rdf:resource="http://www.w3.org/2002/07/owl#NamedIndividual"/>
    <rdf:type rdf:resource="https://www.commoncoreontologies.org/ont00001352"/>
    <rdfs:label xml:lang="en">GMT+10</rdfs:label>
    <skos:altLabel xml:lang="en">AET</skos:altLabel>
    <skos:altLabel xml:lang="en">Australia Eastern Time</skos:altLabel>
    <cco:ont00001760 rdf:datatype="http://www.w3.org/2001/XMLSchema#anyURI">https://www.commoncoreontologies.org/InformationEntityOntology</cco:ont00001760>
  </rdf:Description>
  <rdf:Description rdf:about="https://www.commoncoreontologies.org/ont00000915">
    <rdf:type rdf:resource="http://www.w3.org/2002/07/owl#Class"/>
    <rdfs:subClassOf rdf:resource="https://www.commoncoreontologies.org/ont00000605"/>
    <rdfs:label xml:lang="en">Acronym</rdfs:label>
    <skos:definition xml:lang="en">An Abbreviated Name that combines the initial letters of a Designative Name and which is pronounced as a word.</skos:definition>
    <skos:example>Wi-Fi, ASCII, OPSEC</skos:example>
    <cco:ont00001760 rdf:datatype="http://www.w3.org/2001/XMLSchema#anyURI">https://www.commoncoreontologies.org/InformationEntityOntology</cco:ont00001760>
  </rdf:Description>
  <rdf:Description rdf:nodeID="na8580e9876f64da8bd2fccebf064ee6cb48">
    <rdf:type rdf:resource="http://www.w3.org/2002/07/owl#Restriction"/>
    <owl:onProperty rdf:resource="https://www.commoncoreontologies.org/ont00001982"/>
    <owl:someValuesFrom rdf:resource="http://purl.obolibrary.org/obo/BFO_0000001"/>
  </rdf:Description>
  <rdf:Description rdf:about="https://www.commoncoreontologies.org/ont00001900">
    <rdf:type rdf:resource="http://www.w3.org/2002/07/owl#ObjectProperty"/>
    <rdfs:subPropertyOf rdf:resource="https://www.commoncoreontologies.org/ont00001997"/>
    <owl:inverseOf rdf:resource="https://www.commoncoreontologies.org/ont00001913"/>
    <rdfs:domain rdf:resource="https://www.commoncoreontologies.org/ont00000469"/>
    <rdfs:range rdf:resource="https://www.commoncoreontologies.org/ont00000253"/>
    <rdfs:label xml:lang="en">is geospatial coordinate reference system of</rdfs:label>
    <skos:definition xml:lang="en">x is_geospatial_coordinate_reference_system_of y iff y is an instance of Information Bearing Entity and x is an instance of Geospatial Coordinate Reference System, such that x describes the set of standards mentioned in y.</skos:definition>
    <cco:ont00001760 rdf:datatype="http://www.w3.org/2001/XMLSchema#anyURI">https://www.commoncoreontologies.org/InformationEntityOntology</cco:ont00001760>
  </rdf:Description>
  <rdf:Description rdf:about="https://www.commoncoreontologies.org/ont00000973">
    <rdf:type rdf:resource="http://www.w3.org/2002/07/owl#Class"/>
    <rdfs:subClassOf rdf:resource="https://www.commoncoreontologies.org/ont00000827"/>
    <rdfs:label xml:lang="en">Decimal Time of Day Identifier</rdfs:label>
    <skos:altLabel xml:lang="en">Fractional Time of Day Identifier</skos:altLabel>
    <skos:definition xml:lang="en">A Time of Day Identifier that designates an approximate Temporal Instant that is part of some Day and is specified using a decimal value for the portion of the Day that preceded the Temporal Instant.</skos:definition>
    <cco:ont00001760 rdf:datatype="http://www.w3.org/2001/XMLSchema#anyURI">https://www.commoncoreontologies.org/InformationEntityOntology</cco:ont00001760>
  </rdf:Description>
  <rdf:Description rdf:about="https://www.commoncoreontologies.org/ont00002019">
    <rdf:type rdf:resource="http://www.w3.org/2002/07/owl#Class"/>
    <rdfs:subClassOf rdf:resource="https://www.commoncoreontologies.org/ont00002015"/>
    <rdfs:label xml:lang="en">PDF417 Code</rdfs:label>
    <skos:definition xml:lang="en">A Two-Dimensional Barcode that is used in applications that require the storage of huge amounts of data.</skos:definition>
    <cco:ont00001760 rdf:datatype="http://www.w3.org/2001/XMLSchema#anyURI">https://www.commoncoreontologies.org/InformationEntityOntology</cco:ont00001760>
  </rdf:Description>
  <rdf:Description rdf:nodeID="na8580e9876f64da8bd2fccebf064ee6cb56">
    <rdf:type rdf:resource="http://www.w3.org/2002/07/owl#Restriction"/>
    <owl:onProperty rdf:resource="https://www.commoncoreontologies.org/ont00001942"/>
    <owl:someValuesFrom rdf:resource="http://purl.obolibrary.org/obo/BFO_0000001"/>
  </rdf:Description>
  <rdf:Description rdf:about="https://www.commoncoreontologies.org/ont00000390">
    <rdf:type rdf:resource="http://www.w3.org/2002/07/owl#Class"/>
    <owl:equivalentClass rdf:nodeID="na8580e9876f64da8bd2fccebf064ee6cb19"/>
    <rdfs:subClassOf rdf:resource="https://www.commoncoreontologies.org/ont00000686"/>
    <rdfs:label xml:lang="en">Spatial Region Identifier</rdfs:label>
    <skos:definition xml:lang="en">A Designative Information Content Entity that designates some Spatial Region.</skos:definition>
    <cco:ont00001760 rdf:datatype="http://www.w3.org/2001/XMLSchema#anyURI">https://www.commoncoreontologies.org/InformationEntityOntology</cco:ont00001760>
  </rdf:Description>
  <rdf:Description rdf:about="https://www.commoncoreontologies.org/ont00001395">
    <rdf:type rdf:resource="http://www.w3.org/2002/07/owl#NamedIndividual"/>
    <rdf:type rdf:resource="https://www.commoncoreontologies.org/ont00001352"/>
    <rdfs:label xml:lang="en">GMT-3:30</rdfs:label>
    <skos:altLabel xml:lang="en">Newfoundland Standard Time</skos:altLabel>
    <cco:ont00001753>NST</cco:ont00001753>
    <cco:ont00001760 rdf:datatype="http://www.w3.org/2001/XMLSchema#anyURI">https://www.commoncoreontologies.org/InformationEntityOntology</cco:ont00001760>
  </rdf:Description>
  <rdf:Description rdf:about="https://www.commoncoreontologies.org/ont00000729">
    <rdf:type rdf:resource="http://www.w3.org/2002/07/owl#Class"/>
    <rdfs:subClassOf rdf:resource="https://www.commoncoreontologies.org/ont00000275"/>
    <rdfs:label xml:lang="en">Spherical Coordinate System</rdfs:label>
    <skos:definition xml:lang="en">A Spatial Reference System for three-dimensional spatial regions that identifies each point using an ordered triple of numerical coordinates that consist of the radial distance of the point of interest from a fixed origin, its polar angle measured from a fixed zenith direction, and the azimuth angle of its orthogonal projection measured from a fixed direction on a reference plane that passes through the origin and is orthogonal to the zenith.</skos:definition>
    <cco:ont00001754 rdf:datatype="http://www.w3.org/2001/XMLSchema#anyURI">https://en.wikipedia.org/w/index.php?title=Spherical_coordinate_system&amp;oldid=1061029174</cco:ont00001754>
    <cco:ont00001760 rdf:datatype="http://www.w3.org/2001/XMLSchema#anyURI">https://www.commoncoreontologies.org/InformationEntityOntology</cco:ont00001760>
  </rdf:Description>
  <rdf:Description rdf:about="https://www.commoncoreontologies.org/ont00001982">
    <rdf:type rdf:resource="http://www.w3.org/2002/07/owl#ObjectProperty"/>
    <rdfs:subPropertyOf rdf:resource="https://www.commoncoreontologies.org/ont00001808"/>
    <rdfs:domain rdf:resource="https://www.commoncoreontologies.org/ont00000853"/>
    <rdfs:range rdf:resource="http://purl.obolibrary.org/obo/BFO_0000001"/>
    <rdfs:comment xml:lang="en">It is possible that this relation should be a functional property, that is for all x, y, z if x describes y and x describes z then y = z. For example, if a financial report x describes the quarterly results of a company y and that same financial report describes the quarterly results of a company z, then it should be inferred that companies y and z are the same. We refrained from classifying the relation as a functional property on the concern that descriptions are multifaceted and so consequently it may be that the same report would contain descriptions of multiple entities.</rdfs:comment>
    <rdfs:label xml:lang="en">describes</rdfs:label>
    <skos:definition xml:lang="en">x describes y iff x is an instance of Descriptive Information Content Entity, and y is an instance of Entity, such that x is_about the characteristics that identify y.</skos:definition>
    <skos:example>the content of a newspaper article describes some current event</skos:example>
    <skos:example>the content of a visitor's log describes some facility visit</skos:example>
    <skos:example>the content of an accident report describes some accident</skos:example>
    <cco:ont00001760 rdf:datatype="http://www.w3.org/2001/XMLSchema#anyURI">https://www.commoncoreontologies.org/InformationEntityOntology</cco:ont00001760>
  </rdf:Description>
  <rdf:Description rdf:about="https://www.commoncoreontologies.org/ont00002029">
    <rdf:type rdf:resource="http://www.w3.org/2002/07/owl#Class"/>
    <rdfs:subClassOf rdf:resource="https://www.commoncoreontologies.org/ont00002025"/>
    <rdfs:label xml:lang="en">EAN-8 Barcode</rdfs:label>
    <skos:definition xml:lang="en">An EAN Barcode that represents 8 numerical digits and is used to designate products at the point of sale.</skos:definition>
    <cco:ont00001760 rdf:datatype="http://www.w3.org/2001/XMLSchema#anyURI">https://www.commoncoreontologies.org/InformationEntityOntology</cco:ont00001760>
  </rdf:Description>
  <rdf:Description rdf:about="https://www.commoncoreontologies.org/ont00001256">
    <rdf:type rdf:resource="http://www.w3.org/2002/07/owl#Class"/>
    <rdfs:subClassOf rdf:resource="https://www.commoncoreontologies.org/ont00001163"/>
    <rdfs:comment xml:lang="en">Note, the term 'accuracy' is avoided due to its ambiguity between: correctness-of-performance ('Reliability Measurement Information Content Entity'), correctness-of-information (see: 'Veracity Measurement Information Content Entity'), and adherance-to-expectations (see: 'Deviation Measurement Information Content Entity').</rdfs:comment>
    <rdfs:label xml:lang="en">Reliability Measurement Information Content Entity</rdfs:label>
    <skos:altLabel xml:lang="en">Accuracy of Process</skos:altLabel>
    <skos:altLabel xml:lang="en">Reliability Measurement</skos:altLabel>
    <skos:definition xml:lang="en">A Measurement Information Content Entity that is a measurement of the extent to which an entity can consistently produce an outcome.</skos:definition>
    <skos:scopeNote xml:lang="en">Reliability concerns both a measure of past performance and the expectation that future performance will conform to the range of past performances.</skos:scopeNote>
    <cco:ont00001754>https://en.wikipedia.org/wiki/Reliability_(statistics)</cco:ont00001754>
    <cco:ont00001760 rdf:datatype="http://www.w3.org/2001/XMLSchema#anyURI">https://www.commoncoreontologies.org/InformationEntityOntology</cco:ont00001760>
  </rdf:Description>
  <rdf:Description rdf:about="https://www.commoncoreontologies.org/ont00001769">
    <rdf:type rdf:resource="http://www.w3.org/2002/07/owl#DatatypeProperty"/>
    <rdfs:domain rdf:resource="https://www.commoncoreontologies.org/ont00000253"/>
    <rdfs:range rdf:resource="http://www.w3.org/2001/XMLSchema#decimal"/>
    <rdfs:label xml:lang="en">has decimal value</rdfs:label>
    <skos:definition xml:lang="en">A data property that has as its range a decimal value.</skos:definition>
    <cco:ont00001760 rdf:datatype="http://www.w3.org/2001/XMLSchema#anyURI">https://www.commoncoreontologies.org/InformationEntityOntology</cco:ont00001760>
  </rdf:Description>
  <rdf:Description rdf:about="https://www.commoncoreontologies.org/ont00000087">
    <rdf:type rdf:resource="http://www.w3.org/2002/07/owl#Class"/>
    <rdfs:subClassOf rdf:resource="https://www.commoncoreontologies.org/ont00000894"/>
    <rdfs:comment xml:lang="en">An Ordinal Date Identifier may or may not also contain a number indicating a specific Year. If both numbers are included, the ISO 8601 ordinal date format stipulates that the two numbers be formatted as YYYY-DDD or YYYYDDD where [YYYY] indicates a year and [DDD] is the day of that year, from 001 through 365 (or 366 in leap years).</rdfs:comment>
    <rdfs:label xml:lang="en">Ordinal Date Identifier</rdfs:label>
    <skos:altLabel xml:lang="en">Ordinal Date</skos:altLabel>
    <skos:definition xml:lang="en">A Decimal Date Identifier that designates some Day by using a number to indicate the sequential ordering of the Day since the beginning of the Year.</skos:definition>
    <cco:ont00001754 rdf:datatype="http://www.w3.org/2001/XMLSchema#anyURI">https://en.wikipedia.org/w/index.php?title=Ordinal_date&amp;oldid=1061989434</cco:ont00001754>
    <cco:ont00001760 rdf:datatype="http://www.w3.org/2001/XMLSchema#anyURI">https://www.commoncoreontologies.org/InformationEntityOntology</cco:ont00001760>
  </rdf:Description>
  <rdf:Description rdf:about="https://www.commoncoreontologies.org/ont00000080">
    <rdf:type rdf:resource="http://www.w3.org/2002/07/owl#Class"/>
    <rdfs:subClassOf rdf:resource="https://www.commoncoreontologies.org/ont00000827"/>
    <rdfs:label xml:lang="en">Standard Time of Day Identifier</rdfs:label>
    <skos:definition xml:lang="en">A Time of Day Identifier that designates an approximate Temporal Instant that is part of some Day and is specified using the Hours, Minutes, and Seconds of the Day that preceded the Temporal Instant.</skos:definition>
    <cco:ont00001760 rdf:datatype="http://www.w3.org/2001/XMLSchema#anyURI">https://www.commoncoreontologies.org/InformationEntityOntology</cco:ont00001760>
  </rdf:Description>
  <rdf:Description rdf:about="https://www.commoncoreontologies.org/ont00002038">
    <rdf:type rdf:resource="http://www.w3.org/2002/07/owl#Class"/>
    <rdfs:subClassOf rdf:resource="https://www.commoncoreontologies.org/ont00002001"/>
    <rdfs:subClassOf rdf:nodeID="na8580e9876f64da8bd2fccebf064ee6cb79"/>
    <rdfs:label xml:lang="en">Document Field Content</rdfs:label>
    <skos:altLabel xml:lang="en">Document Field</skos:altLabel>
    <skos:definition xml:lang="en">A Media Content Entity that is a part of some document content entity, and which  prescribes the eliciation of information to be written or selected within the document content entity.</skos:definition>
    <cco:ont00001760 rdf:datatype="http://www.w3.org/2001/XMLSchema#anyURI">https://www.commoncoreontologies.org/InformationEntityOntology</cco:ont00001760>
  </rdf:Description>
  <rdf:Description rdf:about="https://www.commoncoreontologies.org/ont00000419">
    <rdf:type rdf:resource="http://www.w3.org/2002/07/owl#Class"/>
    <rdfs:subClassOf rdf:resource="https://www.commoncoreontologies.org/ont00000077"/>
    <rdfs:label xml:lang="en">Part Number</rdfs:label>
    <skos:definition xml:lang="en">A Code Identifier that designates a type of part whose instances are designed to be part of some Artifact.</skos:definition>
    <cco:ont00001760 rdf:datatype="http://www.w3.org/2001/XMLSchema#anyURI">https://www.commoncoreontologies.org/InformationEntityOntology</cco:ont00001760>
  </rdf:Description>
  <rdf:Description rdf:nodeID="na8580e9876f64da8bd2fccebf064ee6cb71">
    <owl:intersectionOf rdf:nodeID="na8580e9876f64da8bd2fccebf064ee6cb73"/>
    <rdf:type rdf:resource="http://www.w3.org/2002/07/owl#Class"/>
  </rdf:Description>
  <rdf:Description rdf:nodeID="na8580e9876f64da8bd2fccebf064ee6cb38">
    <rdf:first rdf:nodeID="na8580e9876f64da8bd2fccebf064ee6cb36"/>
    <rdf:rest rdf:resource="http://www.w3.org/1999/02/22-rdf-syntax-ns#nil"/>
  </rdf:Description>
  <rdf:Description rdf:nodeID="na8580e9876f64da8bd2fccebf064ee6cb75">
    <owl:intersectionOf rdf:nodeID="na8580e9876f64da8bd2fccebf064ee6cb77"/>
    <rdf:type rdf:resource="http://www.w3.org/2002/07/owl#Class"/>
  </rdf:Description>
  <rdf:Description rdf:about="https://www.commoncoreontologies.org/ont00001938">
    <rdf:type rdf:resource="http://www.w3.org/2002/07/owl#ObjectProperty"/>
    <rdfs:subPropertyOf rdf:resource="https://www.commoncoreontologies.org/ont00001808"/>
    <rdfs:domain rdf:resource="https://www.commoncoreontologies.org/ont00000958"/>
    <rdfs:range rdf:resource="http://purl.obolibrary.org/obo/BFO_0000001"/>
    <rdfs:comment xml:lang="en">Isomorphism between the carrier of x and the represented entity can be via a direct similarity relation, e.g., grooves in a vinyl record corresponding to sound waves, or linguistic convention, e.g., a court stenographer's transcription of spoken words, as well as others, such as encoding processes for images.</rdfs:comment>
    <rdfs:label xml:lang="en">represents</rdfs:label>
    <skos:definition xml:lang="en">x represents y iff x is an instance of Information Content Entity, y is an instance of Entity, and z is carrier of x, such that x is about y in virtue of there existing an isomorphism between characteristics of z and y.</skos:definition>
    <skos:scopeNote xml:lang="en">Given a stronger temporal interpretation, this property may be functional. For more info please refer to https://github.com/BFO-ontology/BFO-2020/tree/master/src/owl/temporal%20extensions.</skos:scopeNote>
    <skos:scopeNote xml:lang="en">The relationship that is being defined here is that between the content of a photographic image and its object, between the content of a video and its objects and events, between the content of an audio recording and the sounds or events generating those sounds, or between the content of a written transcript and the verbal event that it transcribes.</skos:scopeNote>
    <cco:ont00001760 rdf:datatype="http://www.w3.org/2001/XMLSchema#anyURI">https://www.commoncoreontologies.org/InformationEntityOntology</cco:ont00001760>
  </rdf:Description>
  <rdf:Description rdf:about="https://www.commoncoreontologies.org/ont00000649">
    <rdf:type rdf:resource="http://www.w3.org/2002/07/owl#Class"/>
    <rdfs:subClassOf rdf:resource="https://www.commoncoreontologies.org/ont00000686"/>
    <rdfs:label xml:lang="en">Non-Name Identifier</rdfs:label>
    <skos:altLabel xml:lang="en">ID</skos:altLabel>
    <skos:altLabel xml:lang="en">Identifier</skos:altLabel>
    <skos:definition xml:lang="en">A Designative Information Content Entity that consists of a string of characters that designates an entity within a specified namespace or context, is not a Designative Name, may be automatically or randomly generated, and typically has no preexisting cultural or social significance.</skos:definition>
    <cco:ont00001760 rdf:datatype="http://www.w3.org/2001/XMLSchema#anyURI">https://www.commoncoreontologies.org/InformationEntityOntology</cco:ont00001760>
  </rdf:Description>
  <rdf:Description rdf:about="https://www.commoncoreontologies.org/ont00001771">
    <rdf:type rdf:resource="http://www.w3.org/2002/07/owl#DatatypeProperty"/>
    <rdfs:domain rdf:resource="https://www.commoncoreontologies.org/ont00000253"/>
    <rdfs:label xml:lang="en">has date value</rdfs:label>
    <skos:definition xml:lang="en">A data property that has as its range a date value.</skos:definition>
    <cco:ont00001760 rdf:datatype="http://www.w3.org/2001/XMLSchema#anyURI">https://www.commoncoreontologies.org/InformationEntityOntology</cco:ont00001760>
  </rdf:Description>
  <rdf:Description rdf:nodeID="na8580e9876f64da8bd2fccebf064ee6cb10">
    <owl:intersectionOf rdf:nodeID="na8580e9876f64da8bd2fccebf064ee6cb12"/>
    <rdf:type rdf:resource="http://www.w3.org/2002/07/owl#Class"/>
  </rdf:Description>
  <rdf:Description rdf:about="https://www.commoncoreontologies.org/ont00001582">
    <rdf:type rdf:resource="http://www.w3.org/2002/07/owl#NamedIndividual"/>
    <rdf:type rdf:resource="https://www.commoncoreontologies.org/ont00000469"/>
    <rdfs:label xml:lang="en">Universal Transverse Mercator Reference System</rdfs:label>
    <cco:ont00001753>UTM</cco:ont00001753>
    <cco:ont00001760 rdf:datatype="http://www.w3.org/2001/XMLSchema#anyURI">https://www.commoncoreontologies.org/InformationEntityOntology</cco:ont00001760>
  </rdf:Description>
  <rdf:Description rdf:about="https://www.commoncoreontologies.org/ont00001723">
    <rdf:type rdf:resource="http://www.w3.org/2002/07/owl#NamedIndividual"/>
    <rdf:type rdf:resource="https://www.commoncoreontologies.org/ont00001235"/>
    <rdfs:comment xml:lang="en">Offset from Universal Coordinated Time = UTC+4</rdfs:comment>
    <rdfs:label xml:lang="en">Delta Time Zone</rdfs:label>
    <cco:ont00001753>D</cco:ont00001753>
    <cco:ont00001760 rdf:datatype="http://www.w3.org/2001/XMLSchema#anyURI">https://www.commoncoreontologies.org/InformationEntityOntology</cco:ont00001760>
  </rdf:Description>
  <rdf:Description rdf:about="https://www.commoncoreontologies.org/ont00000630">
    <rdf:type rdf:resource="http://www.w3.org/2002/07/owl#Class"/>
    <rdfs:subClassOf rdf:resource="https://www.commoncoreontologies.org/ont00000124"/>
    <rdfs:label xml:lang="en">Universal Time Reference System</rdfs:label>
    <skos:definition xml:lang="en">A Solar Time Reference System that is based on the average speed of the Earth's rotation and which uses the prime meridian at 0 longitude as a reference point.</skos:definition>
    <cco:ont00001753>UT</cco:ont00001753>
    <cco:ont00001760 rdf:datatype="http://www.w3.org/2001/XMLSchema#anyURI">https://www.commoncoreontologies.org/InformationEntityOntology</cco:ont00001760>
  </rdf:Description>
  <rdf:Description rdf:about="https://www.commoncoreontologies.org/ont00000653">
    <rdf:type rdf:resource="http://www.w3.org/2002/07/owl#Class"/>
    <rdfs:subClassOf rdf:resource="https://www.commoncoreontologies.org/ont00000965"/>
    <rdfs:label xml:lang="en">Algorithm</rdfs:label>
    <skos:definition xml:lang="en">A Directive Information Content Entity that prescribes some Process and contains a finite sequence of unambiguous instructions in order to achieve some Objective.</skos:definition>
    <cco:ont00001754 rdf:datatype="http://www.w3.org/2001/XMLSchema#anyURI">http://purl.obolibrary.org/obo/IAO_0000064</cco:ont00001754>
    <cco:ont00001760 rdf:datatype="http://www.w3.org/2001/XMLSchema#anyURI">https://www.commoncoreontologies.org/InformationEntityOntology</cco:ont00001760>
  </rdf:Description>
  <rdf:Description rdf:nodeID="na8580e9876f64da8bd2fccebf064ee6cb6">
    <rdf:type rdf:resource="http://www.w3.org/2002/07/owl#Restriction"/>
    <owl:onProperty rdf:resource="https://www.commoncoreontologies.org/ont00001916"/>
    <owl:someValuesFrom rdf:resource="http://purl.obolibrary.org/obo/BFO_0000038"/>
  </rdf:Description>
  <rdf:Description rdf:about="https://www.commoncoreontologies.org/ont00000891">
    <rdf:type rdf:resource="http://www.w3.org/2002/07/owl#Class"/>
    <rdfs:subClassOf rdf:resource="https://www.commoncoreontologies.org/ont00001328"/>
    <rdfs:label xml:lang="en">Calendar System</rdfs:label>
    <skos:definition xml:lang="en">A Temporal Reference System that is designed to organize and identify dates.</skos:definition>
    <skos:scopeNote xml:lang="en">Calendars typically organize dates through the use of naming and temporal conventions based on Days, Weeks, Months, and Years.</skos:scopeNote>
    <cco:ont00001760 rdf:datatype="http://www.w3.org/2001/XMLSchema#anyURI">https://www.commoncoreontologies.org/InformationEntityOntology</cco:ont00001760>
  </rdf:Description>
  <rdf:Description rdf:about="https://www.commoncoreontologies.org/ont00001661">
    <rdf:type rdf:resource="http://www.w3.org/2002/07/owl#NamedIndividual"/>
    <rdf:type rdf:resource="https://www.commoncoreontologies.org/ont00001352"/>
    <rdfs:label xml:lang="en">GMT+8</rdfs:label>
    <skos:altLabel xml:lang="en">CTT</skos:altLabel>
    <skos:altLabel xml:lang="en">China Taiwan Time</skos:altLabel>
    <cco:ont00001760 rdf:datatype="http://www.w3.org/2001/XMLSchema#anyURI">https://www.commoncoreontologies.org/InformationEntityOntology</cco:ont00001760>
  </rdf:Description>
  <rdf:Description rdf:nodeID="na8580e9876f64da8bd2fccebf064ee6cb72">
    <rdf:type rdf:resource="http://www.w3.org/2002/07/owl#Restriction"/>
    <owl:onProperty rdf:resource="https://www.commoncoreontologies.org/ont00001966"/>
    <owl:someValuesFrom rdf:resource="http://purl.obolibrary.org/obo/BFO_0000001"/>
  </rdf:Description>
  <rdf:Description rdf:nodeID="na8580e9876f64da8bd2fccebf064ee6cb55">
    <owl:intersectionOf rdf:nodeID="na8580e9876f64da8bd2fccebf064ee6cb57"/>
    <rdf:type rdf:resource="http://www.w3.org/2002/07/owl#Class"/>
  </rdf:Description>
  <rdf:Description rdf:nodeID="na8580e9876f64da8bd2fccebf064ee6cb73">
    <rdf:first rdf:resource="https://www.commoncoreontologies.org/ont00000853"/>
    <rdf:rest rdf:nodeID="na8580e9876f64da8bd2fccebf064ee6cb74"/>
  </rdf:Description>
  <rdf:Description rdf:about="https://www.commoncoreontologies.org/ont00002042">
    <rdf:type rdf:resource="http://www.w3.org/2002/07/owl#Class"/>
    <rdfs:subClassOf rdf:resource="https://www.commoncoreontologies.org/ont00002039"/>
    <rdfs:label xml:lang="en">Spreadsheet</rdfs:label>
    <skos:definition xml:lang="en">A Document Content Entity that canonically appears as a interactive, tabular form.</skos:definition>
    <cco:ont00001754 rdf:datatype="http://www.w3.org/2001/XMLSchema#anyURI">https://en.wikipedia.org/w/index.php?title=Spreadsheet&amp;oldid=1064060503</cco:ont00001754>
    <cco:ont00001760 rdf:datatype="http://www.w3.org/2001/XMLSchema#anyURI">https://www.commoncoreontologies.org/InformationEntityOntology</cco:ont00001760>
  </rdf:Description>
  <rdf:Description rdf:about="https://www.commoncoreontologies.org/ont00001712">
    <rdf:type rdf:resource="http://www.w3.org/2002/07/owl#NamedIndividual"/>
    <rdf:type rdf:resource="https://www.commoncoreontologies.org/ont00001235"/>
    <rdfs:comment xml:lang="en">Offset from Universal Coordinated Time = UTC-5</rdfs:comment>
    <rdfs:label xml:lang="en">Romeo Time Zone</rdfs:label>
    <cco:ont00001753>R</cco:ont00001753>
    <cco:ont00001760 rdf:datatype="http://www.w3.org/2001/XMLSchema#anyURI">https://www.commoncoreontologies.org/InformationEntityOntology</cco:ont00001760>
  </rdf:Description>
  <rdf:Description rdf:about="https://www.commoncoreontologies.org/ont00001773">
    <rdf:type rdf:resource="http://www.w3.org/2002/07/owl#DatatypeProperty"/>
    <rdfs:domain rdf:resource="https://www.commoncoreontologies.org/ont00000253"/>
    <rdfs:range rdf:resource="http://www.w3.org/2001/XMLSchema#integer"/>
    <rdfs:label xml:lang="en">has integer value</rdfs:label>
    <skos:definition xml:lang="en">A data property that has as its range an integer value.</skos:definition>
    <cco:ont00001760 rdf:datatype="http://www.w3.org/2001/XMLSchema#anyURI">https://www.commoncoreontologies.org/InformationEntityOntology</cco:ont00001760>
  </rdf:Description>
  <rdf:Description rdf:about="https://www.commoncoreontologies.org/ont00000749">
    <rdf:type rdf:resource="http://www.w3.org/2002/07/owl#Class"/>
    <rdfs:subClassOf rdf:resource="https://www.commoncoreontologies.org/ont00000894"/>
    <rdfs:subClassOf rdf:nodeID="na8580e9876f64da8bd2fccebf064ee6cb39"/>
    <rdfs:label xml:lang="en">Julian Day Number</rdfs:label>
    <skos:definition xml:lang="en">A Decimal Date Identifier that designates some Julian Day by using a number to indicate the sequential ordering of the Day since the Julian Date epoch.</skos:definition>
    <cco:ont00001760 rdf:datatype="http://www.w3.org/2001/XMLSchema#anyURI">https://www.commoncoreontologies.org/InformationEntityOntology</cco:ont00001760>
  </rdf:Description>
  <rdf:Description rdf:about="https://www.commoncoreontologies.org/ont00001175">
    <rdf:type rdf:resource="http://www.w3.org/2002/07/owl#Class"/>
    <rdfs:subClassOf rdf:resource="https://www.commoncoreontologies.org/ont00000965"/>
    <rdfs:label xml:lang="en">Language</rdfs:label>
    <skos:definition xml:lang="en">A Directive Information Content Entity that prescribes a canonical format for communication.</skos:definition>
    <cco:ont00001760 rdf:datatype="http://www.w3.org/2001/XMLSchema#anyURI">https://www.commoncoreontologies.org/InformationEntityOntology</cco:ont00001760>
  </rdf:Description>
  <rdf:Description rdf:about="https://www.commoncoreontologies.org/ont00001417">
    <rdf:type rdf:resource="http://www.w3.org/2002/07/owl#NamedIndividual"/>
    <rdf:type rdf:resource="https://www.commoncoreontologies.org/ont00001328"/>
    <rdfs:comment xml:lang="en">ET is an astronomical time scale that was adopted as a standard in 1952 by the IAU but has since been superseded and is no longer actively used. ET is based on the ephemeris second, which was defined as a fraction of the tropical year for 1900 January 01 as calculated using Newcomb's 1895 tables of the Sun. ET was designed to avoid problems caused by variations in Earth's rotational period and was used for Solar System ephemeris calculations until being replaced by Terrestrial Dynamical Time (TDT) in 1979.</rdfs:comment>
    <rdfs:label xml:lang="en">Ephemeris Time</rdfs:label>
    <cco:ont00001753>ET</cco:ont00001753>
    <cco:ont00001760 rdf:datatype="http://www.w3.org/2001/XMLSchema#anyURI">https://www.commoncoreontologies.org/InformationEntityOntology</cco:ont00001760>
  </rdf:Description>
  <rdf:Description rdf:nodeID="na8580e9876f64da8bd2fccebf064ee6cb30">
    <rdf:first rdf:nodeID="na8580e9876f64da8bd2fccebf064ee6cb28"/>
    <rdf:rest rdf:resource="http://www.w3.org/1999/02/22-rdf-syntax-ns#nil"/>
  </rdf:Description>
  <rdf:Description rdf:nodeID="na8580e9876f64da8bd2fccebf064ee6cb50">
    <rdf:first rdf:nodeID="na8580e9876f64da8bd2fccebf064ee6cb48"/>
    <rdf:rest rdf:resource="http://www.w3.org/1999/02/22-rdf-syntax-ns#nil"/>
  </rdf:Description>
  <rdf:Description rdf:about="https://www.commoncoreontologies.org/ont00001965">
    <rdf:type rdf:resource="http://www.w3.org/2002/07/owl#ObjectProperty"/>
    <rdfs:subPropertyOf rdf:resource="https://www.commoncoreontologies.org/ont00001904"/>
    <owl:inverseOf rdf:resource="https://www.commoncoreontologies.org/ont00001983"/>
    <rdfs:domain rdf:resource="http://purl.obolibrary.org/obo/BFO_0000001"/>
    <rdfs:range rdf:resource="https://www.commoncoreontologies.org/ont00001022"/>
    <rdfs:label xml:lang="en">is measured by ratio</rdfs:label>
    <skos:definition xml:lang="en">y is_measured_by_ratio x iff x is an instance of Ratio Measurement Information Content Entity and y is an instance of Entity, such that x describes some attribute of y relative to a scale having equal unit values and a zero value that corresponds to the absence of the attribute being measured.</skos:definition>
    <cco:ont00001760 rdf:datatype="http://www.w3.org/2001/XMLSchema#anyURI">https://www.commoncoreontologies.org/InformationEntityOntology</cco:ont00001760>
  </rdf:Description>
  <rdf:Description rdf:about="https://www.commoncoreontologies.org/ont00001328">
    <rdf:type rdf:resource="http://www.w3.org/2002/07/owl#Class"/>
    <rdfs:subClassOf rdf:resource="https://www.commoncoreontologies.org/ont00000398"/>
    <rdfs:label xml:lang="en">Temporal Reference System</rdfs:label>
    <skos:altLabel xml:lang="en">Temporal Reference Frame</skos:altLabel>
    <skos:altLabel xml:lang="en">Time Scale</skos:altLabel>
    <skos:definition xml:lang="en">A Reference System that describes a set of standards for measuring time as well as understanding the context of and organizing temporal data.</skos:definition>
    <cco:ont00001760 rdf:datatype="http://www.w3.org/2001/XMLSchema#anyURI">https://www.commoncoreontologies.org/InformationEntityOntology</cco:ont00001760>
  </rdf:Description>
  <rdf:Description rdf:about="https://www.commoncoreontologies.org/ont00000406">
    <rdf:type rdf:resource="http://www.w3.org/2002/07/owl#Class"/>
    <rdfs:subClassOf rdf:resource="https://www.commoncoreontologies.org/ont00000120"/>
    <rdfs:label xml:lang="en">Measurement Unit of Geocoordinate</rdfs:label>
    <skos:definition xml:lang="en">A Measurement Unit specifying the geospatial coordinates of a location.</skos:definition>
    <cco:ont00001760 rdf:datatype="http://www.w3.org/2001/XMLSchema#anyURI">https://www.commoncoreontologies.org/InformationEntityOntology</cco:ont00001760>
  </rdf:Description>
  <rdf:Description rdf:about="https://www.commoncoreontologies.org/ont00001727">
    <rdf:type rdf:resource="http://www.w3.org/2002/07/owl#NamedIndividual"/>
    <rdf:type rdf:resource="https://www.commoncoreontologies.org/ont00001235"/>
    <rdfs:comment xml:lang="en">Offset from Universal Coordinated Time = UTC+10</rdfs:comment>
    <rdfs:label xml:lang="en">Kilo Time Zone</rdfs:label>
    <cco:ont00001753>K</cco:ont00001753>
    <cco:ont00001760 rdf:datatype="http://www.w3.org/2001/XMLSchema#anyURI">https://www.commoncoreontologies.org/InformationEntityOntology</cco:ont00001760>
  </rdf:Description>
  <rdf:Description rdf:about="https://www.commoncoreontologies.org/ont00001584">
    <rdf:type rdf:resource="http://www.w3.org/2002/07/owl#NamedIndividual"/>
    <rdf:type rdf:resource="https://www.commoncoreontologies.org/ont00000469"/>
    <rdfs:label xml:lang="en">World Geographic Reference System</rdfs:label>
    <cco:ont00001753>WGRS</cco:ont00001753>
    <cco:ont00001760 rdf:datatype="http://www.w3.org/2001/XMLSchema#anyURI">https://www.commoncoreontologies.org/InformationEntityOntology</cco:ont00001760>
  </rdf:Description>
  <rdf:Description rdf:about="https://www.commoncoreontologies.org/ont00000894">
    <rdf:type rdf:resource="http://www.w3.org/2002/07/owl#Class"/>
    <rdfs:subClassOf rdf:resource="https://www.commoncoreontologies.org/ont00000529"/>
    <rdfs:label xml:lang="en">Decimal Date Identifier</rdfs:label>
    <skos:definition xml:lang="en">A Date Identifier that designates some Day by using a number to indicate the sequential ordering of the Day since a specified Reference Time.</skos:definition>
    <cco:ont00001760 rdf:datatype="http://www.w3.org/2001/XMLSchema#anyURI">https://www.commoncoreontologies.org/InformationEntityOntology</cco:ont00001760>
  </rdf:Description>
  <rdf:Description rdf:about="https://www.commoncoreontologies.org/ont00000605">
    <rdf:type rdf:resource="http://www.w3.org/2002/07/owl#Class"/>
    <rdfs:subClassOf rdf:resource="https://www.commoncoreontologies.org/ont00000003"/>
    <rdfs:label xml:lang="en">Abbreviated Name</rdfs:label>
    <skos:definition xml:lang="en">A Designative Name that is a shortened form of a Proper Name.</skos:definition>
    <cco:ont00001760 rdf:datatype="http://www.w3.org/2001/XMLSchema#anyURI">https://www.commoncoreontologies.org/InformationEntityOntology</cco:ont00001760>
  </rdf:Description>
  <rdf:Description rdf:about="https://www.commoncoreontologies.org/ont00002025">
    <rdf:type rdf:resource="http://www.w3.org/2002/07/owl#Class"/>
    <rdfs:subClassOf rdf:resource="https://www.commoncoreontologies.org/ont00002020"/>
    <rdfs:label xml:lang="en">EAN Barcode</rdfs:label>
    <skos:definition xml:lang="en">A One-Dimensional Barcode that represents 8 or 13 numerical digits and is used to scan consumer goods.</skos:definition>
    <cco:ont00001760 rdf:datatype="http://www.w3.org/2001/XMLSchema#anyURI">https://www.commoncoreontologies.org/InformationEntityOntology</cco:ont00001760>
  </rdf:Description>
  <rdf:Description rdf:about="https://www.commoncoreontologies.org/ont00001961">
    <rdf:type rdf:resource="http://www.w3.org/2002/07/owl#ObjectProperty"/>
    <rdfs:subPropertyOf rdf:resource="http://purl.obolibrary.org/obo/BFO_0000084"/>
    <rdfs:domain rdf:resource="https://www.commoncoreontologies.org/ont00000120"/>
    <rdfs:range rdf:resource="https://www.commoncoreontologies.org/ont00000253"/>
    <rdfs:label xml:lang="en">is measurement unit of</rdfs:label>
    <skos:definition xml:lang="en">x is_measurement_unit_of y iff y is an instance of Information Bearing Entity and x is an instance of Measurement Unit, such that x describes the magnitude of measured physical quantity mentioned in y.</skos:definition>
    <cco:ont00001760 rdf:datatype="http://www.w3.org/2001/XMLSchema#anyURI">https://www.commoncoreontologies.org/InformationEntityOntology</cco:ont00001760>
  </rdf:Description>
  <rdf:Description rdf:about="https://www.commoncoreontologies.org/ont00001732">
    <rdf:type rdf:resource="http://www.w3.org/2002/07/owl#NamedIndividual"/>
    <rdf:type rdf:resource="https://www.commoncoreontologies.org/ont00001235"/>
    <rdfs:comment xml:lang="en">Offset from Universal Coordinated Time = UTC+3</rdfs:comment>
    <rdfs:label xml:lang="en">Charlie Time Zone</rdfs:label>
    <cco:ont00001753>C</cco:ont00001753>
    <cco:ont00001760 rdf:datatype="http://www.w3.org/2001/XMLSchema#anyURI">https://www.commoncoreontologies.org/InformationEntityOntology</cco:ont00001760>
  </rdf:Description>
  <rdf:Description rdf:about="https://www.commoncoreontologies.org/ont00001753">
    <rdf:type rdf:resource="http://www.w3.org/2002/07/owl#AnnotationProperty"/>
  </rdf:Description>
  <rdf:Description rdf:nodeID="na8580e9876f64da8bd2fccebf064ee6cb49">
    <rdf:first rdf:resource="https://www.commoncoreontologies.org/ont00000958"/>
    <rdf:rest rdf:nodeID="na8580e9876f64da8bd2fccebf064ee6cb50"/>
  </rdf:Description>
  <rdf:Description rdf:about="https://www.commoncoreontologies.org/ont00000965">
    <rdf:type rdf:resource="http://www.w3.org/2002/07/owl#Class"/>
    <owl:equivalentClass rdf:nodeID="na8580e9876f64da8bd2fccebf064ee6cb55"/>
    <rdfs:subClassOf rdf:resource="https://www.commoncoreontologies.org/ont00000958"/>
    <rdfs:label xml:lang="en">Prescriptive Information Content Entity</rdfs:label>
    <skos:altLabel xml:lang="en">Directive ICE</skos:altLabel>
    <skos:definition xml:lang="en">An Information Content Entity that consists of a set of propositions or images (as in the case of a blueprint) that prescribe some Entity.</skos:definition>
    <cco:ont00001760 rdf:datatype="http://www.w3.org/2001/XMLSchema#anyURI">https://www.commoncoreontologies.org/InformationEntityOntology</cco:ont00001760>
  </rdf:Description>
  <rdf:Description rdf:about="https://www.commoncoreontologies.org/ont00001580">
    <rdf:type rdf:resource="http://www.w3.org/2002/07/owl#NamedIndividual"/>
    <rdf:type rdf:resource="https://www.commoncoreontologies.org/ont00001235"/>
    <rdfs:comment xml:lang="en">Offset from Universal Coordinated Time = UTC-3</rdfs:comment>
    <rdfs:label xml:lang="en">Papa Time Zone</rdfs:label>
    <cco:ont00001753>P</cco:ont00001753>
    <cco:ont00001760 rdf:datatype="http://www.w3.org/2001/XMLSchema#anyURI">https://www.commoncoreontologies.org/InformationEntityOntology</cco:ont00001760>
  </rdf:Description>
  <rdf:Description rdf:about="https://www.commoncoreontologies.org/ont00000127">
    <rdf:type rdf:resource="http://www.w3.org/2002/07/owl#Class"/>
    <rdfs:subClassOf rdf:resource="https://www.commoncoreontologies.org/ont00000965"/>
    <rdfs:subClassOf rdf:nodeID="na8580e9876f64da8bd2fccebf064ee6cb9"/>
    <rdfs:label xml:lang="en">Performance Specification</rdfs:label>
    <skos:definition xml:lang="en">A Directive Information Content Entity that prescribes some aspect of the behavior of a participant in a Process given one or more operating conditions.</skos:definition>
    <skos:example>Maximum Speed at high altitude; Rate of Ascent at 10 degrees celsius with nominal payload.</skos:example>
    <cco:ont00001760 rdf:datatype="http://www.w3.org/2001/XMLSchema#anyURI">https://www.commoncoreontologies.org/InformationEntityOntology</cco:ont00001760>
  </rdf:Description>
  <rdf:Description rdf:about="https://www.commoncoreontologies.org/ont00000186">
    <rdf:type rdf:resource="http://www.w3.org/2002/07/owl#Class"/>
    <rdfs:subClassOf rdf:resource="https://www.commoncoreontologies.org/ont00001010"/>
    <rdfs:label xml:lang="en">Artifact Version Ordinality</rdfs:label>
    <skos:definition xml:lang="en">An Ordinal Measurement Information Content Entity that is about the form of an Artifact which differs in some respects from previous or future forms of that Artifact.</skos:definition>
    <cco:ont00001760 rdf:datatype="http://www.w3.org/2001/XMLSchema#anyURI">https://www.commoncoreontologies.org/InformationEntityOntology</cco:ont00001760>
  </rdf:Description>
  <rdf:Description rdf:about="https://www.commoncoreontologies.org/ont00001920">
    <rdf:type rdf:resource="http://www.w3.org/2002/07/owl#ObjectProperty"/>
    <rdfs:subPropertyOf rdf:resource="https://www.commoncoreontologies.org/ont00001801"/>
    <owl:inverseOf rdf:resource="https://www.commoncoreontologies.org/ont00001942"/>
    <rdfs:domain rdf:resource="http://purl.obolibrary.org/obo/BFO_0000001"/>
    <rdfs:range rdf:resource="https://www.commoncoreontologies.org/ont00000965"/>
    <rdfs:label xml:lang="en">prescribed by</rdfs:label>
    <skos:definition xml:lang="en">x prescribed_by y iff y is an instance of Directive Information Content Entity and x is an instance of Entity and y prescribes x.</skos:definition>
    <cco:ont00001760 rdf:datatype="http://www.w3.org/2001/XMLSchema#anyURI">https://www.commoncoreontologies.org/InformationEntityOntology</cco:ont00001760>
  </rdf:Description>
  <rdf:Description rdf:nodeID="na8580e9876f64da8bd2fccebf064ee6cb60">
    <rdf:type rdf:resource="http://www.w3.org/2002/07/owl#Restriction"/>
    <owl:onProperty rdf:resource="https://www.commoncoreontologies.org/ont00001811"/>
    <owl:someValuesFrom rdf:resource="http://purl.obolibrary.org/obo/BFO_0000001"/>
  </rdf:Description>
  <rdf:Description rdf:about="https://www.commoncoreontologies.org/ont00001014">
    <rdf:type rdf:resource="http://www.w3.org/2002/07/owl#Class"/>
    <rdfs:subClassOf rdf:resource="https://www.commoncoreontologies.org/ont00000003"/>
    <rdfs:label xml:lang="en">Proper Name</rdfs:label>
    <skos:definition xml:lang="en">A Designative Name that is an official name for a particular entity.</skos:definition>
    <cco:ont00001760 rdf:datatype="http://www.w3.org/2001/XMLSchema#anyURI">https://www.commoncoreontologies.org/InformationEntityOntology</cco:ont00001760>
  </rdf:Description>
  <rdf:Description rdf:about="https://www.commoncoreontologies.org/ont00001537">
    <rdf:type rdf:resource="http://www.w3.org/2002/07/owl#NamedIndividual"/>
    <rdf:type rdf:resource="https://www.commoncoreontologies.org/ont00000067"/>
    <rdf:type rdf:resource="https://www.commoncoreontologies.org/ont00000630"/>
    <rdfs:comment xml:lang="en">UTC is a variant of Universal Time that is calculated by combining Universal Time 1 with International Atomic Time by occasionally adding leap seconds to TAI in order to maintain UTC within 0.9 seconds of UT1. The difference between UTC and UT1 is called DUT1 and always has a value between -0.9 seconds and +0.9 seconds. Coordinated Universal Time is the current basis for civil time and is the reference time for time zones, whose local times are defined based on an offset from UTC.</rdfs:comment>
    <rdfs:label xml:lang="en">Coordinated Universal Time</rdfs:label>
    <cco:ont00001753>UTC</cco:ont00001753>
    <cco:ont00001760 rdf:datatype="http://www.w3.org/2001/XMLSchema#anyURI">https://www.commoncoreontologies.org/InformationEntityOntology</cco:ont00001760>
  </rdf:Description>
  <rdf:Description rdf:about="https://www.commoncoreontologies.org/ont00001837">
    <rdf:type rdf:resource="http://www.w3.org/2002/07/owl#ObjectProperty"/>
    <rdfs:subPropertyOf rdf:resource="http://purl.obolibrary.org/obo/BFO_0000084"/>
    <owl:inverseOf rdf:resource="https://www.commoncoreontologies.org/ont00001908"/>
    <rdfs:domain rdf:resource="https://www.commoncoreontologies.org/ont00000829"/>
    <rdfs:range rdf:resource="https://www.commoncoreontologies.org/ont00000253"/>
    <rdfs:label xml:lang="en">time zone identifier used by</rdfs:label>
    <skos:definition xml:lang="en">x time_zone_identifier_used_by y iff y is an instance of Information Bearing Entity and x is an instance of Time Zone Identifier, such that x designates the spatial region associated with the time zone mentioned in y.</skos:definition>
    <cco:ont00001760 rdf:datatype="http://www.w3.org/2001/XMLSchema#anyURI">https://www.commoncoreontologies.org/InformationEntityOntology</cco:ont00001760>
  </rdf:Description>
  <rdf:Description rdf:about="https://www.commoncoreontologies.org/ont00000073">
    <rdf:type rdf:resource="http://www.w3.org/2002/07/owl#Class"/>
    <owl:equivalentClass rdf:nodeID="na8580e9876f64da8bd2fccebf064ee6cb5"/>
    <rdfs:subClassOf rdf:resource="https://www.commoncoreontologies.org/ont00000399"/>
    <rdfs:label xml:lang="en">Temporal Interval Identifier</rdfs:label>
    <skos:altLabel xml:lang="en">One-Dimensional Temporal Region Identifier</skos:altLabel>
    <skos:definition xml:lang="en">A Temporal Region Identifier that designates some Temporal Interval.</skos:definition>
    <cco:ont00001760 rdf:datatype="http://www.w3.org/2001/XMLSchema#anyURI">https://www.commoncoreontologies.org/InformationEntityOntology</cco:ont00001760>
  </rdf:Description>
  <rdf:Description rdf:about="https://www.commoncoreontologies.org/ont00000275">
    <rdf:type rdf:resource="http://www.w3.org/2002/07/owl#Class"/>
    <rdfs:subClassOf rdf:resource="https://www.commoncoreontologies.org/ont00000398"/>
    <rdfs:comment xml:lang="en">Note that, while reference systems and reference frames are treated as synonyms here, some people treat them as related but separate entities. See: http://www.ggos-portal.org/lang_en/GGOS-Portal/EN/Topics/GeodeticApplications/GeodeticReferenceSystemsAndFrames/GeodeticReferenceSystemsAndFrames.html</rdfs:comment>
    <rdfs:label xml:lang="en">Spatial Reference System</rdfs:label>
    <skos:altLabel xml:lang="en">Coordinate System</skos:altLabel>
    <skos:altLabel xml:lang="en">Spatial Coordinate System</skos:altLabel>
    <skos:altLabel xml:lang="en">Spatial Reference Frame</skos:altLabel>
    <skos:definition xml:lang="en">A Reference System that describes a set of standards for uniquely identifying the position of an entity or the direction of a vector within a defined spatial region by means of measurements along one or more Coordinate System Axes.</skos:definition>
    <cco:ont00001754 rdf:datatype="http://www.w3.org/2001/XMLSchema#anyURI">https://en.wikipedia.org/w/index.php?title=Coordinate_system&amp;oldid=1060461397</cco:ont00001754>
    <cco:ont00001760 rdf:datatype="http://www.w3.org/2001/XMLSchema#anyURI">https://www.commoncoreontologies.org/InformationEntityOntology</cco:ont00001760>
  </rdf:Description>
  <rdf:Description rdf:nodeID="na8580e9876f64da8bd2fccebf064ee6cb13">
    <rdf:first rdf:nodeID="na8580e9876f64da8bd2fccebf064ee6cb11"/>
    <rdf:rest rdf:resource="http://www.w3.org/1999/02/22-rdf-syntax-ns#nil"/>
  </rdf:Description>
  <rdf:Description rdf:about="https://www.commoncoreontologies.org/ont00002031">
    <rdf:type rdf:resource="http://www.w3.org/2002/07/owl#Class"/>
    <rdfs:subClassOf rdf:resource="https://www.commoncoreontologies.org/ont00002020"/>
    <rdfs:comment xml:lang="en">Further variants of GS1 DataBar have not been defined here.</rdfs:comment>
    <rdfs:label xml:lang="en">GS1 DataBar Barcode</rdfs:label>
    <skos:definition xml:lang="en">A One-Dimensional Barcode that represents 12-14 numerical digits and is used in retail and healthcare.</skos:definition>
    <cco:ont00001760 rdf:datatype="http://www.w3.org/2001/XMLSchema#anyURI">https://www.commoncoreontologies.org/InformationEntityOntology</cco:ont00001760>
  </rdf:Description>
  <rdf:Description rdf:about="https://www.commoncoreontologies.org/ont00002010">
    <rdf:type rdf:resource="http://www.w3.org/2002/07/owl#Class"/>
    <rdfs:subClassOf rdf:resource="https://www.commoncoreontologies.org/ont00002001"/>
    <rdfs:label xml:lang="en">Message</rdfs:label>
    <skos:definition xml:lang="en">A Media Content Entity that is relatively brief and designed to be transmitted from a sender to a recipient.</skos:definition>
    <cco:ont00001754 rdf:datatype="http://www.w3.org/2001/XMLSchema#anyURI">https://en.wikipedia.org/w/index.php?title=Message&amp;oldid=1060098631</cco:ont00001754>
    <cco:ont00001760 rdf:datatype="http://www.w3.org/2001/XMLSchema#anyURI">https://www.commoncoreontologies.org/InformationEntityOntology</cco:ont00001760>
  </rdf:Description>
  <rdf:Description rdf:about="https://www.commoncoreontologies.org/ont00001983">
    <rdf:type rdf:resource="http://www.w3.org/2002/07/owl#ObjectProperty"/>
    <rdfs:subPropertyOf rdf:resource="https://www.commoncoreontologies.org/ont00001966"/>
    <rdfs:domain rdf:resource="https://www.commoncoreontologies.org/ont00001022"/>
    <rdfs:range rdf:resource="http://purl.obolibrary.org/obo/BFO_0000001"/>
    <rdfs:label xml:lang="en">is a ratio measurement of</rdfs:label>
    <skos:definition xml:lang="en">x is_a_ratio_measurement_of y iff x is an instance of Ratio Measurement Information Content Entity and y is an instance of Entity and x describes some attribute of y relative to a scale having equal unit values and a zero value that corresponds to the absence of the attribute being measured.</skos:definition>
    <cco:ont00001760 rdf:datatype="http://www.w3.org/2001/XMLSchema#anyURI">https://www.commoncoreontologies.org/InformationEntityOntology</cco:ont00001760>
  </rdf:Description>
  <rdf:Description rdf:nodeID="na8580e9876f64da8bd2fccebf064ee6cb15">
    <rdf:type rdf:resource="http://www.w3.org/2002/07/owl#Restriction"/>
    <owl:onProperty rdf:resource="https://www.commoncoreontologies.org/ont00001868"/>
    <owl:someValuesFrom rdf:resource="http://purl.obolibrary.org/obo/BFO_0000001"/>
  </rdf:Description>
  <rdf:Description rdf:about="https://www.commoncoreontologies.org/ont00001772">
    <rdf:type rdf:resource="http://www.w3.org/2002/07/owl#DatatypeProperty"/>
    <rdfs:domain rdf:resource="https://www.commoncoreontologies.org/ont00000253"/>
    <rdfs:range rdf:resource="http://www.w3.org/2001/XMLSchema#boolean"/>
    <rdfs:label xml:lang="en">has boolean value</rdfs:label>
    <skos:definition xml:lang="en">A data property that has as its range a boolean value.</skos:definition>
    <cco:ont00001760 rdf:datatype="http://www.w3.org/2001/XMLSchema#anyURI">https://www.commoncoreontologies.org/InformationEntityOntology</cco:ont00001760>
  </rdf:Description>
  <rdf:Description rdf:about="https://www.commoncoreontologies.org/ont00002040">
    <rdf:type rdf:resource="http://www.w3.org/2002/07/owl#Class"/>
    <rdfs:subClassOf rdf:resource="https://www.commoncoreontologies.org/ont00002039"/>
    <rdfs:label xml:lang="en">Book</rdfs:label>
    <skos:definition xml:lang="en">A Document Content Entity that canonically appears as ink on paper or parchment, or other materials fastened together to hinge at one side.</skos:definition>
    <cco:ont00001754 rdf:datatype="http://www.w3.org/2001/XMLSchema#anyURI">https://en.wikipedia.org/w/index.php?title=Book&amp;oldid=1063132471</cco:ont00001754>
    <cco:ont00001760 rdf:datatype="http://www.w3.org/2001/XMLSchema#anyURI">https://www.commoncoreontologies.org/InformationEntityOntology</cco:ont00001760>
  </rdf:Description>
  <rdf:Description rdf:about="https://www.commoncoreontologies.org/ont00001877">
    <rdf:type rdf:resource="http://www.w3.org/2002/07/owl#ObjectProperty"/>
    <rdfs:subPropertyOf rdf:resource="https://www.commoncoreontologies.org/ont00001966"/>
    <owl:inverseOf rdf:resource="https://www.commoncoreontologies.org/ont00001964"/>
    <rdfs:domain rdf:resource="https://www.commoncoreontologies.org/ont00001364"/>
    <rdfs:range rdf:resource="http://purl.obolibrary.org/obo/BFO_0000001"/>
    <rdfs:label xml:lang="en">is an interval measurement of</rdfs:label>
    <skos:definition xml:lang="en">x is_an_interval_measurement_of y iff x is an instance of Information Content Entity and y is an instance of Entity and y is_measured_by_interval x.</skos:definition>
    <skos:example>a measurement of air temperature on the Celsius scale.</skos:example>
    <cco:ont00001760 rdf:datatype="http://www.w3.org/2001/XMLSchema#anyURI">https://www.commoncoreontologies.org/InformationEntityOntology</cco:ont00001760>
  </rdf:Description>
  <rdf:Description rdf:about="https://www.commoncoreontologies.org/ont00000369">
    <rdf:type rdf:resource="http://www.w3.org/2002/07/owl#Class"/>
    <rdfs:subClassOf rdf:resource="https://www.commoncoreontologies.org/ont00001010"/>
    <rdfs:label xml:lang="en">Priority Measurement Information Content Entity</rdfs:label>
    <skos:altLabel xml:lang="en">Criticality Measurement</skos:altLabel>
    <skos:altLabel xml:lang="en">Importance Measurement</skos:altLabel>
    <skos:altLabel xml:lang="en">Priority Measurement</skos:altLabel>
    <skos:definition xml:lang="en">An Ordinal Measurement Information Content Entity that is a measurement of the relative importance of an entity.</skos:definition>
    <skos:example>low, normal, high, urgent, or immediate priority</skos:example>
    <cco:ont00001760 rdf:datatype="http://www.w3.org/2001/XMLSchema#anyURI">https://www.commoncoreontologies.org/InformationEntityOntology</cco:ont00001760>
  </rdf:Description>
  <rdf:Description rdf:nodeID="na8580e9876f64da8bd2fccebf064ee6cb47">
    <owl:intersectionOf rdf:nodeID="na8580e9876f64da8bd2fccebf064ee6cb49"/>
    <rdf:type rdf:resource="http://www.w3.org/2002/07/owl#Class"/>
  </rdf:Description>
  <rdf:Description rdf:about="https://www.commoncoreontologies.org/ont00001424">
    <rdf:type rdf:resource="http://www.w3.org/2002/07/owl#NamedIndividual"/>
    <rdf:type rdf:resource="https://www.commoncoreontologies.org/ont00001235"/>
    <rdfs:comment xml:lang="en">Offset from Universal Coordinated Time = UTC+1</rdfs:comment>
    <rdfs:label xml:lang="en">Alpha Time Zone</rdfs:label>
    <cco:ont00001753>A</cco:ont00001753>
    <cco:ont00001760 rdf:datatype="http://www.w3.org/2001/XMLSchema#anyURI">https://www.commoncoreontologies.org/InformationEntityOntology</cco:ont00001760>
  </rdf:Description>
  <rdf:Description rdf:about="https://www.commoncoreontologies.org/ont00002024">
    <rdf:type rdf:resource="http://www.w3.org/2002/07/owl#Class"/>
    <rdfs:subClassOf rdf:resource="https://www.commoncoreontologies.org/ont00002020"/>
    <rdfs:label xml:lang="en">MSI Plessey Barcode</rdfs:label>
    <skos:definition xml:lang="en">A One-Dimensional Barcode that represents an indefinite number of numerical characters and is used for inventory control and marking storage containers and shelves in warehouse environments.</skos:definition>
    <cco:ont00001760 rdf:datatype="http://www.w3.org/2001/XMLSchema#anyURI">https://www.commoncoreontologies.org/InformationEntityOntology</cco:ont00001760>
  </rdf:Description>
  <rdf:Description rdf:about="https://www.commoncoreontologies.org/ont00001440">
    <rdf:type rdf:resource="http://www.w3.org/2002/07/owl#NamedIndividual"/>
    <rdf:type rdf:resource="https://www.commoncoreontologies.org/ont00001352"/>
    <rdfs:label xml:lang="en">GMT-9</rdfs:label>
    <skos:altLabel xml:lang="en">AST</skos:altLabel>
    <skos:altLabel xml:lang="en">Alaska Standard Time</skos:altLabel>
    <cco:ont00001760 rdf:datatype="http://www.w3.org/2001/XMLSchema#anyURI">https://www.commoncoreontologies.org/InformationEntityOntology</cco:ont00001760>
  </rdf:Description>
  <rdf:Description rdf:nodeID="na8580e9876f64da8bd2fccebf064ee6cb19">
    <owl:intersectionOf rdf:nodeID="na8580e9876f64da8bd2fccebf064ee6cb21"/>
    <rdf:type rdf:resource="http://www.w3.org/2002/07/owl#Class"/>
  </rdf:Description>
  <rdf:Description rdf:about="https://www.commoncoreontologies.org/ont00001476">
    <rdf:type rdf:resource="http://www.w3.org/2002/07/owl#NamedIndividual"/>
    <rdf:type rdf:resource="https://www.commoncoreontologies.org/ont00001352"/>
    <rdfs:label xml:lang="en">GMT+4</rdfs:label>
    <skos:altLabel xml:lang="en">NET</skos:altLabel>
    <skos:altLabel xml:lang="en">Near East Time</skos:altLabel>
    <cco:ont00001760 rdf:datatype="http://www.w3.org/2001/XMLSchema#anyURI">https://www.commoncoreontologies.org/InformationEntityOntology</cco:ont00001760>
  </rdf:Description>
  <rdf:Description rdf:about="https://www.commoncoreontologies.org/ont00001534">
    <rdf:type rdf:resource="http://www.w3.org/2002/07/owl#NamedIndividual"/>
    <rdf:type rdf:resource="https://www.commoncoreontologies.org/ont00001352"/>
    <rdfs:label xml:lang="en">GMT+7</rdfs:label>
    <skos:altLabel xml:lang="en">VST</skos:altLabel>
    <skos:altLabel xml:lang="en">Vietnam Standard Time</skos:altLabel>
    <cco:ont00001760 rdf:datatype="http://www.w3.org/2001/XMLSchema#anyURI">https://www.commoncoreontologies.org/InformationEntityOntology</cco:ont00001760>
  </rdf:Description>
  <rdf:Description rdf:nodeID="na8580e9876f64da8bd2fccebf064ee6cb57">
    <rdf:first rdf:resource="https://www.commoncoreontologies.org/ont00000958"/>
    <rdf:rest rdf:nodeID="na8580e9876f64da8bd2fccebf064ee6cb58"/>
  </rdf:Description>
  <rdf:Description rdf:about="https://www.commoncoreontologies.org/ont00000120">
    <rdf:type rdf:resource="http://www.w3.org/2002/07/owl#Class"/>
    <rdfs:subClassOf rdf:resource="https://www.commoncoreontologies.org/ont00000853"/>
    <rdfs:label xml:lang="en">Measurement Unit</rdfs:label>
    <skos:definition xml:lang="en">A Descriptive Information Content Entity that describes a definite magnitude of a physical quantity, defined and adopted by convention and/or by law, that is used as a standard for measurement of the same physical quantity.</skos:definition>
    <cco:ont00001754 rdf:datatype="http://www.w3.org/2001/XMLSchema#anyURI">https://en.wikipedia.org/w/index.php?title=Unit_of_measurement&amp;oldid=1061038125</cco:ont00001754>
    <cco:ont00001760 rdf:datatype="http://www.w3.org/2001/XMLSchema#anyURI">https://www.commoncoreontologies.org/InformationEntityOntology</cco:ont00001760>
  </rdf:Description>
  <rdf:Description rdf:about="https://www.commoncoreontologies.org/ont00001041">
    <rdf:type rdf:resource="http://www.w3.org/2002/07/owl#Class"/>
    <rdfs:subClassOf rdf:resource="https://www.commoncoreontologies.org/ont00001010"/>
    <rdfs:label xml:lang="en">Sequence Position Ordinality</rdfs:label>
    <skos:definition xml:lang="en">An Ordinal Measurement Information Content Entity that is about the position of some entity in some ordered sequence.</skos:definition>
    <cco:ont00001760 rdf:datatype="http://www.w3.org/2001/XMLSchema#anyURI">https://www.commoncoreontologies.org/InformationEntityOntology</cco:ont00001760>
  </rdf:Description>
  <rdf:Description rdf:about="https://www.commoncoreontologies.org/ont00001412">
    <rdf:type rdf:resource="http://www.w3.org/2002/07/owl#NamedIndividual"/>
    <rdf:type rdf:resource="https://www.commoncoreontologies.org/ont00001352"/>
    <rdfs:comment xml:lang="en">Offset from Universal Coordinated Time = UTC+0</rdfs:comment>
    <rdfs:label xml:lang="en">GMT</rdfs:label>
    <skos:altLabel xml:lang="en">Greenwich Mean Time</skos:altLabel>
    <cco:ont00001760 rdf:datatype="http://www.w3.org/2001/XMLSchema#anyURI">https://www.commoncoreontologies.org/InformationEntityOntology</cco:ont00001760>
  </rdf:Description>
  <rdf:Description rdf:about="https://www.commoncoreontologies.org/ont00001553">
    <rdf:type rdf:resource="http://www.w3.org/2002/07/owl#NamedIndividual"/>
    <rdf:type rdf:resource="https://www.commoncoreontologies.org/ont00001352"/>
    <rdfs:label xml:lang="en">GMT+6</rdfs:label>
    <skos:altLabel xml:lang="en">BST</skos:altLabel>
    <skos:altLabel xml:lang="en">Bangladesh Standard Time</skos:altLabel>
    <cco:ont00001760 rdf:datatype="http://www.w3.org/2001/XMLSchema#anyURI">https://www.commoncoreontologies.org/InformationEntityOntology</cco:ont00001760>
  </rdf:Description>
  <rdf:Description rdf:nodeID="na8580e9876f64da8bd2fccebf064ee6cb5">
    <owl:intersectionOf rdf:nodeID="na8580e9876f64da8bd2fccebf064ee6cb7"/>
    <rdf:type rdf:resource="http://www.w3.org/2002/07/owl#Class"/>
  </rdf:Description>
  <rdf:Description rdf:about="https://www.commoncoreontologies.org/ont00001457">
    <rdf:type rdf:resource="http://www.w3.org/2002/07/owl#NamedIndividual"/>
    <rdf:type rdf:resource="https://www.commoncoreontologies.org/ont00001235"/>
    <rdfs:comment xml:lang="en">Offset from Universal Coordinated Time = UTC-4</rdfs:comment>
    <rdfs:label xml:lang="en">Quebec Time Zone</rdfs:label>
    <cco:ont00001753>Q</cco:ont00001753>
    <cco:ont00001760 rdf:datatype="http://www.w3.org/2001/XMLSchema#anyURI">https://www.commoncoreontologies.org/InformationEntityOntology</cco:ont00001760>
  </rdf:Description>
  <rdf:Description rdf:nodeID="na8580e9876f64da8bd2fccebf064ee6cb45">
    <rdf:type rdf:resource="http://www.w3.org/2002/07/owl#Restriction"/>
    <owl:onProperty rdf:resource="http://purl.obolibrary.org/obo/BFO_0000178"/>
    <owl:someValuesFrom rdf:resource="https://www.commoncoreontologies.org/ont00000749"/>
  </rdf:Description>
  <rdf:Description rdf:about="https://www.commoncoreontologies.org/ont00000496">
    <rdf:type rdf:resource="http://www.w3.org/2002/07/owl#Class"/>
    <rdfs:subClassOf rdf:resource="https://www.commoncoreontologies.org/ont00001175"/>
    <rdfs:label xml:lang="en">Natural Language</rdfs:label>
    <skos:definition xml:lang="en">A Language that is developed and evolves through use and repetition, rather than through conscious planning or premeditation.</skos:definition>
    <skos:example>English</skos:example>
    <skos:example>Mandarin (Chinese)</skos:example>
    <skos:example>Spanish</skos:example>
    <cco:ont00001754 rdf:datatype="http://www.w3.org/2001/XMLSchema#anyURI">https://en.wikipedia.org/w/index.php?title=Natural_language&amp;oldid=1060890461</cco:ont00001754>
    <cco:ont00001760 rdf:datatype="http://www.w3.org/2001/XMLSchema#anyURI">https://www.commoncoreontologies.org/InformationEntityOntology</cco:ont00001760>
  </rdf:Description>
  <rdf:Description rdf:about="https://www.commoncoreontologies.org/ont00001548">
    <rdf:type rdf:resource="http://www.w3.org/2002/07/owl#NamedIndividual"/>
    <rdf:type rdf:resource="https://www.commoncoreontologies.org/ont00000630"/>
    <rdfs:comment xml:lang="en">UT1R is a variant of Universal Time that is a smoothed version of UT1 by filtering out periodic variations due to tidal waves.</rdfs:comment>
    <rdfs:label xml:lang="en">Universal Time 1 R</rdfs:label>
    <cco:ont00001753>UT1R</cco:ont00001753>
    <cco:ont00001760 rdf:datatype="http://www.w3.org/2001/XMLSchema#anyURI">https://www.commoncoreontologies.org/InformationEntityOntology</cco:ont00001760>
  </rdf:Description>
  <rdf:Description rdf:nodeID="na8580e9876f64da8bd2fccebf064ee6cb33">
    <rdf:first rdf:resource="https://www.commoncoreontologies.org/ont00000399"/>
    <rdf:rest rdf:nodeID="na8580e9876f64da8bd2fccebf064ee6cb34"/>
  </rdf:Description>
  <rdf:Description rdf:about="https://www.commoncoreontologies.org/ont00000692">
    <rdf:type rdf:resource="http://www.w3.org/2002/07/owl#Class"/>
    <rdfs:subClassOf rdf:resource="https://www.commoncoreontologies.org/ont00001163"/>
    <rdfs:comment xml:lang="en">Every probability measurement is made within a particular context given certain background assumptions.</rdfs:comment>
    <rdfs:label xml:lang="en">Probability Measurement Information Content Entity</rdfs:label>
    <skos:altLabel xml:lang="en">Likelihood Measurement</skos:altLabel>
    <skos:altLabel xml:lang="en">Probability Measurement</skos:altLabel>
    <skos:definition xml:lang="en">A Measurement Information Content Entity that is a measurement of the likelihood that a Process or Process Aggregate occurs.</skos:definition>
    <cco:ont00001754 rdf:datatype="http://www.w3.org/2001/XMLSchema#anyURI">https://en.wikipedia.org/w/index.php?title=Probability&amp;oldid=1059657543</cco:ont00001754>
    <cco:ont00001760 rdf:datatype="http://www.w3.org/2001/XMLSchema#anyURI">https://www.commoncoreontologies.org/InformationEntityOntology</cco:ont00001760>
  </rdf:Description>
  <rdf:Description rdf:nodeID="na8580e9876f64da8bd2fccebf064ee6cb35">
    <owl:intersectionOf rdf:nodeID="na8580e9876f64da8bd2fccebf064ee6cb37"/>
    <rdf:type rdf:resource="http://www.w3.org/2002/07/owl#Class"/>
  </rdf:Description>
  <rdf:Description rdf:about="https://www.commoncoreontologies.org/ont00001624">
    <rdf:type rdf:resource="http://www.w3.org/2002/07/owl#NamedIndividual"/>
    <rdf:type rdf:resource="https://www.commoncoreontologies.org/ont00001235"/>
    <rdfs:comment xml:lang="en">Offset from Universal Coordinated Time = UTC+7</rdfs:comment>
    <rdfs:label xml:lang="en">Golf Time Zone</rdfs:label>
    <cco:ont00001753>G</cco:ont00001753>
    <cco:ont00001760 rdf:datatype="http://www.w3.org/2001/XMLSchema#anyURI">https://www.commoncoreontologies.org/InformationEntityOntology</cco:ont00001760>
  </rdf:Description>
  <rdf:Description rdf:about="https://www.commoncoreontologies.org/ont00000540">
    <rdf:type rdf:resource="http://www.w3.org/2002/07/owl#Class"/>
    <owl:equivalentClass rdf:nodeID="na8580e9876f64da8bd2fccebf064ee6cb31"/>
    <rdfs:subClassOf rdf:resource="https://www.commoncoreontologies.org/ont00000399"/>
    <rdfs:label xml:lang="en">Temporal Instant Identifier</rdfs:label>
    <skos:altLabel xml:lang="en">Zero-Dimensional Temporal Region Identifier</skos:altLabel>
    <skos:definition xml:lang="en">A Temporal Region Identifier that designates some Temporal Instant.</skos:definition>
    <cco:ont00001760 rdf:datatype="http://www.w3.org/2001/XMLSchema#anyURI">https://www.commoncoreontologies.org/InformationEntityOntology</cco:ont00001760>
  </rdf:Description>
  <rdf:Description rdf:about="https://www.commoncoreontologies.org/ont00001529">
    <rdf:type rdf:resource="http://www.w3.org/2002/07/owl#NamedIndividual"/>
    <rdf:type rdf:resource="https://www.commoncoreontologies.org/ont00001328"/>
    <rdfs:comment xml:lang="en">"TCG is a coordinate time standard intended to be used as the independent variable of time for all calculations pertaining to precession, nutation, the Moon, and artificial satellites of the Earth. It is equivalent to the proper time experienced by a clock at rest in a coordinate frame co-moving with the center of the Earth: that is, a clock that performs exactly the same movements as the Earth but is outside the Earth's gravity well. It is therefore not influenced by the gravitational time dilation caused by the Earth."
From: (https://en.wikipedia.org/wiki/Geocentric_Coordinate_Time)</rdfs:comment>
    <rdfs:label xml:lang="en">Geocentric Coordinate Time</rdfs:label>
    <cco:ont00001753>TCG</cco:ont00001753>
    <cco:ont00001760 rdf:datatype="http://www.w3.org/2001/XMLSchema#anyURI">https://www.commoncoreontologies.org/InformationEntityOntology</cco:ont00001760>
  </rdf:Description>
  <rdf:Description rdf:nodeID="na8580e9876f64da8bd2fccebf064ee6cb62">
    <rdf:first rdf:nodeID="na8580e9876f64da8bd2fccebf064ee6cb60"/>
    <rdf:rest rdf:resource="http://www.w3.org/1999/02/22-rdf-syntax-ns#nil"/>
  </rdf:Description>
  <rdf:Description rdf:nodeID="na8580e9876f64da8bd2fccebf064ee6cb29">
    <rdf:first rdf:resource="https://www.commoncoreontologies.org/ont00000073"/>
    <rdf:rest rdf:nodeID="na8580e9876f64da8bd2fccebf064ee6cb30"/>
  </rdf:Description>
  <rdf:Description rdf:about="https://www.commoncoreontologies.org/ont00002009">
    <rdf:type rdf:resource="http://www.w3.org/2002/07/owl#Class"/>
    <rdfs:subClassOf rdf:resource="https://www.commoncoreontologies.org/ont00002001"/>
    <rdfs:label xml:lang="en">Video</rdfs:label>
    <skos:definition xml:lang="en">A Media Content Entity that contains a sequence of representations that are presented sufficiently rapidly to create the appearance of motion and continuity.</skos:definition>
    <cco:ont00001754 rdf:datatype="http://www.w3.org/2001/XMLSchema#anyURI">https://en.wikipedia.org/w/index.php?title=Video&amp;oldid=1049376249</cco:ont00001754>
    <cco:ont00001760 rdf:datatype="http://www.w3.org/2001/XMLSchema#anyURI">https://www.commoncoreontologies.org/InformationEntityOntology</cco:ont00001760>
  </rdf:Description>
  <rdf:Description rdf:about="https://www.commoncoreontologies.org/ont00002030">
    <rdf:type rdf:resource="http://www.w3.org/2002/07/owl#Class"/>
    <rdfs:subClassOf rdf:resource="https://www.commoncoreontologies.org/ont00002025"/>
    <rdfs:label xml:lang="en">ISBN Barcode</rdfs:label>
    <skos:definition xml:lang="en">An EAN Barcode that is designed to designate a book.</skos:definition>
    <cco:ont00001760 rdf:datatype="http://www.w3.org/2001/XMLSchema#anyURI">https://www.commoncoreontologies.org/InformationEntityOntology</cco:ont00001760>
  </rdf:Description>
  <rdf:Description rdf:about="https://www.commoncoreontologies.org/ont00002015">
    <rdf:type rdf:resource="http://www.w3.org/2002/07/owl#Class"/>
    <rdfs:subClassOf rdf:resource="https://www.commoncoreontologies.org/ont00002014"/>
    <rdfs:label xml:lang="en">Two-Dimensional Barcode</rdfs:label>
    <skos:definition xml:lang="en">A Barcode that represents lines of varying widths, spacing, height, and color that has, as part, some Directive Information Content Entity.</skos:definition>
    <cco:ont00001760 rdf:datatype="http://www.w3.org/2001/XMLSchema#anyURI">https://www.commoncoreontologies.org/InformationEntityOntology</cco:ont00001760>
  </rdf:Description>
  <rdf:Description rdf:about="https://www.commoncoreontologies.org/ont00001597">
    <rdf:type rdf:resource="http://www.w3.org/2002/07/owl#NamedIndividual"/>
    <rdf:type rdf:resource="https://www.commoncoreontologies.org/ont00001352"/>
    <rdfs:label xml:lang="en">GMT+11</rdfs:label>
    <skos:altLabel xml:lang="en">SST</skos:altLabel>
    <skos:altLabel xml:lang="en">Solomon Standard Time</skos:altLabel>
    <cco:ont00001760 rdf:datatype="http://www.w3.org/2001/XMLSchema#anyURI">https://www.commoncoreontologies.org/InformationEntityOntology</cco:ont00001760>
  </rdf:Description>
  <rdf:Description rdf:about="https://www.commoncoreontologies.org/ont00001634">
    <rdf:type rdf:resource="http://www.w3.org/2002/07/owl#NamedIndividual"/>
    <rdf:type rdf:resource="https://www.commoncoreontologies.org/ont00001352"/>
    <rdfs:label xml:lang="en">GMT-1</rdfs:label>
    <skos:altLabel xml:lang="en">CAT</skos:altLabel>
    <skos:altLabel xml:lang="en">Central African Time</skos:altLabel>
    <cco:ont00001760 rdf:datatype="http://www.w3.org/2001/XMLSchema#anyURI">https://www.commoncoreontologies.org/InformationEntityOntology</cco:ont00001760>
  </rdf:Description>
  <rdf:Description rdf:nodeID="na8580e9876f64da8bd2fccebf064ee6cb34">
    <rdf:first rdf:nodeID="na8580e9876f64da8bd2fccebf064ee6cb32"/>
    <rdf:rest rdf:resource="http://www.w3.org/1999/02/22-rdf-syntax-ns#nil"/>
  </rdf:Description>
  <rdf:Description rdf:nodeID="na8580e9876f64da8bd2fccebf064ee6cb2">
    <rdf:first rdf:resource="http://purl.obolibrary.org/obo/BFO_0000176"/>
    <rdf:rest rdf:resource="http://www.w3.org/1999/02/22-rdf-syntax-ns#nil"/>
  </rdf:Description>
  <rdf:Description rdf:nodeID="na8580e9876f64da8bd2fccebf064ee6cb46">
    <rdf:type rdf:resource="http://www.w3.org/2002/07/owl#Restriction"/>
    <owl:onProperty rdf:resource="https://www.commoncoreontologies.org/ont00001916"/>
    <owl:someValuesFrom rdf:resource="https://www.commoncoreontologies.org/ont00000359"/>
  </rdf:Description>
  <rdf:Description rdf:nodeID="na8580e9876f64da8bd2fccebf064ee6cb44">
    <rdf:type rdf:resource="http://www.w3.org/2002/07/owl#Restriction"/>
    <owl:onProperty rdf:resource="http://purl.obolibrary.org/obo/BFO_0000178"/>
    <owl:someValuesFrom rdf:resource="https://www.commoncoreontologies.org/ont00000589"/>
  </rdf:Description>
  <rdf:Description rdf:about="https://www.commoncoreontologies.org/ont00002011">
    <rdf:type rdf:resource="http://www.w3.org/2002/07/owl#Class"/>
    <rdfs:subClassOf rdf:resource="https://www.commoncoreontologies.org/ont00002010"/>
    <rdfs:label xml:lang="en">Warning Message</rdfs:label>
    <skos:definition xml:lang="en">A Message that describes a possible or impending threat.</skos:definition>
    <cco:ont00001760 rdf:datatype="http://www.w3.org/2001/XMLSchema#anyURI">https://www.commoncoreontologies.org/InformationEntityOntology</cco:ont00001760>
  </rdf:Description>
  <rdf:Description rdf:about="https://www.commoncoreontologies.org/ont00001434">
    <rdf:type rdf:resource="http://www.w3.org/2002/07/owl#NamedIndividual"/>
    <rdf:type rdf:resource="https://www.commoncoreontologies.org/ont00001352"/>
    <rdfs:label xml:lang="en">GMT+1</rdfs:label>
    <skos:altLabel xml:lang="en">ECT</skos:altLabel>
    <skos:altLabel xml:lang="en">European Central Time</skos:altLabel>
    <cco:ont00001760 rdf:datatype="http://www.w3.org/2001/XMLSchema#anyURI">https://www.commoncoreontologies.org/InformationEntityOntology</cco:ont00001760>
  </rdf:Description>
  <rdf:Description rdf:about="https://www.commoncoreontologies.org/ont00001904">
    <rdf:type rdf:resource="http://www.w3.org/2002/07/owl#ObjectProperty"/>
    <rdfs:subPropertyOf rdf:resource="https://www.commoncoreontologies.org/ont00001917"/>
    <owl:inverseOf rdf:resource="https://www.commoncoreontologies.org/ont00001966"/>
    <rdfs:domain rdf:resource="http://purl.obolibrary.org/obo/BFO_0000001"/>
    <rdfs:range rdf:resource="https://www.commoncoreontologies.org/ont00001163"/>
    <rdfs:label xml:lang="en">is measured by</rdfs:label>
    <skos:definition xml:lang="en">y is_measured_by x iff x is an instance of Measurement Information Content Entity and y is an instance of Entity and y is_a_measurement_of x.</skos:definition>
    <cco:ont00001760 rdf:datatype="http://www.w3.org/2001/XMLSchema#anyURI">https://www.commoncoreontologies.org/InformationEntityOntology</cco:ont00001760>
  </rdf:Description>
  <rdf:Description rdf:about="https://www.commoncoreontologies.org/ont00002045">
    <rdf:type rdf:resource="http://www.w3.org/2002/07/owl#Class"/>
    <rdfs:subClassOf rdf:resource="https://www.commoncoreontologies.org/ont00002039"/>
    <rdfs:label xml:lang="en">Journal Article</rdfs:label>
    <skos:definition xml:lang="en">A Document Content Entity that is part of a Journal Issue.</skos:definition>
    <cco:ont00001754 rdf:datatype="http://www.w3.org/2001/XMLSchema#anyURI">https://en.wikipedia.org/w/index.php?title=Academic_journal&amp;oldid=1059723283</cco:ont00001754>
    <cco:ont00001760 rdf:datatype="http://www.w3.org/2001/XMLSchema#anyURI">https://www.commoncoreontologies.org/InformationEntityOntology</cco:ont00001760>
  </rdf:Description>
  <rdf:Description rdf:nodeID="na8580e9876f64da8bd2fccebf064ee6cb4">
    <rdf:first rdf:resource="https://www.commoncoreontologies.org/ont00001982"/>
    <rdf:rest rdf:resource="http://www.w3.org/1999/02/22-rdf-syntax-ns#nil"/>
  </rdf:Description>
  <rdf:Description rdf:nodeID="na8580e9876f64da8bd2fccebf064ee6cb77">
    <rdf:first rdf:resource="https://www.commoncoreontologies.org/ont00001163"/>
    <rdf:rest rdf:nodeID="na8580e9876f64da8bd2fccebf064ee6cb78"/>
  </rdf:Description>
  <rdf:Description rdf:nodeID="na8580e9876f64da8bd2fccebf064ee6cb79">
    <rdf:type rdf:resource="http://www.w3.org/2002/07/owl#Restriction"/>
    <owl:onProperty rdf:resource="http://purl.obolibrary.org/obo/BFO_0000176"/>
    <owl:someValuesFrom rdf:resource="https://www.commoncoreontologies.org/ont00002039"/>
  </rdf:Description>
  <rdf:Description rdf:nodeID="na8580e9876f64da8bd2fccebf064ee6cb52">
    <rdf:type rdf:resource="http://www.w3.org/2002/07/owl#Restriction"/>
    <owl:onProperty rdf:resource="https://www.commoncoreontologies.org/ont00001808"/>
    <owl:someValuesFrom rdf:resource="http://purl.obolibrary.org/obo/BFO_0000001"/>
  </rdf:Description>
  <rdf:Description rdf:about="https://www.commoncoreontologies.org/ont00000498">
    <rdf:type rdf:resource="http://www.w3.org/2002/07/owl#Class"/>
  </rdf:Description>
  <rdf:Description rdf:about="https://www.commoncoreontologies.org/ont00001419">
    <rdf:type rdf:resource="http://www.w3.org/2002/07/owl#NamedIndividual"/>
    <rdf:type rdf:resource="https://www.commoncoreontologies.org/ont00001352"/>
    <rdfs:label xml:lang="en">GMT+5</rdfs:label>
    <skos:altLabel xml:lang="en">PLT</skos:altLabel>
    <skos:altLabel xml:lang="en">Pakistan Lahore Time</skos:altLabel>
    <cco:ont00001760 rdf:datatype="http://www.w3.org/2001/XMLSchema#anyURI">https://www.commoncoreontologies.org/InformationEntityOntology</cco:ont00001760>
  </rdf:Description>
  <rdf:Description rdf:nodeID="na8580e9876f64da8bd2fccebf064ee6cb25">
    <rdf:first rdf:resource="https://www.commoncoreontologies.org/ont00000686"/>
    <rdf:rest rdf:nodeID="na8580e9876f64da8bd2fccebf064ee6cb26"/>
  </rdf:Description>
  <rdf:Description rdf:nodeID="na8580e9876f64da8bd2fccebf064ee6cb31">
    <owl:intersectionOf rdf:nodeID="na8580e9876f64da8bd2fccebf064ee6cb33"/>
    <rdf:type rdf:resource="http://www.w3.org/2002/07/owl#Class"/>
  </rdf:Description>
  <rdf:Description rdf:nodeID="na8580e9876f64da8bd2fccebf064ee6cb26">
    <rdf:first rdf:nodeID="na8580e9876f64da8bd2fccebf064ee6cb24"/>
    <rdf:rest rdf:resource="http://www.w3.org/1999/02/22-rdf-syntax-ns#nil"/>
  </rdf:Description>
  <rdf:Description rdf:about="https://www.commoncoreontologies.org/ont00001205">
    <rdf:type rdf:resource="http://www.w3.org/2002/07/owl#Class"/>
    <rdfs:subClassOf rdf:resource="https://www.commoncoreontologies.org/ont00000398"/>
    <rdfs:label xml:lang="en">Priority Scale</rdfs:label>
    <skos:definition xml:lang="en">A Reference System that is designed to be used to rank or identify the importance of entities of the specified type.</skos:definition>
    <cco:ont00001760 rdf:datatype="http://www.w3.org/2001/XMLSchema#anyURI">https://www.commoncoreontologies.org/InformationEntityOntology</cco:ont00001760>
  </rdf:Description>
  <rdf:Description rdf:about="https://www.commoncoreontologies.org/ont00001770">
    <rdf:type rdf:resource="http://www.w3.org/2002/07/owl#DatatypeProperty"/>
    <rdfs:domain rdf:resource="https://www.commoncoreontologies.org/ont00000253"/>
    <rdfs:range rdf:resource="http://www.w3.org/2001/XMLSchema#double"/>
    <rdfs:label xml:lang="en">has double value</rdfs:label>
    <skos:definition xml:lang="en">A data property that has as its range a double value.</skos:definition>
    <cco:ont00001760 rdf:datatype="http://www.w3.org/2001/XMLSchema#anyURI">https://www.commoncoreontologies.org/InformationEntityOntology</cco:ont00001760>
  </rdf:Description>
  <rdf:Description rdf:about="https://www.commoncoreontologies.org/ont00000077">
    <rdf:type rdf:resource="http://www.w3.org/2002/07/owl#Class"/>
    <rdfs:subClassOf rdf:resource="https://www.commoncoreontologies.org/ont00000649"/>
    <owl:disjointWith rdf:resource="https://www.commoncoreontologies.org/ont00000923"/>
    <rdfs:label xml:lang="en">Code Identifier</rdfs:label>
    <skos:altLabel xml:lang="en">Code ID</skos:altLabel>
    <skos:altLabel xml:lang="en">ID Code</skos:altLabel>
    <skos:altLabel xml:lang="en">Identifier Code</skos:altLabel>
    <skos:definition xml:lang="en">A Non-Name Identifier that consists of a string of characters that was created and assigned according to an encoding system such that metadata can be derived from the identifier.</skos:definition>
    <cco:ont00001760 rdf:datatype="http://www.w3.org/2001/XMLSchema#anyURI">https://www.commoncoreontologies.org/InformationEntityOntology</cco:ont00001760>
  </rdf:Description>
  <rdf:Description rdf:about="https://www.commoncoreontologies.org/ont00001506">
    <rdf:type rdf:resource="http://www.w3.org/2002/07/owl#NamedIndividual"/>
    <rdf:type rdf:resource="https://www.commoncoreontologies.org/ont00000630"/>
    <rdfs:label xml:lang="en">Universal Time 1 F</rdfs:label>
    <cco:ont00001753>UT1F</cco:ont00001753>
    <cco:ont00001760 rdf:datatype="http://www.w3.org/2001/XMLSchema#anyURI">https://www.commoncoreontologies.org/InformationEntityOntology</cco:ont00001760>
  </rdf:Description>
  <rdf:Description rdf:about="https://www.commoncoreontologies.org/ont00000263">
    <rdf:type rdf:resource="http://www.w3.org/2002/07/owl#Class"/>
    <rdfs:subClassOf rdf:resource="https://www.commoncoreontologies.org/ont00001328"/>
    <rdfs:comment xml:lang="en">A single Clock Time System does not provide a complete means for identifying or measuring times. Depending on the particular Clock Time System, it may be compatible for use with one or more other Temporal Reference Systems.</rdfs:comment>
    <rdfs:label xml:lang="en">Clock Time System</rdfs:label>
    <skos:definition xml:lang="en">A Temporal Reference System that is a convention for keeping and displaying the Time of Day.</skos:definition>
    <cco:ont00001760 rdf:datatype="http://www.w3.org/2001/XMLSchema#anyURI">https://www.commoncoreontologies.org/InformationEntityOntology</cco:ont00001760>
  </rdf:Description>
  <rdf:Description rdf:about="https://www.commoncoreontologies.org/ont00002027">
    <rdf:type rdf:resource="http://www.w3.org/2002/07/owl#Class"/>
    <rdfs:subClassOf rdf:resource="https://www.commoncoreontologies.org/ont00002025"/>
    <rdfs:label xml:lang="en">JAN-13 Barcode</rdfs:label>
    <skos:definition xml:lang="en">An EAN Barcode that is designed to designate 13 numerical digits and is used primarily in Japan to designate products at the point of sale.</skos:definition>
    <cco:ont00001760 rdf:datatype="http://www.w3.org/2001/XMLSchema#anyURI">https://www.commoncoreontologies.org/InformationEntityOntology</cco:ont00001760>
  </rdf:Description>
  <rdf:Description rdf:about="https://www.commoncoreontologies.org/ont00001570">
    <rdf:type rdf:resource="http://www.w3.org/2002/07/owl#NamedIndividual"/>
    <rdf:type rdf:resource="https://www.commoncoreontologies.org/ont00001352"/>
    <rdfs:label xml:lang="en">GMT+2</rdfs:label>
    <skos:altLabel xml:lang="en">EET</skos:altLabel>
    <skos:altLabel xml:lang="en">Eastern European Time</skos:altLabel>
    <cco:ont00001760 rdf:datatype="http://www.w3.org/2001/XMLSchema#anyURI">https://www.commoncoreontologies.org/InformationEntityOntology</cco:ont00001760>
  </rdf:Description>
  <rdf:Description rdf:about="https://www.commoncoreontologies.org/ont00002044">
    <rdf:type rdf:resource="http://www.w3.org/2002/07/owl#Class"/>
    <rdfs:subClassOf rdf:resource="https://www.commoncoreontologies.org/ont00002039"/>
    <rdfs:label xml:lang="en">Form Document</rdfs:label>
    <skos:definition xml:lang="en">A Document Content Entity that has Document Field Contents as parts.</skos:definition>
    <cco:ont00001754>https://en.wikipedia.org/wiki/Form_(document)</cco:ont00001754>
    <cco:ont00001760 rdf:datatype="http://www.w3.org/2001/XMLSchema#anyURI">https://www.commoncoreontologies.org/InformationEntityOntology</cco:ont00001760>
  </rdf:Description>
  <rdf:Description rdf:about="https://www.commoncoreontologies.org/ont00002036">
    <rdf:type rdf:resource="http://www.w3.org/2002/07/owl#Class"/>
    <rdfs:subClassOf rdf:resource="https://www.commoncoreontologies.org/ont00002034"/>
    <rdfs:label xml:lang="en">UPC-E Barcode</rdfs:label>
    <skos:definition xml:lang="en">A UPC Barcode that represents 6 numerical digits.</skos:definition>
    <cco:ont00001760 rdf:datatype="http://www.w3.org/2001/XMLSchema#anyURI">https://www.commoncoreontologies.org/InformationEntityOntology</cco:ont00001760>
  </rdf:Description>
  <rdf:Description rdf:nodeID="na8580e9876f64da8bd2fccebf064ee6cb63">
    <owl:intersectionOf rdf:nodeID="na8580e9876f64da8bd2fccebf064ee6cb65"/>
    <rdf:type rdf:resource="http://www.w3.org/2002/07/owl#Class"/>
  </rdf:Description>
  <rdf:Description rdf:about="https://www.commoncoreontologies.org/ont00002004">
    <rdf:type rdf:resource="http://www.w3.org/2002/07/owl#Class"/>
    <rdfs:subClassOf rdf:resource="https://www.commoncoreontologies.org/ont00002001"/>
    <rdfs:label xml:lang="en">Image</rdfs:label>
    <skos:definition xml:lang="en">A Media Content Entity represents some entity owing to a visual isomorphism between the carrying artifact and the entity.</skos:definition>
    <cco:ont00001754 rdf:datatype="http://www.w3.org/2001/XMLSchema#anyURI">https://en.wikipedia.org/w/index.php?title=Image&amp;oldid=1062709732</cco:ont00001754>
    <cco:ont00001760 rdf:datatype="http://www.w3.org/2001/XMLSchema#anyURI">https://www.commoncoreontologies.org/InformationEntityOntology</cco:ont00001760>
  </rdf:Description>
  <rdf:Description rdf:nodeID="na8580e9876f64da8bd2fccebf064ee6cb58">
    <rdf:first rdf:nodeID="na8580e9876f64da8bd2fccebf064ee6cb56"/>
    <rdf:rest rdf:resource="http://www.w3.org/1999/02/22-rdf-syntax-ns#nil"/>
  </rdf:Description>
  <rdf:Description rdf:nodeID="na8580e9876f64da8bd2fccebf064ee6cb27">
    <owl:intersectionOf rdf:nodeID="na8580e9876f64da8bd2fccebf064ee6cb29"/>
    <rdf:type rdf:resource="http://www.w3.org/2002/07/owl#Class"/>
  </rdf:Description>
  <rdf:Description rdf:about="https://www.commoncoreontologies.org/ont00002028">
    <rdf:type rdf:resource="http://www.w3.org/2002/07/owl#Class"/>
    <rdfs:subClassOf rdf:resource="https://www.commoncoreontologies.org/ont00002025"/>
    <rdfs:label xml:lang="en">EAN-13 Barcode</rdfs:label>
    <skos:definition xml:lang="en">An EAN Barcode that represents 13 numerical digits and is used to designate products at the point of sale.</skos:definition>
    <cco:ont00001760 rdf:datatype="http://www.w3.org/2001/XMLSchema#anyURI">https://www.commoncoreontologies.org/InformationEntityOntology</cco:ont00001760>
  </rdf:Description>
  <rdf:Description rdf:about="https://www.commoncoreontologies.org/ont00001704">
    <rdf:type rdf:resource="http://www.w3.org/2002/07/owl#NamedIndividual"/>
    <rdf:type rdf:resource="https://www.commoncoreontologies.org/ont00001352"/>
    <rdfs:label xml:lang="en">GMT+3</rdfs:label>
    <skos:altLabel xml:lang="en">EAT</skos:altLabel>
    <skos:altLabel xml:lang="en">Eastern African Time</skos:altLabel>
    <cco:ont00001760 rdf:datatype="http://www.w3.org/2001/XMLSchema#anyURI">https://www.commoncoreontologies.org/InformationEntityOntology</cco:ont00001760>
  </rdf:Description>
  <rdf:Description rdf:about="https://www.commoncoreontologies.org/ont00001581">
    <rdf:type rdf:resource="http://www.w3.org/2002/07/owl#NamedIndividual"/>
    <rdf:type rdf:resource="https://www.commoncoreontologies.org/ont00000469"/>
    <rdfs:comment xml:lang="en">The ITRS definition fulfills the following conditions:
1. It is geocentric, the center of mass being defined for the whole earth, including oceans and atmosphere.
2. The unit of length is the metre (SI). This scale is consistent with the TCG time coordinate for a geocentric local frame, in agreement with IAU and IUGG (1991) resolutions. This is obtained by appropriate relativistic modelling.
3. Its orientation was initially given by the BIH orientation at 1984.0.
4. The time evolution of the orientation is ensured by using a no-net-rotation condition with regards to horizontal tectonic motions over the whole earth.
From: (https://www.iers.org/IERS/EN/Science/ITRS/ITRS.html)</rdfs:comment>
    <rdfs:label xml:lang="en">International Terrestrial Reference System</rdfs:label>
    <cco:ont00001753>ITRS</cco:ont00001753>
    <cco:ont00001760 rdf:datatype="http://www.w3.org/2001/XMLSchema#anyURI">https://www.commoncoreontologies.org/InformationEntityOntology</cco:ont00001760>
  </rdf:Description>
  <rdf:Description rdf:about="https://www.commoncoreontologies.org/ont00001878">
    <rdf:type rdf:resource="http://www.w3.org/2002/07/owl#ObjectProperty"/>
    <owl:inverseOf rdf:resource="https://www.commoncoreontologies.org/ont00001919"/>
    <rdfs:domain rdf:resource="https://www.commoncoreontologies.org/ont00000253"/>
    <rdfs:range rdf:resource="http://purl.obolibrary.org/obo/BFO_0000001"/>
    <rdfs:label xml:lang="en">is mention of</rdfs:label>
    <skos:definition xml:lang="en">x is_mention_of y iff x is an instance Information Bearing Entity and y is an instance of Entity, such that x is used as a reference to y.</skos:definition>
    <cco:ont00001760 rdf:datatype="http://www.w3.org/2001/XMLSchema#anyURI">https://www.commoncoreontologies.org/InformationEntityOntology</cco:ont00001760>
  </rdf:Description>
  <rdf:Description rdf:nodeID="na8580e9876f64da8bd2fccebf064ee6cb70">
    <rdf:first rdf:nodeID="na8580e9876f64da8bd2fccebf064ee6cb68"/>
    <rdf:rest rdf:resource="http://www.w3.org/1999/02/22-rdf-syntax-ns#nil"/>
  </rdf:Description>
  <rdf:Description rdf:nodeID="na8580e9876f64da8bd2fccebf064ee6cb18">
    <rdf:type rdf:resource="http://www.w3.org/2002/07/owl#Restriction"/>
    <owl:onProperty rdf:resource="http://purl.obolibrary.org/obo/BFO_0000197"/>
    <owl:someValuesFrom rdf:resource="https://www.commoncoreontologies.org/ont00000253"/>
  </rdf:Description>
  <rdf:Description rdf:about="https://www.commoncoreontologies.org/ont00000124">
    <rdf:type rdf:resource="http://www.w3.org/2002/07/owl#Class"/>
    <rdfs:subClassOf rdf:resource="https://www.commoncoreontologies.org/ont00001328"/>
    <rdfs:label xml:lang="en">Solar Time Reference System</rdfs:label>
    <skos:definition xml:lang="en">A Temporal Reference System that is based on the position of the Sun in the sky.</skos:definition>
    <cco:ont00001760 rdf:datatype="http://www.w3.org/2001/XMLSchema#anyURI">https://www.commoncoreontologies.org/InformationEntityOntology</cco:ont00001760>
  </rdf:Description>
  <rdf:Description rdf:about="https://www.commoncoreontologies.org/ont00001700">
    <rdf:type rdf:resource="http://www.w3.org/2002/07/owl#NamedIndividual"/>
    <rdf:type rdf:resource="https://www.commoncoreontologies.org/ont00001235"/>
    <rdfs:comment xml:lang="en">Juliet time is used as an indexical to refer to local time without otherwise specifying the time zone.</rdfs:comment>
    <rdfs:label xml:lang="en">Juliet Time Zone</rdfs:label>
    <cco:ont00001753>J</cco:ont00001753>
    <cco:ont00001760 rdf:datatype="http://www.w3.org/2001/XMLSchema#anyURI">https://www.commoncoreontologies.org/InformationEntityOntology</cco:ont00001760>
  </rdf:Description>
  <rdf:Description rdf:about="https://www.commoncoreontologies.org/ont00001340">
    <rdf:type rdf:resource="http://www.w3.org/2002/07/owl#Class"/>
    <rdfs:subClassOf rdf:resource="https://www.commoncoreontologies.org/ont00000529"/>
    <rdfs:label xml:lang="en">Calendar Date Identifier</rdfs:label>
    <skos:definition xml:lang="en">A Date Identifier that designates some Day by using a combination of Day, Week, Month, or Year Identifiers formatted according to an implementation of a Calendar System.</skos:definition>
    <skos:example>January 1, 2018; 1 January 2018; 01/01/18; 01Jan18</skos:example>
    <cco:ont00001760 rdf:datatype="http://www.w3.org/2001/XMLSchema#anyURI">https://www.commoncoreontologies.org/InformationEntityOntology</cco:ont00001760>
  </rdf:Description>
  <rdf:Description rdf:about="https://www.commoncoreontologies.org/ont00001873">
    <rdf:type rdf:resource="http://www.w3.org/2002/07/owl#ObjectProperty"/>
    <rdfs:subPropertyOf rdf:resource="https://www.commoncoreontologies.org/ont00001801"/>
    <owl:inverseOf rdf:resource="https://www.commoncoreontologies.org/ont00001938"/>
    <rdfs:range rdf:resource="https://www.commoncoreontologies.org/ont00001069"/>
    <rdfs:comment>See notes for inverse property.</rdfs:comment>
    <rdfs:label xml:lang="en">represented by</rdfs:label>
    <skos:definition xml:lang="en">y represented_by x iff x is an instance of Representational Information Content Entity, and y is an instance of Entity, and z is carrier of x, such that x is about y in virtue of there existing an isomorphism between characteristics of z and y.</skos:definition>
    <cco:ont00001760 rdf:datatype="http://www.w3.org/2001/XMLSchema#anyURI">https://www.commoncoreontologies.org/InformationEntityOntology</cco:ont00001760>
  </rdf:Description>
  <rdf:Description rdf:about="https://www.commoncoreontologies.org/ont00001408">
    <rdf:type rdf:resource="http://www.w3.org/2002/07/owl#NamedIndividual"/>
    <rdf:type rdf:resource="https://www.commoncoreontologies.org/ont00001235"/>
    <rdfs:comment xml:lang="en">Offset from Universal Coordinated Time = UTC-11</rdfs:comment>
    <rdfs:label xml:lang="en">X-ray Time Zone</rdfs:label>
    <cco:ont00001753>X</cco:ont00001753>
    <cco:ont00001760 rdf:datatype="http://www.w3.org/2001/XMLSchema#anyURI">https://www.commoncoreontologies.org/InformationEntityOntology</cco:ont00001760>
  </rdf:Description>
  <rdf:Description rdf:about="https://www.commoncoreontologies.org/ont00001524">
    <rdf:type rdf:resource="http://www.w3.org/2002/07/owl#NamedIndividual"/>
    <rdf:type rdf:resource="https://www.commoncoreontologies.org/ont00001352"/>
    <rdfs:label xml:lang="en">GMT-11</rdfs:label>
    <skos:altLabel xml:lang="en">MIT</skos:altLabel>
    <skos:altLabel xml:lang="en">Midway Islands Time</skos:altLabel>
    <cco:ont00001760 rdf:datatype="http://www.w3.org/2001/XMLSchema#anyURI">https://www.commoncoreontologies.org/InformationEntityOntology</cco:ont00001760>
  </rdf:Description>
  <rdf:Description rdf:nodeID="na8580e9876f64da8bd2fccebf064ee6cb8">
    <rdf:first rdf:nodeID="na8580e9876f64da8bd2fccebf064ee6cb6"/>
    <rdf:rest rdf:resource="http://www.w3.org/1999/02/22-rdf-syntax-ns#nil"/>
  </rdf:Description>
  <rdf:Description rdf:about="https://www.commoncoreontologies.org/ont00001149">
    <rdf:type rdf:resource="http://www.w3.org/2002/07/owl#Class"/>
    <rdfs:subClassOf rdf:resource="https://www.commoncoreontologies.org/ont00001101"/>
    <rdfs:label xml:lang="en">Data Range Interval Estimate Information Content Entity</rdfs:label>
    <skos:definition xml:lang="en">A Ratio Measurement Information Content Entity that is a measurement of a set of values and is equal to the absolute difference between the largest value and the smallest value in the set.</skos:definition>
    <cco:ont00001760 rdf:datatype="http://www.w3.org/2001/XMLSchema#anyURI">https://www.commoncoreontologies.org/InformationEntityOntology</cco:ont00001760>
  </rdf:Description>
  <rdf:Description rdf:about="https://www.commoncoreontologies.org/ont00001768">
    <rdf:type rdf:resource="http://www.w3.org/2002/07/owl#DatatypeProperty"/>
    <rdfs:domain rdf:resource="https://www.commoncoreontologies.org/ont00000253"/>
    <rdfs:range rdf:resource="http://www.w3.org/2001/XMLSchema#anyURI"/>
    <rdfs:label xml:lang="en">has URI value</rdfs:label>
    <skos:definition xml:lang="en">A data property that has as its range a URI value.</skos:definition>
    <cco:ont00001760 rdf:datatype="http://www.w3.org/2001/XMLSchema#anyURI">https://www.commoncoreontologies.org/InformationEntityOntology</cco:ont00001760>
  </rdf:Description>
  <rdf:Description rdf:about="https://www.commoncoreontologies.org/ont00001615">
    <rdf:type rdf:resource="http://www.w3.org/2002/07/owl#NamedIndividual"/>
    <rdf:type rdf:resource="https://www.commoncoreontologies.org/ont00001352"/>
    <rdfs:label xml:lang="en">GMT-7</rdfs:label>
    <skos:altLabel xml:lang="en">MST</skos:altLabel>
    <skos:altLabel xml:lang="en">Mountain Standard Time</skos:altLabel>
    <skos:altLabel xml:lang="en">PNT</skos:altLabel>
    <skos:altLabel xml:lang="en">Phoenix Standard Time</skos:altLabel>
    <cco:ont00001760 rdf:datatype="http://www.w3.org/2001/XMLSchema#anyURI">https://www.commoncoreontologies.org/InformationEntityOntology</cco:ont00001760>
  </rdf:Description>
  <rdf:Description rdf:about="https://www.commoncoreontologies.org/ont00001554">
    <rdf:type rdf:resource="http://www.w3.org/2002/07/owl#NamedIndividual"/>
    <rdf:type rdf:resource="https://www.commoncoreontologies.org/ont00001352"/>
    <rdfs:label xml:lang="en">GMT-10</rdfs:label>
    <skos:altLabel xml:lang="en">HST</skos:altLabel>
    <skos:altLabel xml:lang="en">Hawaii Standard Time</skos:altLabel>
    <cco:ont00001760 rdf:datatype="http://www.w3.org/2001/XMLSchema#anyURI">https://www.commoncoreontologies.org/InformationEntityOntology</cco:ont00001760>
  </rdf:Description>
  <rdf:Description rdf:nodeID="na8580e9876f64da8bd2fccebf064ee6cb20">
    <rdf:type rdf:resource="http://www.w3.org/2002/07/owl#Restriction"/>
    <owl:onProperty rdf:resource="https://www.commoncoreontologies.org/ont00001916"/>
    <owl:someValuesFrom rdf:resource="http://purl.obolibrary.org/obo/BFO_0000006"/>
  </rdf:Description>
  <rdf:Description rdf:about="https://www.commoncoreontologies.org/ont00001431">
    <rdf:type rdf:resource="http://www.w3.org/2002/07/owl#NamedIndividual"/>
    <rdf:type rdf:resource="https://www.commoncoreontologies.org/ont00001235"/>
    <rdfs:comment xml:lang="en">Offset from Universal Coordinated Time = UTC-10</rdfs:comment>
    <rdfs:label xml:lang="en">Whiskey Time Zone</rdfs:label>
    <cco:ont00001753>W</cco:ont00001753>
    <cco:ont00001760 rdf:datatype="http://www.w3.org/2001/XMLSchema#anyURI">https://www.commoncoreontologies.org/InformationEntityOntology</cco:ont00001760>
  </rdf:Description>
  <rdf:Description rdf:about="https://www.commoncoreontologies.org/ont00002013">
    <rdf:type rdf:resource="http://www.w3.org/2002/07/owl#Class"/>
    <rdfs:subClassOf rdf:resource="https://www.commoncoreontologies.org/ont00002010"/>
    <rdfs:label xml:lang="en">Notification Message</rdfs:label>
    <skos:definition xml:lang="en">A Message that describes a scenario that has been determined to merit attention by the recipient.</skos:definition>
    <cco:ont00001760 rdf:datatype="http://www.w3.org/2001/XMLSchema#anyURI">https://www.commoncoreontologies.org/InformationEntityOntology</cco:ont00001760>
  </rdf:Description>
  <rdf:Description rdf:about="https://www.commoncoreontologies.org/ont00001630">
    <rdf:type rdf:resource="http://www.w3.org/2002/07/owl#NamedIndividual"/>
    <rdf:type rdf:resource="https://www.commoncoreontologies.org/ont00000469"/>
    <rdfs:comment xml:lang="en">"WGS 84 is an Earth-centered, Earth-fixed terrestrial reference system and geodetic datum. WGS 84 is based on a consistent set of constants and model parameters that describe the Earth's size, shape, and gravity and geomagnetic fields. WGS 84 is the standard U.S. Department of Defense definition of a global reference system for geospatial information and is the reference system for the Global Positioning System (GPS). It is compatible with the International Terrestrial Reference System (ITRS)."
From: (http://www.unoosa.org/pdf/icg/2012/template/WGS_84.pdf)</rdfs:comment>
    <rdfs:label xml:lang="en">World Geodetic System 1984</rdfs:label>
    <cco:ont00001753>WGS 84</cco:ont00001753>
    <cco:ont00001760 rdf:datatype="http://www.w3.org/2001/XMLSchema#anyURI">https://www.commoncoreontologies.org/InformationEntityOntology</cco:ont00001760>
  </rdf:Description>
  <rdf:Description rdf:nodeID="na8580e9876f64da8bd2fccebf064ee6cb59">
    <owl:intersectionOf rdf:nodeID="na8580e9876f64da8bd2fccebf064ee6cb61"/>
    <rdf:type rdf:resource="http://www.w3.org/2002/07/owl#Class"/>
  </rdf:Description>
  <rdf:Description rdf:about="https://www.commoncoreontologies.org/ont00001480">
    <rdf:type rdf:resource="http://www.w3.org/2002/07/owl#NamedIndividual"/>
    <rdf:type rdf:resource="https://www.commoncoreontologies.org/ont00001235"/>
    <rdfs:comment xml:lang="en">Offset from Universal Coordinated Time = UTC+9</rdfs:comment>
    <rdfs:label xml:lang="en">India Time Zone</rdfs:label>
    <cco:ont00001753>I</cco:ont00001753>
    <cco:ont00001760 rdf:datatype="http://www.w3.org/2001/XMLSchema#anyURI">https://www.commoncoreontologies.org/InformationEntityOntology</cco:ont00001760>
  </rdf:Description>
  <rdf:Description rdf:about="https://www.commoncoreontologies.org/ont00001565">
    <rdf:type rdf:resource="http://www.w3.org/2002/07/owl#NamedIndividual"/>
    <rdf:type rdf:resource="https://www.commoncoreontologies.org/ont00001352"/>
    <rdfs:label xml:lang="en">GMT-5</rdfs:label>
    <skos:altLabel xml:lang="en">EST</skos:altLabel>
    <skos:altLabel xml:lang="en">Eastern Standard Time</skos:altLabel>
    <skos:altLabel xml:lang="en">IET</skos:altLabel>
    <skos:altLabel xml:lang="en">Indiana Eastern Standard Time</skos:altLabel>
    <cco:ont00001760 rdf:datatype="http://www.w3.org/2001/XMLSchema#anyURI">https://www.commoncoreontologies.org/InformationEntityOntology</cco:ont00001760>
  </rdf:Description>
  <rdf:Description rdf:nodeID="na8580e9876f64da8bd2fccebf064ee6cb11">
    <rdf:type rdf:resource="http://www.w3.org/2002/07/owl#Restriction"/>
    <owl:onProperty rdf:resource="http://purl.obolibrary.org/obo/BFO_0000101"/>
    <owl:someValuesFrom rdf:resource="https://www.commoncoreontologies.org/ont00000958"/>
  </rdf:Description>
  <rdf:Description rdf:nodeID="na8580e9876f64da8bd2fccebf064ee6cb17">
    <rdf:first rdf:nodeID="na8580e9876f64da8bd2fccebf064ee6cb15"/>
    <rdf:rest rdf:resource="http://www.w3.org/1999/02/22-rdf-syntax-ns#nil"/>
  </rdf:Description>
  <rdf:Description rdf:nodeID="na8580e9876f64da8bd2fccebf064ee6cb61">
    <rdf:first rdf:resource="https://www.commoncoreontologies.org/ont00001163"/>
    <rdf:rest rdf:nodeID="na8580e9876f64da8bd2fccebf064ee6cb62"/>
  </rdf:Description>
  <rdf:Description rdf:about="https://www.commoncoreontologies.org/ont00001550">
    <rdf:type rdf:resource="http://www.w3.org/2002/07/owl#NamedIndividual"/>
    <rdf:type rdf:resource="https://www.commoncoreontologies.org/ont00000276"/>
    <rdfs:comment xml:lang="en">The Julian Calendar was proposed by Julius Caesar as a reform of the Roman Calendar, took effect on 1 January 46 BC, and was the predominant Calendar System in Europe until being largely replaced by the Gregorian Calendar.</rdfs:comment>
    <rdfs:label xml:lang="en">Julian Calendar</rdfs:label>
    <skos:definition xml:lang="en">A Solar Calendar System that has a regular Year of 365 24-Hour Days divided into 12 Months with a leap day added at the end of February every 4 Years such that the average length of a Julian Year is 365.25 Days.</skos:definition>
    <cco:ont00001754 rdf:datatype="http://www.w3.org/2001/XMLSchema#anyURI">https://en.wikipedia.org/w/index.php?title=Julian_calendar&amp;oldid=1063127575</cco:ont00001754>
    <cco:ont00001760 rdf:datatype="http://www.w3.org/2001/XMLSchema#anyURI">https://www.commoncoreontologies.org/InformationEntityOntology</cco:ont00001760>
  </rdf:Description>
  <rdf:Description rdf:nodeID="na8580e9876f64da8bd2fccebf064ee6cb28">
    <rdf:type rdf:resource="http://www.w3.org/2002/07/owl#Restriction"/>
    <owl:onProperty rdf:resource="https://www.commoncoreontologies.org/ont00001916"/>
    <owl:someValuesFrom rdf:resource="https://www.commoncoreontologies.org/ont00000800"/>
  </rdf:Description>
  <rdf:Description rdf:nodeID="na8580e9876f64da8bd2fccebf064ee6cb24">
    <rdf:type rdf:resource="http://www.w3.org/2002/07/owl#Restriction"/>
    <owl:onProperty rdf:resource="https://www.commoncoreontologies.org/ont00001916"/>
    <owl:someValuesFrom rdf:resource="http://purl.obolibrary.org/obo/BFO_0000008"/>
  </rdf:Description>
  <rdf:Description rdf:nodeID="na8580e9876f64da8bd2fccebf064ee6cb78">
    <rdf:first rdf:nodeID="na8580e9876f64da8bd2fccebf064ee6cb76"/>
    <rdf:rest rdf:resource="http://www.w3.org/1999/02/22-rdf-syntax-ns#nil"/>
  </rdf:Description>
  <rdf:Description rdf:nodeID="na8580e9876f64da8bd2fccebf064ee6cb37">
    <rdf:first rdf:resource="https://www.commoncoreontologies.org/ont00000958"/>
    <rdf:rest rdf:nodeID="na8580e9876f64da8bd2fccebf064ee6cb38"/>
  </rdf:Description>
  <rdf:Description rdf:nodeID="na8580e9876f64da8bd2fccebf064ee6cb42">
    <rdf:first rdf:resource="https://www.commoncoreontologies.org/ont00000540"/>
    <rdf:rest rdf:nodeID="na8580e9876f64da8bd2fccebf064ee6cb43"/>
  </rdf:Description>
  <rdf:Description rdf:nodeID="na8580e9876f64da8bd2fccebf064ee6cb74">
    <rdf:first rdf:nodeID="na8580e9876f64da8bd2fccebf064ee6cb72"/>
    <rdf:rest rdf:resource="http://www.w3.org/1999/02/22-rdf-syntax-ns#nil"/>
  </rdf:Description>
  <rdf:Description rdf:nodeID="na8580e9876f64da8bd2fccebf064ee6cb51">
    <owl:intersectionOf rdf:nodeID="na8580e9876f64da8bd2fccebf064ee6cb53"/>
    <rdf:type rdf:resource="http://www.w3.org/2002/07/owl#Class"/>
  </rdf:Description>
  <rdf:Description rdf:nodeID="na8580e9876f64da8bd2fccebf064ee6cb7">
    <rdf:first rdf:resource="https://www.commoncoreontologies.org/ont00000399"/>
    <rdf:rest rdf:nodeID="na8580e9876f64da8bd2fccebf064ee6cb8"/>
  </rdf:Description>
  <rdf:Description rdf:about="https://www.commoncoreontologies.org/ont00002018">
    <rdf:type rdf:resource="http://www.w3.org/2002/07/owl#Class"/>
    <rdfs:subClassOf rdf:resource="https://www.commoncoreontologies.org/ont00002015"/>
    <rdfs:label xml:lang="en">QR Code</rdfs:label>
    <skos:definition xml:lang="en">A Two-Dimensional Barcode that represents numeric, alphanumeric, binary, or kanji information and is used primarily for tracking and marketing.</skos:definition>
    <cco:ont00001760 rdf:datatype="http://www.w3.org/2001/XMLSchema#anyURI">https://www.commoncoreontologies.org/InformationEntityOntology</cco:ont00001760>
  </rdf:Description>
  <rdf:Description rdf:nodeID="na8580e9876f64da8bd2fccebf064ee6cb9">
    <rdf:type rdf:resource="http://www.w3.org/2002/07/owl#Restriction"/>
    <owl:onProperty rdf:resource="https://www.commoncoreontologies.org/ont00001980"/>
    <owl:someValuesFrom rdf:resource="http://purl.obolibrary.org/obo/BFO_0000001"/>
  </rdf:Description>
  <rdf:Description rdf:nodeID="na8580e9876f64da8bd2fccebf064ee6cb14">
    <owl:intersectionOf rdf:nodeID="na8580e9876f64da8bd2fccebf064ee6cb16"/>
    <rdf:type rdf:resource="http://www.w3.org/2002/07/owl#Class"/>
  </rdf:Description>
  <rdf:Description rdf:nodeID="na8580e9876f64da8bd2fccebf064ee6cb39">
    <rdf:type rdf:resource="http://www.w3.org/2002/07/owl#Restriction"/>
    <owl:onProperty rdf:resource="https://www.commoncoreontologies.org/ont00001916"/>
    <owl:someValuesFrom rdf:resource="https://www.commoncoreontologies.org/ont00000498"/>
  </rdf:Description>
  <rdf:Description rdf:about="https://www.commoncoreontologies.org/ont00001421">
    <rdf:type rdf:resource="http://www.w3.org/2002/07/owl#NamedIndividual"/>
    <rdf:type rdf:resource="https://www.commoncoreontologies.org/ont00001235"/>
    <rdfs:comment xml:lang="en">Offset from Universal Coordinated Time = UTC-6</rdfs:comment>
    <rdfs:label xml:lang="en">Sierra Time Zone</rdfs:label>
    <cco:ont00001753>S</cco:ont00001753>
    <cco:ont00001760 rdf:datatype="http://www.w3.org/2001/XMLSchema#anyURI">https://www.commoncoreontologies.org/InformationEntityOntology</cco:ont00001760>
  </rdf:Description>
  <rdf:Description rdf:nodeID="na8580e9876f64da8bd2fccebf064ee6cb66">
    <rdf:first rdf:nodeID="na8580e9876f64da8bd2fccebf064ee6cb64"/>
    <rdf:rest rdf:resource="http://www.w3.org/1999/02/22-rdf-syntax-ns#nil"/>
  </rdf:Description>
  <rdf:Description rdf:nodeID="na8580e9876f64da8bd2fccebf064ee6cb67">
    <owl:intersectionOf rdf:nodeID="na8580e9876f64da8bd2fccebf064ee6cb69"/>
    <rdf:type rdf:resource="http://www.w3.org/2002/07/owl#Class"/>
  </rdf:Description>
  <rdf:Description rdf:nodeID="na8580e9876f64da8bd2fccebf064ee6cb41">
    <rdf:type rdf:resource="http://www.w3.org/2002/07/owl#Restriction"/>
    <owl:onProperty rdf:resource="https://www.commoncoreontologies.org/ont00001916"/>
    <owl:someValuesFrom rdf:resource="https://www.commoncoreontologies.org/ont00000223"/>
  </rdf:Description>
  <rdf:Description rdf:about="https://www.commoncoreontologies.org/ont00001760">
    <rdf:type rdf:resource="http://www.w3.org/2002/07/owl#AnnotationProperty"/>
  </rdf:Description>
  <rdf:Description rdf:nodeID="na8580e9876f64da8bd2fccebf064ee6cb68">
    <rdf:type rdf:resource="http://www.w3.org/2002/07/owl#Restriction"/>
    <owl:onProperty rdf:resource="https://www.commoncoreontologies.org/ont00001938"/>
    <owl:someValuesFrom rdf:resource="http://purl.obolibrary.org/obo/BFO_0000001"/>
  </rdf:Description>
  <rdf:Description rdf:nodeID="na8580e9876f64da8bd2fccebf064ee6cb64">
    <rdf:type rdf:resource="http://www.w3.org/2002/07/owl#Restriction"/>
    <owl:onProperty rdf:resource="https://www.commoncoreontologies.org/ont00001983"/>
    <owl:someValuesFrom rdf:resource="http://purl.obolibrary.org/obo/BFO_0000001"/>
  </rdf:Description>
  <rdf:Description rdf:about="http://purl.org/dc/terms/rights">
    <rdf:type rdf:resource="http://www.w3.org/2002/07/owl#AnnotationProperty"/>
  </rdf:Description>
  <rdf:Description rdf:about="https://www.commoncoreontologies.org/ont00000223">
    <rdf:type rdf:resource="http://www.w3.org/2002/07/owl#Class"/>
  </rdf:Description>
</rdf:RDF>
